update

theory/Sound_Semantics.thy
@@ -4,9 +4,9 @@ theory Sound_Semantics
 begin
 
 fun value_to_abstract_value :: "val \<Rightarrow> abstract_value" ("|_|" [0]61) where
-  "|\<lbrace>\<rbrace>| = ^\<lparr>\<rparr>" |
-  "|\<lbrace>Ch \<pi> x\<rbrace>| = ^Chan x" |
-  "|\<lbrace>p, \<rho>\<rbrace>| = ^p"
+  "|VUnit| = ^\<lparr>\<rparr>" |
+  "|VChan (Ch \<pi> x)| = ^Chan x" |
+  "|VClosure p \<rho>| = ^p"
 
 
 definition env_to_abstract_value_env :: "(var \<rightharpoonup> val) \<Rightarrow> abstract_value_env" ("\<parallel>_\<parallel>" [0]61) where
@@ -19,35 +19,35 @@ inductive static_eval_value :: "abstract_value_env \<times> abstract_value_env \
 and  static_eval_env :: "abstract_value_env \<times> abstract_value_env \<Rightarrow> val_env \<Rightarrow> bool" (infix "\<Turnstile>\<^sub>\<rho>" 55) 
 where
   Unit: "
-    (\<V>, \<C>) \<Turnstile>\<^sub>\<omega> \<lbrace>\<rbrace>
+    (\<V>, \<C>) \<Turnstile>\<^sub>\<omega> VUnit
   " |
 
   Chan: "
-    (\<V>, \<C>) \<Turnstile>\<^sub>\<omega> \<lbrace>c\<rbrace>
+    (\<V>, \<C>) \<Turnstile>\<^sub>\<omega> VChan c
   " |
 
   Send_Evt: "
     (\<V>, \<C>) \<Turnstile>\<^sub>\<rho> \<rho>
     \<Longrightarrow>
-    (\<V>, \<C>) \<Turnstile>\<^sub>\<omega> \<lbrace>Send_Evt _ _, \<rho>\<rbrace>
+    (\<V>, \<C>) \<Turnstile>\<^sub>\<omega> (VClosure (Send_Evt _ _) \<rho>)
   " |
 
   Recv_Evt: "
     (\<V>, \<C>) \<Turnstile>\<^sub>\<rho> \<rho>
     \<Longrightarrow>
-    (\<V>, \<C>) \<Turnstile>\<^sub>\<omega> \<lbrace>Recv_Evt _, \<rho>\<rbrace>
+    (\<V>, \<C>) \<Turnstile>\<^sub>\<omega> (VClosure (Recv_Evt _) \<rho>)
   " |
 
   Left: "
     (\<V>, \<C>) \<Turnstile>\<^sub>\<rho> \<rho>
     \<Longrightarrow>
-    (\<V>, \<C>) \<Turnstile>\<^sub>\<omega> \<lbrace>Left _, \<rho>\<rbrace>
+    (\<V>, \<C>) \<Turnstile>\<^sub>\<omega> (VClosure (Left _) \<rho>)
   " |
 
   Right: "
     (\<V>, \<C>) \<Turnstile>\<^sub>\<rho> \<rho>
     \<Longrightarrow>
-    (\<V>, \<C>) \<Turnstile>\<^sub>\<omega> \<lbrace>Right _, \<rho>\<rbrace>
+    (\<V>, \<C>) \<Turnstile>\<^sub>\<omega> (VClosure (Right _) \<rho>)
   " |
 
   Abs: "
@@ -56,13 +56,13 @@ where
       (\<V>, \<C>) \<Turnstile>\<^sub>e e;
       (\<V>, \<C>) \<Turnstile>\<^sub>\<rho> \<rho>
     \<rbrakk> \<Longrightarrow> 
-    (\<V>, \<C>) \<Turnstile>\<^sub>\<omega> \<lbrace>Abs f x e, \<rho>\<rbrace>
+    (\<V>, \<C>) \<Turnstile>\<^sub>\<omega> (VClosure (Abs f x e) \<rho>)
   " |
 
   Pair: "
     (\<V>, \<C>) \<Turnstile>\<^sub>\<rho> \<rho>
     \<Longrightarrow>
-    (\<V>, \<C>) \<Turnstile>\<^sub>\<omega> \<lbrace>Pair _ _, \<rho>\<rbrace>
+    (\<V>, \<C>) \<Turnstile>\<^sub>\<omega> (VClosure (Pair _ _) \<rho>)
   " |
 
   Any : "
@@ -117,17 +117,17 @@ qed
 
 lemma static_eval_state_to_exp_let_case_left: "
   (\<V>, \<C>) \<Turnstile>\<^sub>\<sigma> \<langle>LET x = CASE x\<^sub>s LEFT x\<^sub>l |> e\<^sub>l RIGHT x\<^sub>r |> e\<^sub>r in e; \<rho>; \<kappa>\<rangle> \<Longrightarrow> 
-  \<rho> x\<^sub>s = Some \<lbrace>prim.Left x\<^sub>l', \<rho>\<^sub>l\<rbrace> \<Longrightarrow> 
+  \<rho> x\<^sub>s = Some (VClosure (Left x\<^sub>l') \<rho>\<^sub>l) \<Longrightarrow> 
   (\<V>, \<C>) \<Turnstile>\<^sub>e e\<^sub>l
 "
 proof -
-  assume "\<rho> x\<^sub>s = Some \<lbrace>prim.Left x\<^sub>l', \<rho>\<^sub>l\<rbrace>"
+  assume "\<rho> x\<^sub>s = Some (VClosure (Left x\<^sub>l') \<rho>\<^sub>l)"
   assume "(\<V>, \<C>) \<Turnstile>\<^sub>\<sigma> \<langle>LET x = CASE x\<^sub>s LEFT x\<^sub>l |> e\<^sub>l RIGHT x\<^sub>r |> e\<^sub>r in e; \<rho>; \<kappa>\<rangle>" then
   have "(\<V>, \<C>) \<Turnstile>\<^sub>e LET x = CASE x\<^sub>s LEFT x\<^sub>l |> e\<^sub>l RIGHT x\<^sub>r |> e\<^sub>r in e"  
   and "(\<V>, \<C>) \<Turnstile>\<^sub>\<rho> \<rho>"
   by (simp add: static_eval_state.simps)+ then
   have "\<forall>x \<omega>. \<rho> x = Some \<omega> \<longrightarrow> {|\<omega>|} \<subseteq> \<V> x" by (simp add: static_eval_env.simps)
-  with `\<rho> x\<^sub>s = Some \<lbrace>prim.Left x\<^sub>l', \<rho>\<^sub>l\<rbrace>`
+  with `\<rho> x\<^sub>s = Some (VClosure (Left x\<^sub>l') \<rho>\<^sub>l)`
   have "^prim.Left x\<^sub>l' \<in> \<V> x\<^sub>s" by fastforce
   with `(\<V>, \<C>) \<Turnstile>\<^sub>e LET x = CASE x\<^sub>s LEFT x\<^sub>l |> e\<^sub>l RIGHT x\<^sub>r |> e\<^sub>r in e`
   show "(\<V>, \<C>) \<Turnstile>\<^sub>e e\<^sub>l"
@@ -143,17 +143,17 @@ qed
 
 lemma static_eval_state_to_exp_let_case_right: "
   (\<V>, \<C>) \<Turnstile>\<^sub>\<sigma> \<langle>LET x = CASE x\<^sub>s LEFT x\<^sub>l |> e\<^sub>l RIGHT x\<^sub>r |> e\<^sub>r in e; \<rho>; \<kappa>\<rangle> \<Longrightarrow> 
-  \<rho> x\<^sub>s = Some \<lbrace>prim.Right x\<^sub>r', \<rho>\<^sub>r\<rbrace> \<Longrightarrow> 
+  \<rho> x\<^sub>s = Some (VClosure (Right x\<^sub>r') \<rho>\<^sub>r) \<Longrightarrow> 
   (\<V>, \<C>) \<Turnstile>\<^sub>e e\<^sub>r
 "
 proof -
-  assume "\<rho> x\<^sub>s = Some \<lbrace>prim.Right x\<^sub>r', \<rho>\<^sub>r\<rbrace>"
+  assume "\<rho> x\<^sub>s = Some (VClosure (Right x\<^sub>r') \<rho>\<^sub>r)"
   assume "(\<V>, \<C>) \<Turnstile>\<^sub>\<sigma> \<langle>LET x = CASE x\<^sub>s LEFT x\<^sub>l |> e\<^sub>l RIGHT x\<^sub>r |> e\<^sub>r in e; \<rho>; \<kappa>\<rangle>" then
   have "(\<V>, \<C>) \<Turnstile>\<^sub>e LET x = CASE x\<^sub>s LEFT x\<^sub>l |> e\<^sub>l RIGHT x\<^sub>r |> e\<^sub>r in e"  
   and "(\<V>, \<C>) \<Turnstile>\<^sub>\<rho> \<rho>" 
     by (simp add: static_eval_state.simps)+ then
   have "\<forall>x \<omega>. \<rho> x = Some \<omega> \<longrightarrow> {|\<omega>|} \<subseteq> \<V> x" by (simp add: static_eval_env.simps)
-  with `\<rho> x\<^sub>s = Some \<lbrace>prim.Right x\<^sub>r', \<rho>\<^sub>r\<rbrace>`
+  with `\<rho> x\<^sub>s = Some (VClosure (Right x\<^sub>r') \<rho>\<^sub>r)`
   have "^prim.Right x\<^sub>r' \<in> \<V> x\<^sub>s" by fastforce
   with `(\<V>, \<C>) \<Turnstile>\<^sub>e LET x = CASE x\<^sub>s LEFT x\<^sub>l |> e\<^sub>l RIGHT x\<^sub>r |> e\<^sub>r in e`
   show "(\<V>, \<C>) \<Turnstile>\<^sub>e e\<^sub>r"
@@ -179,17 +179,17 @@ qed
 
 lemma static_eval_state_to_exp_let_app: "
  (\<V>, \<C>) \<Turnstile>\<^sub>\<sigma> \<langle>LET x = APP f x\<^sub>a in e; \<rho>; \<kappa>\<rangle> \<Longrightarrow> 
- \<rho> f = Some \<lbrace>Abs f' x\<^sub>p e\<^sub>b, \<rho>'\<rbrace> \<Longrightarrow>
+ \<rho> f = Some (VClosure (Abs f' x\<^sub>p e\<^sub>b) \<rho>') \<Longrightarrow>
  (\<V>, \<C>) \<Turnstile>\<^sub>e e\<^sub>b
 "
 
 proof -
-  assume "\<rho> f = Some \<lbrace>Abs f' x\<^sub>p e\<^sub>b, \<rho>'\<rbrace>"
+  assume "\<rho> f = Some (VClosure (Abs f' x\<^sub>p e\<^sub>b) \<rho>')"
   assume "(\<V>, \<C>) \<Turnstile>\<^sub>\<sigma> \<langle>LET x = APP f x\<^sub>a in e; \<rho>; \<kappa>\<rangle>" then
   have "(\<V>, \<C>) \<Turnstile>\<^sub>\<rho> \<rho>" by (simp add: static_eval_state.simps) then
   have "\<forall>x \<omega>. \<rho> x = Some \<omega> \<longrightarrow> {|\<omega>|} \<subseteq> \<V> x \<and> (\<V>, \<C>) \<Turnstile>\<^sub>\<omega> \<omega>" by (simp add: static_eval_env.simps)
-  with `\<rho> f = Some \<lbrace>Abs f' x\<^sub>p e\<^sub>b, \<rho>'\<rbrace>`
-  have "(\<V>, \<C>) \<Turnstile>\<^sub>\<omega> \<lbrace>Abs f' x\<^sub>p e\<^sub>b, \<rho>'\<rbrace>" by simp then
+  with `\<rho> f = Some (VClosure (Abs f' x\<^sub>p e\<^sub>b) \<rho>')`
+  have "(\<V>, \<C>) \<Turnstile>\<^sub>\<omega> (VClosure (Abs f' x\<^sub>p e\<^sub>b) \<rho>')" by simp then
   show "(\<V>, \<C>) \<Turnstile>\<^sub>e e\<^sub>b" by (rule static_eval_value.cases; auto)
 qed
 
@@ -272,7 +272,7 @@ qed
 
 
 lemma static_eval_state_to_env_let_unit: "
-  (\<V>, \<C>) \<Turnstile>\<^sub>\<sigma> \<langle>LET x = \<lparr>\<rparr> in e; \<rho>; \<kappa>\<rangle> \<Longrightarrow> (\<V>, \<C>) \<Turnstile>\<^sub>\<rho> \<rho>(x \<mapsto> \<lbrace>\<rbrace>)
+  (\<V>, \<C>) \<Turnstile>\<^sub>\<sigma> \<langle>LET x = \<lparr>\<rparr> in e; \<rho>; \<kappa>\<rangle> \<Longrightarrow> (\<V>, \<C>) \<Turnstile>\<^sub>\<rho> \<rho>(x \<mapsto> VUnit)
 "
 proof
   assume "(\<V>, \<C>) \<Turnstile>\<^sub>\<sigma> \<langle>LET x = \<lparr>\<rparr> in e; \<rho>; \<kappa>\<rangle>" then 
@@ -280,20 +280,20 @@ proof
 
   from `(\<V>, \<C>) \<Turnstile>\<^sub>e LET x = \<lparr>\<rparr> in e`
   have "{^\<lparr>\<rparr>} \<subseteq> \<V> x" by (rule static_eval.cases; auto)+
-  have "(\<V>, \<C>) \<Turnstile>\<^sub>\<omega> \<lbrace>\<rbrace>" by (simp add: Unit)
+  have "(\<V>, \<C>) \<Turnstile>\<^sub>\<omega> VUnit" by (simp add: Unit)
 
   {
     fix x' \<omega>'
-    assume "(\<rho>(x \<mapsto> \<lbrace>\<rbrace>)) x' = Some \<omega>'" 
+    assume "(\<rho>(x \<mapsto> VUnit)) x' = Some \<omega>'" 
     have "{|\<omega>'|} \<subseteq> \<V> x' \<and> (\<V>, \<C>) \<Turnstile>\<^sub>\<omega> \<omega>'"
     proof cases
       assume "x' = x" 
-      with `(\<rho>(x \<mapsto> \<lbrace>\<rbrace>)) x' = Some \<omega>'` 
-      and `{^\<lparr>\<rparr>} \<subseteq> \<V> x` `(\<V>, \<C>) \<Turnstile>\<^sub>\<omega> \<lbrace>\<rbrace>`
+      with `(\<rho>(x \<mapsto> VUnit)) x' = Some \<omega>'` 
+      and `{^\<lparr>\<rparr>} \<subseteq> \<V> x` `(\<V>, \<C>) \<Turnstile>\<^sub>\<omega> VUnit`
 
       show "{|\<omega>'|} \<subseteq> \<V> x' \<and> (\<V>, \<C>) \<Turnstile>\<^sub>\<omega> \<omega>'" by simp
     next 
-      assume "x' \<noteq> x"  with `(\<rho>(x \<mapsto> \<lbrace>\<rbrace>)) x' = Some \<omega>'` 
+      assume "x' \<noteq> x"  with `(\<rho>(x \<mapsto> VUnit)) x' = Some \<omega>'` 
 
       have "\<rho> x' = Some \<omega>'" by simp
 
@@ -303,8 +303,8 @@ proof
     qed
 
   }
-  with `{^\<lparr>\<rparr>} \<subseteq> \<V> x` `(\<V>, \<C>) \<Turnstile>\<^sub>\<omega> \<lbrace>\<rbrace>`
-  show "\<forall>x' \<omega>'. (\<rho>(x \<mapsto> \<lbrace>\<rbrace>)) x' = Some \<omega>' \<longrightarrow> {|\<omega>'|} \<subseteq> \<V> x' \<and> (\<V>, \<C>) \<Turnstile>\<^sub>\<omega> \<omega>'" by auto
+  with `{^\<lparr>\<rparr>} \<subseteq> \<V> x` `(\<V>, \<C>) \<Turnstile>\<^sub>\<omega> VUnit`
+  show "\<forall>x' \<omega>'. (\<rho>(x \<mapsto> VUnit)) x' = Some \<omega>' \<longrightarrow> {|\<omega>'|} \<subseteq> \<V> x' \<and> (\<V>, \<C>) \<Turnstile>\<^sub>\<omega> \<omega>'" by auto
 qed
 
 
@@ -314,14 +314,14 @@ lemma static_eval_state_to_stack_let: "
 by (erule static_eval_state.cases; auto)
 
 lemma static_eval_state_to_state_let_unit: "
-  (\<V>, \<C>) \<Turnstile>\<^sub>\<sigma> \<langle>LET x = \<lparr>\<rparr> in e; \<rho>; \<kappa>\<rangle> \<Longrightarrow> (\<V>, \<C>) \<Turnstile>\<^sub>\<sigma> \<langle>e; \<rho>(x \<mapsto> \<lbrace>\<rbrace>); \<kappa>\<rangle>
+  (\<V>, \<C>) \<Turnstile>\<^sub>\<sigma> \<langle>LET x = \<lparr>\<rparr> in e; \<rho>; \<kappa>\<rangle> \<Longrightarrow> (\<V>, \<C>) \<Turnstile>\<^sub>\<sigma> \<langle>e; \<rho>(x \<mapsto> VUnit); \<kappa>\<rangle>
 "
 proof
   assume "(\<V>, \<C>) \<Turnstile>\<^sub>\<sigma> \<langle>LET x = \<lparr>\<rparr> in e; \<rho>; \<kappa>\<rangle>" then
   show "(\<V>, \<C>) \<Turnstile>\<^sub>e e" by (auto simp: static_eval_state_to_exp_let)
 
   from `(\<V>, \<C>) \<Turnstile>\<^sub>\<sigma> \<langle>LET x = \<lparr>\<rparr> in e; \<rho>; \<kappa>\<rangle>` 
-  show "(\<V>, \<C>) \<Turnstile>\<^sub>\<rho> \<rho>(x \<mapsto> \<lbrace>\<rbrace>)" by (auto simp: static_eval_state_to_env_let_unit)
+  show "(\<V>, \<C>) \<Turnstile>\<^sub>\<rho> \<rho>(x \<mapsto> VUnit)" by (auto simp: static_eval_state_to_env_let_unit)
 
   from `(\<V>, \<C>) \<Turnstile>\<^sub>\<sigma> \<langle>LET x = \<lparr>\<rparr> in e; \<rho>; \<kappa>\<rangle>` 
   show "(\<V>, \<C>) \<Turnstile>\<^sub>\<kappa> \<V> (\<lfloor>e\<rfloor>) \<Rrightarrow> \<kappa>" by (auto simp: static_eval_state_to_stack_let)
@@ -329,32 +329,32 @@ proof
 qed
 
 lemma static_eval_to_value_let_prim: "
-  (\<V>, \<C>) \<Turnstile>\<^sub>e LET x = Prim p in e \<Longrightarrow> (\<V>, \<C>) \<Turnstile>\<^sub>\<rho> \<rho> \<Longrightarrow> (\<V>, \<C>) \<Turnstile>\<^sub>\<omega> \<lbrace>p, \<rho>\<rbrace>
+  (\<V>, \<C>) \<Turnstile>\<^sub>e LET x = Prim p in e \<Longrightarrow> (\<V>, \<C>) \<Turnstile>\<^sub>\<rho> \<rho> \<Longrightarrow> (\<V>, \<C>) \<Turnstile>\<^sub>\<omega> (VClosure p \<rho>)
 "
 by (erule static_eval.cases; auto; rule; auto)
 
 lemma static_eval_state_to_env_let_prim: "
-  (\<V>, \<C>) \<Turnstile>\<^sub>\<sigma> \<langle>LET x = Prim p in e; \<rho>; \<kappa>\<rangle> \<Longrightarrow> (\<V>, \<C>) \<Turnstile>\<^sub>\<rho> \<rho>(x \<mapsto> \<lbrace>p, \<rho>\<rbrace>)
+  (\<V>, \<C>) \<Turnstile>\<^sub>\<sigma> \<langle>LET x = Prim p in e; \<rho>; \<kappa>\<rangle> \<Longrightarrow> (\<V>, \<C>) \<Turnstile>\<^sub>\<rho> \<rho>(x \<mapsto> (VClosure p \<rho>))
 "
 proof
   assume "(\<V>, \<C>) \<Turnstile>\<^sub>\<sigma> \<langle>LET x = Prim p in e; \<rho>; \<kappa>\<rangle> " then 
   have "(\<V>, \<C>) \<Turnstile>\<^sub>e LET x = Prim p in e" "(\<V>, \<C>) \<Turnstile>\<^sub>\<rho> \<rho>" by (simp add: static_eval_state.simps)+ then
-  have "(\<V>, \<C>) \<Turnstile>\<^sub>\<omega> \<lbrace>p, \<rho>\<rbrace>" by (simp add: static_eval_to_value_let_prim)
+  have "(\<V>, \<C>) \<Turnstile>\<^sub>\<omega> (VClosure p \<rho>)" by (simp add: static_eval_to_value_let_prim)
 
   from `(\<V>, \<C>) \<Turnstile>\<^sub>e LET x = Prim p in e`
   have "{^p} \<subseteq> \<V> x" by (rule static_eval.cases; auto)+
  
   {
     fix x' \<omega>'
-    assume "(\<rho>(x \<mapsto> \<lbrace>p, \<rho>\<rbrace>)) x' = Some \<omega>'" 
+    assume "(\<rho>(x \<mapsto> (VClosure p \<rho>))) x' = Some \<omega>'" 
     have "{|\<omega>'|} \<subseteq> \<V> x' \<and> (\<V>, \<C>) \<Turnstile>\<^sub>\<omega> \<omega>'"
     proof cases
-      assume "x' = x" with \<open>(\<rho>(x \<mapsto> \<lbrace>p, \<rho>\<rbrace>)) x' = Some \<omega>'\<close>
-      and `{^p} \<subseteq> \<V> x` `(\<V>, \<C>) \<Turnstile>\<^sub>\<omega> \<lbrace>p, \<rho>\<rbrace>`
+      assume "x' = x" with \<open>(\<rho>(x \<mapsto> (VClosure p \<rho>))) x' = Some \<omega>'\<close>
+      and `{^p} \<subseteq> \<V> x` `(\<V>, \<C>) \<Turnstile>\<^sub>\<omega> (VClosure p \<rho>)`
 
       show "{|\<omega>'|} \<subseteq> \<V> x' \<and> (\<V>, \<C>) \<Turnstile>\<^sub>\<omega> \<omega>'" by auto
     next
-      assume  "x' \<noteq> x"  with \<open>(\<rho>(x \<mapsto> \<lbrace>p, \<rho>\<rbrace>)) x' = Some \<omega>'\<close>
+      assume  "x' \<noteq> x"  with \<open>(\<rho>(x \<mapsto> (VClosure p \<rho>))) x' = Some \<omega>'\<close>
 
       have "\<rho> x' = Some \<omega>'" by simp
       with `(\<V>, \<C>) \<Turnstile>\<^sub>\<rho> \<rho>` 
@@ -364,11 +364,11 @@ proof
 
   } then
 
-  show "\<forall>x' \<omega>'. (\<rho>(x \<mapsto> \<lbrace>p, \<rho>\<rbrace>)) x' = Some \<omega>' \<longrightarrow> {|\<omega>'|} \<subseteq> \<V> x' \<and> (\<V>, \<C>) \<Turnstile>\<^sub>\<omega> \<omega>'" by auto
+  show "\<forall>x' \<omega>'. (\<rho>(x \<mapsto> (VClosure p \<rho>))) x' = Some \<omega>' \<longrightarrow> {|\<omega>'|} \<subseteq> \<V> x' \<and> (\<V>, \<C>) \<Turnstile>\<^sub>\<omega> \<omega>'" by auto
 qed
 
 lemma static_eval_state_to_state_let_prim: "
-  (\<V>, \<C>) \<Turnstile>\<^sub>\<sigma> \<langle>LET x = Prim p in e; \<rho>; \<kappa>\<rangle> \<Longrightarrow> (\<V>, \<C>) \<Turnstile>\<^sub>\<sigma> \<langle>e; \<rho>(x \<mapsto> \<lbrace>p, \<rho>\<rbrace>); \<kappa>\<rangle>
+  (\<V>, \<C>) \<Turnstile>\<^sub>\<sigma> \<langle>LET x = Prim p in e; \<rho>; \<kappa>\<rangle> \<Longrightarrow> (\<V>, \<C>) \<Turnstile>\<^sub>\<sigma> \<langle>e; \<rho>(x \<mapsto> (VClosure p \<rho>)); \<kappa>\<rangle>
 "
 proof
   assume "(\<V>, \<C>) \<Turnstile>\<^sub>\<sigma> \<langle>LET x = Prim p in e; \<rho>; \<kappa>\<rangle>" then
@@ -378,31 +378,31 @@ proof
   show "(\<V>, \<C>) \<Turnstile>\<^sub>\<kappa> \<V> (\<lfloor>e\<rfloor>) \<Rrightarrow> \<kappa>" by (auto simp: static_eval_state_to_stack_let)
 
   from `(\<V>, \<C>) \<Turnstile>\<^sub>\<sigma> \<langle>LET x = Prim p in e; \<rho>; \<kappa>\<rangle>` 
-  show "(\<V>, \<C>) \<Turnstile>\<^sub>\<rho> \<rho>(x \<mapsto> \<lbrace>p, \<rho>\<rbrace>)" by (auto simp: static_eval_state_to_env_let_prim)
+  show "(\<V>, \<C>) \<Turnstile>\<^sub>\<rho> \<rho>(x \<mapsto> (VClosure p \<rho>))" by (auto simp: static_eval_state_to_env_let_prim)
 
 qed
 
 
 lemma static_eval_state_to_env_let_case_left: "
   (\<V>, \<C>) \<Turnstile>\<^sub>\<sigma> \<langle>LET x = CASE x\<^sub>s LEFT x\<^sub>l |> e\<^sub>l RIGHT x\<^sub>r |> e\<^sub>r in e; \<rho>; \<kappa>\<rangle> \<Longrightarrow> 
-  \<rho> x\<^sub>s = Some \<lbrace>prim.Left x\<^sub>l', \<rho>\<^sub>l\<rbrace> \<Longrightarrow> \<rho>\<^sub>l x\<^sub>l' = Some \<omega>\<^sub>l \<Longrightarrow> 
+  \<rho> x\<^sub>s = Some (VClosure (Left x\<^sub>l') \<rho>\<^sub>l) \<Longrightarrow> \<rho>\<^sub>l x\<^sub>l' = Some \<omega>\<^sub>l \<Longrightarrow> 
   (\<V>, \<C>) \<Turnstile>\<^sub>\<rho> \<rho>(x\<^sub>l \<mapsto> \<omega>\<^sub>l)
 "
 
 proof
-  assume "\<rho> x\<^sub>s = Some \<lbrace>prim.Left x\<^sub>l', \<rho>\<^sub>l\<rbrace>" "\<rho>\<^sub>l x\<^sub>l' = Some \<omega>\<^sub>l"
+  assume "\<rho> x\<^sub>s = Some (VClosure (Left x\<^sub>l') \<rho>\<^sub>l)" "\<rho>\<^sub>l x\<^sub>l' = Some \<omega>\<^sub>l"
   assume "(\<V>, \<C>) \<Turnstile>\<^sub>\<sigma> \<langle>LET x = CASE x\<^sub>s LEFT x\<^sub>l |> e\<^sub>l RIGHT x\<^sub>r |> e\<^sub>r in e; \<rho>; \<kappa>\<rangle>" then 
   have "(\<V>, \<C>) \<Turnstile>\<^sub>e LET x = CASE x\<^sub>s LEFT x\<^sub>l |> e\<^sub>l RIGHT x\<^sub>r |> e\<^sub>r in e" "(\<V>, \<C>) \<Turnstile>\<^sub>\<rho> \<rho>" by (simp add: static_eval_state.simps)+
 
-  from `(\<V>, \<C>) \<Turnstile>\<^sub>\<rho> \<rho>` `\<rho> x\<^sub>s = Some \<lbrace>prim.Left x\<^sub>l', \<rho>\<^sub>l\<rbrace>`
-  have "(\<V>, \<C>) \<Turnstile>\<^sub>\<omega> \<lbrace>prim.Left x\<^sub>l', \<rho>\<^sub>l\<rbrace>" by (blast intro: static_eval_env.cases) then
+  from `(\<V>, \<C>) \<Turnstile>\<^sub>\<rho> \<rho>` `\<rho> x\<^sub>s = Some (VClosure (Left x\<^sub>l') \<rho>\<^sub>l)`
+  have "(\<V>, \<C>) \<Turnstile>\<^sub>\<omega> (VClosure (Left x\<^sub>l') \<rho>\<^sub>l)" by (blast intro: static_eval_env.cases) then
   have "(\<V>, \<C>) \<Turnstile>\<^sub>\<rho> \<rho>\<^sub>l" by (blast intro: static_eval_value.cases)
 
   from `(\<V>, \<C>) \<Turnstile>\<^sub>\<rho> \<rho>\<^sub>l` `\<rho>\<^sub>l x\<^sub>l' = Some \<omega>\<^sub>l`
   have "{|\<omega>\<^sub>l|} \<subseteq> \<V> x\<^sub>l'" "(\<V>, \<C>) \<Turnstile>\<^sub>\<omega> \<omega>\<^sub>l" by (blast intro: static_eval_env.cases)+
 
-  from `(\<V>, \<C>) \<Turnstile>\<^sub>\<rho> \<rho>` `\<rho> x\<^sub>s = Some \<lbrace>prim.Left x\<^sub>l', \<rho>\<^sub>l\<rbrace>`
-  have " | \<lbrace>prim.Left x\<^sub>l', \<rho>\<^sub>l\<rbrace> | \<in> \<V> x\<^sub>s" by (blast intro: static_eval_env.cases) then
+  from `(\<V>, \<C>) \<Turnstile>\<^sub>\<rho> \<rho>` `\<rho> x\<^sub>s = Some (VClosure (Left x\<^sub>l') \<rho>\<^sub>l)`
+  have " | (VClosure (Left x\<^sub>l') \<rho>\<^sub>l) | \<in> \<V> x\<^sub>s" by (blast intro: static_eval_env.cases) then
   have "^prim.Left x\<^sub>l' \<in> \<V> x\<^sub>s" by simp
 
   from  `(\<V>, \<C>) \<Turnstile>\<^sub>e LET x = CASE x\<^sub>s LEFT x\<^sub>l |> e\<^sub>l RIGHT x\<^sub>r |> e\<^sub>r in e`
@@ -432,19 +432,19 @@ qed
 
 lemma static_eval_state_to_stack_let_case_left: "
   (\<V>, \<C>) \<Turnstile>\<^sub>\<sigma> \<langle>LET x = CASE x\<^sub>s LEFT x\<^sub>l |> e\<^sub>l RIGHT x\<^sub>r |> e\<^sub>r in e; \<rho>; \<kappa>\<rangle> \<Longrightarrow>
-  \<rho> x\<^sub>s = Some \<lbrace>prim.Left x\<^sub>l', \<rho>\<^sub>l\<rbrace> \<Longrightarrow> \<rho>\<^sub>l x\<^sub>l' = Some \<omega>\<^sub>l \<Longrightarrow> 
+  \<rho> x\<^sub>s = Some (VClosure (Left x\<^sub>l') \<rho>\<^sub>l) \<Longrightarrow> \<rho>\<^sub>l x\<^sub>l' = Some \<omega>\<^sub>l \<Longrightarrow> 
   (\<V>, \<C>) \<Turnstile>\<^sub>\<kappa> \<V> (\<lfloor>e\<^sub>l\<rfloor>) \<Rrightarrow> \<langle>x,e,\<rho>\<rangle> # \<kappa>
 "
 proof
 
   assume "(\<V>, \<C>) \<Turnstile>\<^sub>\<sigma> \<langle>LET x = CASE x\<^sub>s LEFT x\<^sub>l |> e\<^sub>l RIGHT x\<^sub>r |> e\<^sub>r in e; \<rho>; \<kappa>\<rangle>"
-  assume "\<rho> x\<^sub>s = Some \<lbrace>prim.Left x\<^sub>l', \<rho>\<^sub>l\<rbrace>" "\<rho>\<^sub>l x\<^sub>l' = Some \<omega>\<^sub>l"
+  assume "\<rho> x\<^sub>s = Some (VClosure (Left x\<^sub>l') \<rho>\<^sub>l)" "\<rho>\<^sub>l x\<^sub>l' = Some \<omega>\<^sub>l"
 
   from `(\<V>, \<C>) \<Turnstile>\<^sub>\<sigma> \<langle>LET x = CASE x\<^sub>s LEFT x\<^sub>l |> e\<^sub>l RIGHT x\<^sub>r |> e\<^sub>r in e;\<rho>;\<kappa>\<rangle>`
   have "(\<V>, \<C>) \<Turnstile>\<^sub>e LET x = CASE x\<^sub>s LEFT x\<^sub>l |> e\<^sub>l RIGHT x\<^sub>r |> e\<^sub>r in e" "(\<V>, \<C>) \<Turnstile>\<^sub>\<rho> \<rho>" by (blast intro: static_eval_state.cases)+
   
-  from `(\<V>, \<C>) \<Turnstile>\<^sub>\<rho> \<rho>` `\<rho> x\<^sub>s = Some \<lbrace>prim.Left x\<^sub>l', \<rho>\<^sub>l\<rbrace>`
-  have " | \<lbrace>prim.Left x\<^sub>l', \<rho>\<^sub>l\<rbrace> | \<in> \<V> x\<^sub>s" by (blast intro: static_eval_env.cases) then
+  from `(\<V>, \<C>) \<Turnstile>\<^sub>\<rho> \<rho>` `\<rho> x\<^sub>s = Some (VClosure (Left x\<^sub>l') \<rho>\<^sub>l)`
+  have " | (VClosure (Left x\<^sub>l') \<rho>\<^sub>l) | \<in> \<V> x\<^sub>s" by (blast intro: static_eval_env.cases) then
   have "^prim.Left x\<^sub>l' \<in> \<V> x\<^sub>s" by simp
 
   from `(\<V>, \<C>) \<Turnstile>\<^sub>e LET x = CASE x\<^sub>s LEFT x\<^sub>l |> e\<^sub>l RIGHT x\<^sub>r |> e\<^sub>r in e`
@@ -470,45 +470,45 @@ qed
 
 lemma static_eval_state_to_state_let_case_left: "
   (\<V>, \<C>) \<Turnstile>\<^sub>\<sigma> \<langle>LET x = CASE x\<^sub>s LEFT x\<^sub>l |> e\<^sub>l RIGHT x\<^sub>r |> e\<^sub>r in e; \<rho>; \<kappa>\<rangle> \<Longrightarrow> 
-  \<rho> x\<^sub>s = Some \<lbrace>prim.Left x\<^sub>l', \<rho>\<^sub>l\<rbrace> \<Longrightarrow> 
+  \<rho> x\<^sub>s = Some (VClosure (Left x\<^sub>l') \<rho>\<^sub>l) \<Longrightarrow> 
   \<rho>\<^sub>l x\<^sub>l' = Some \<omega>\<^sub>l \<Longrightarrow> 
   (\<V>, \<C>) \<Turnstile>\<^sub>\<sigma> \<langle>e\<^sub>l; \<rho>(x\<^sub>l \<mapsto> \<omega>\<^sub>l); \<langle>x,e,\<rho>\<rangle> # \<kappa>\<rangle>
 "
 proof
-  assume "(\<V>, \<C>) \<Turnstile>\<^sub>\<sigma> \<langle>LET x = CASE x\<^sub>s LEFT x\<^sub>l |> e\<^sub>l RIGHT x\<^sub>r |> e\<^sub>r in e; \<rho>; \<kappa>\<rangle>" and "\<rho> x\<^sub>s = Some \<lbrace>prim.Left x\<^sub>l', \<rho>\<^sub>l\<rbrace>" then
+  assume "(\<V>, \<C>) \<Turnstile>\<^sub>\<sigma> \<langle>LET x = CASE x\<^sub>s LEFT x\<^sub>l |> e\<^sub>l RIGHT x\<^sub>r |> e\<^sub>r in e; \<rho>; \<kappa>\<rangle>" and "\<rho> x\<^sub>s = Some (VClosure (Left x\<^sub>l') \<rho>\<^sub>l)" then
   show "(\<V>, \<C>) \<Turnstile>\<^sub>e e\<^sub>l" by (simp add: static_eval_state_to_exp_let_case_left)
 
   assume "\<rho>\<^sub>l x\<^sub>l' = Some \<omega>\<^sub>l"
-  with `(\<V>, \<C>) \<Turnstile>\<^sub>\<sigma> \<langle>LET x = CASE x\<^sub>s LEFT x\<^sub>l |> e\<^sub>l RIGHT x\<^sub>r |> e\<^sub>r in e; \<rho>; \<kappa>\<rangle>` and `\<rho> x\<^sub>s = Some \<lbrace>prim.Left x\<^sub>l', \<rho>\<^sub>l\<rbrace>` 
+  with `(\<V>, \<C>) \<Turnstile>\<^sub>\<sigma> \<langle>LET x = CASE x\<^sub>s LEFT x\<^sub>l |> e\<^sub>l RIGHT x\<^sub>r |> e\<^sub>r in e; \<rho>; \<kappa>\<rangle>` and `\<rho> x\<^sub>s = Some (VClosure (Left x\<^sub>l') \<rho>\<^sub>l)` 
   show "(\<V>, \<C>) \<Turnstile>\<^sub>\<rho> \<rho>(x\<^sub>l \<mapsto> \<omega>\<^sub>l)" by (simp add: static_eval_state_to_env_let_case_left)
 
   from `\<rho>\<^sub>l x\<^sub>l' = Some \<omega>\<^sub>l`  
   and `(\<V>, \<C>) \<Turnstile>\<^sub>\<sigma> \<langle>LET x = CASE x\<^sub>s LEFT x\<^sub>l |> e\<^sub>l RIGHT x\<^sub>r |> e\<^sub>r in e; \<rho>; \<kappa>\<rangle>` 
-  and `\<rho> x\<^sub>s = Some \<lbrace>prim.Left x\<^sub>l', \<rho>\<^sub>l\<rbrace>` 
+  and `\<rho> x\<^sub>s = Some (VClosure (Left x\<^sub>l') \<rho>\<^sub>l)` 
   show "(\<V>, \<C>) \<Turnstile>\<^sub>\<kappa> \<V> (\<lfloor>e\<^sub>l\<rfloor>) \<Rrightarrow> \<langle>x,e,\<rho>\<rangle> # \<kappa>" by (simp add: static_eval_state_to_stack_let_case_left)
 qed
 
 
 lemma static_eval_state_to_env_let_case_right: "
   (\<V>, \<C>) \<Turnstile>\<^sub>\<sigma> \<langle>LET x = CASE x\<^sub>s LEFT x\<^sub>l |> e\<^sub>l RIGHT x\<^sub>r |> e\<^sub>r in e; \<rho>; \<kappa>\<rangle> \<Longrightarrow> 
-  \<rho> x\<^sub>s = Some \<lbrace>prim.Right x\<^sub>r', \<rho>\<^sub>r\<rbrace> \<Longrightarrow> \<rho>\<^sub>r x\<^sub>r' = Some \<omega>\<^sub>r \<Longrightarrow> 
+  \<rho> x\<^sub>s = Some (VClosure (Right x\<^sub>r') \<rho>\<^sub>r) \<Longrightarrow> \<rho>\<^sub>r x\<^sub>r' = Some \<omega>\<^sub>r \<Longrightarrow> 
   (\<V>, \<C>) \<Turnstile>\<^sub>\<rho> \<rho>(x\<^sub>r \<mapsto> \<omega>\<^sub>r)
 "
 
 proof
-  assume "\<rho> x\<^sub>s = Some \<lbrace>prim.Right x\<^sub>r', \<rho>\<^sub>r\<rbrace>" "\<rho>\<^sub>r x\<^sub>r' = Some \<omega>\<^sub>r"
+  assume "\<rho> x\<^sub>s = Some (VClosure (Right x\<^sub>r') \<rho>\<^sub>r)" "\<rho>\<^sub>r x\<^sub>r' = Some \<omega>\<^sub>r"
   assume "(\<V>, \<C>) \<Turnstile>\<^sub>\<sigma> \<langle>LET x = CASE x\<^sub>s LEFT x\<^sub>l |> e\<^sub>l RIGHT x\<^sub>r |> e\<^sub>r in e; \<rho>; \<kappa>\<rangle>" then 
   have "(\<V>, \<C>) \<Turnstile>\<^sub>e LET x = CASE x\<^sub>s LEFT x\<^sub>l |> e\<^sub>l RIGHT x\<^sub>r |> e\<^sub>r in e" "(\<V>, \<C>) \<Turnstile>\<^sub>\<rho> \<rho>" by (simp add: static_eval_state.simps)+
 
-  from `(\<V>, \<C>) \<Turnstile>\<^sub>\<rho> \<rho>` `\<rho> x\<^sub>s = Some \<lbrace>prim.Right x\<^sub>r', \<rho>\<^sub>r\<rbrace>`
-  have "(\<V>, \<C>) \<Turnstile>\<^sub>\<omega> \<lbrace>prim.Right x\<^sub>r', \<rho>\<^sub>r\<rbrace>" by (blast intro: static_eval_env.cases) then
+  from `(\<V>, \<C>) \<Turnstile>\<^sub>\<rho> \<rho>` `\<rho> x\<^sub>s = Some (VClosure (Right x\<^sub>r') \<rho>\<^sub>r)`
+  have "(\<V>, \<C>) \<Turnstile>\<^sub>\<omega> (VClosure (Right x\<^sub>r') \<rho>\<^sub>r)" by (blast intro: static_eval_env.cases) then
   have "(\<V>, \<C>) \<Turnstile>\<^sub>\<rho> \<rho>\<^sub>r" by (blast intro: static_eval_value.cases)
 
   from `(\<V>, \<C>) \<Turnstile>\<^sub>\<rho> \<rho>\<^sub>r` `\<rho>\<^sub>r x\<^sub>r' = Some \<omega>\<^sub>r`
   have "{|\<omega>\<^sub>r|} \<subseteq> \<V> x\<^sub>r'" "(\<V>, \<C>) \<Turnstile>\<^sub>\<omega> \<omega>\<^sub>r" by (blast intro: static_eval_env.cases)+
 
-  from `(\<V>, \<C>) \<Turnstile>\<^sub>\<rho> \<rho>` `\<rho> x\<^sub>s = Some \<lbrace>prim.Right x\<^sub>r', \<rho>\<^sub>r\<rbrace>`
-  have " | \<lbrace>prim.Right x\<^sub>r', \<rho>\<^sub>r\<rbrace> | \<in> \<V> x\<^sub>s" by (blast intro: static_eval_env.cases) then
+  from `(\<V>, \<C>) \<Turnstile>\<^sub>\<rho> \<rho>` `\<rho> x\<^sub>s = Some (VClosure (Right x\<^sub>r') \<rho>\<^sub>r)`
+  have " | (VClosure (Right x\<^sub>r') \<rho>\<^sub>r) | \<in> \<V> x\<^sub>s" by (blast intro: static_eval_env.cases) then
   have "^prim.Right x\<^sub>r' \<in> \<V> x\<^sub>s" by simp
 
   from  `(\<V>, \<C>) \<Turnstile>\<^sub>e LET x = CASE x\<^sub>s LEFT x\<^sub>l |> e\<^sub>l RIGHT x\<^sub>r |> e\<^sub>r in e`
@@ -537,19 +537,19 @@ qed
 
 lemma static_eval_state_to_stack_let_case_right: "
   (\<V>, \<C>) \<Turnstile>\<^sub>\<sigma>  \<langle>LET x = CASE x\<^sub>s LEFT x\<^sub>l |> e\<^sub>l RIGHT x\<^sub>r |> e\<^sub>r in e; \<rho>; \<kappa>\<rangle> \<Longrightarrow>
-  \<rho> x\<^sub>s = Some \<lbrace>prim.Right x\<^sub>r', \<rho>\<^sub>r\<rbrace> \<Longrightarrow> \<rho>\<^sub>r x\<^sub>r' = Some \<omega>\<^sub>r \<Longrightarrow> 
+  \<rho> x\<^sub>s = Some (VClosure (Right x\<^sub>r') \<rho>\<^sub>r) \<Longrightarrow> \<rho>\<^sub>r x\<^sub>r' = Some \<omega>\<^sub>r \<Longrightarrow> 
   (\<V>, \<C>) \<Turnstile>\<^sub>\<kappa>  \<V> (\<lfloor>e\<^sub>r\<rfloor>) \<Rrightarrow> \<langle>x,e,\<rho>\<rangle> # \<kappa>
 "
 proof
 
   assume "(\<V>, \<C>) \<Turnstile>\<^sub>\<sigma> \<langle>LET x = CASE x\<^sub>s LEFT x\<^sub>l |> e\<^sub>l RIGHT x\<^sub>r |> e\<^sub>r in e; \<rho>; \<kappa>\<rangle>"
-  assume "\<rho> x\<^sub>s = Some \<lbrace>prim.Right x\<^sub>r', \<rho>\<^sub>r\<rbrace>" "\<rho>\<^sub>r x\<^sub>r' = Some \<omega>\<^sub>r"
+  assume "\<rho> x\<^sub>s = Some (VClosure (Right x\<^sub>r') \<rho>\<^sub>r)" "\<rho>\<^sub>r x\<^sub>r' = Some \<omega>\<^sub>r"
 
   from `(\<V>, \<C>) \<Turnstile>\<^sub>\<sigma> \<langle>LET x = CASE x\<^sub>s LEFT x\<^sub>l |> e\<^sub>l RIGHT x\<^sub>r |> e\<^sub>r in e;\<rho>;\<kappa>\<rangle>`
   have "(\<V>, \<C>) \<Turnstile>\<^sub>e LET x = CASE x\<^sub>s LEFT x\<^sub>l |> e\<^sub>l RIGHT x\<^sub>r |> e\<^sub>r in e" "(\<V>, \<C>) \<Turnstile>\<^sub>\<rho> \<rho>" by (blast intro: static_eval_state.cases)+
   
-  from `(\<V>, \<C>) \<Turnstile>\<^sub>\<rho> \<rho>` `\<rho> x\<^sub>s = Some \<lbrace>prim.Right x\<^sub>r', \<rho>\<^sub>r\<rbrace>`
-  have " | \<lbrace>prim.Right x\<^sub>r', \<rho>\<^sub>r\<rbrace> | \<in> \<V> x\<^sub>s" by (blast intro: static_eval_env.cases) then
+  from `(\<V>, \<C>) \<Turnstile>\<^sub>\<rho> \<rho>` `\<rho> x\<^sub>s = Some (VClosure (Right x\<^sub>r') \<rho>\<^sub>r)`
+  have " | (VClosure (Right x\<^sub>r') \<rho>\<^sub>r) | \<in> \<V> x\<^sub>s" by (blast intro: static_eval_env.cases) then
   have "^prim.Right x\<^sub>r' \<in> \<V> x\<^sub>s" by simp
 
   from `(\<V>, \<C>) \<Turnstile>\<^sub>e LET x = CASE x\<^sub>s LEFT x\<^sub>l |> e\<^sub>l RIGHT x\<^sub>r |> e\<^sub>r in e`
@@ -574,45 +574,45 @@ qed
 
 lemma static_eval_state_to_state_let_case_right: "
   (\<V>, \<C>) \<Turnstile>\<^sub>\<sigma> \<langle>LET x = CASE x\<^sub>s LEFT x\<^sub>l |> e\<^sub>l RIGHT x\<^sub>r |> e\<^sub>r in e; \<rho>; \<kappa>\<rangle> \<Longrightarrow> 
-  \<rho> x\<^sub>s = Some \<lbrace>prim.Right x\<^sub>r', \<rho>\<^sub>r\<rbrace> \<Longrightarrow> 
+  \<rho> x\<^sub>s = Some (VClosure (Right x\<^sub>r') \<rho>\<^sub>r) \<Longrightarrow> 
   \<rho>\<^sub>r x\<^sub>r' = Some \<omega>\<^sub>r \<Longrightarrow> (\<V>, \<C>) \<Turnstile>\<^sub>\<sigma> \<langle>e\<^sub>r; \<rho>(x\<^sub>r \<mapsto> \<omega>\<^sub>r); \<langle>x,e,\<rho>\<rangle> # \<kappa>\<rangle>
 "
 proof
-  assume "(\<V>, \<C>) \<Turnstile>\<^sub>\<sigma> \<langle>LET x = CASE x\<^sub>s LEFT x\<^sub>l |> e\<^sub>l RIGHT x\<^sub>r |> e\<^sub>r in e; \<rho>; \<kappa>\<rangle>" and "\<rho> x\<^sub>s = Some \<lbrace>prim.Right x\<^sub>r', \<rho>\<^sub>r\<rbrace>" then
+  assume "(\<V>, \<C>) \<Turnstile>\<^sub>\<sigma> \<langle>LET x = CASE x\<^sub>s LEFT x\<^sub>l |> e\<^sub>l RIGHT x\<^sub>r |> e\<^sub>r in e; \<rho>; \<kappa>\<rangle>" and "\<rho> x\<^sub>s = Some (VClosure (Right x\<^sub>r') \<rho>\<^sub>r)" then
   show "(\<V>, \<C>) \<Turnstile>\<^sub>e e\<^sub>r" by (simp add: static_eval_state_to_exp_let_case_right)
 
   assume "\<rho>\<^sub>r x\<^sub>r' = Some \<omega>\<^sub>r"
-  with `(\<V>, \<C>) \<Turnstile>\<^sub>\<sigma> \<langle>LET x = CASE x\<^sub>s LEFT x\<^sub>l |> e\<^sub>l RIGHT x\<^sub>r |> e\<^sub>r in e; \<rho>; \<kappa>\<rangle>` and `\<rho> x\<^sub>s = Some \<lbrace>prim.Right x\<^sub>r', \<rho>\<^sub>r\<rbrace>` 
+  with `(\<V>, \<C>) \<Turnstile>\<^sub>\<sigma> \<langle>LET x = CASE x\<^sub>s LEFT x\<^sub>l |> e\<^sub>l RIGHT x\<^sub>r |> e\<^sub>r in e; \<rho>; \<kappa>\<rangle>` and `\<rho> x\<^sub>s = Some (VClosure (Right x\<^sub>r') \<rho>\<^sub>r)` 
   show "(\<V>, \<C>) \<Turnstile>\<^sub>\<rho> \<rho>(x\<^sub>r \<mapsto> \<omega>\<^sub>r)" by (simp add: static_eval_state_to_env_let_case_right)
 
   from `\<rho>\<^sub>r x\<^sub>r' = Some \<omega>\<^sub>r`  
   and `(\<V>, \<C>) \<Turnstile>\<^sub>\<sigma> \<langle>LET x = CASE x\<^sub>s LEFT x\<^sub>l |> e\<^sub>l RIGHT x\<^sub>r |> e\<^sub>r in e; \<rho>; \<kappa>\<rangle>` 
-  and `\<rho> x\<^sub>s = Some \<lbrace>prim.Right x\<^sub>r', \<rho>\<^sub>r\<rbrace>` 
+  and `\<rho> x\<^sub>s = Some (VClosure (Right x\<^sub>r') \<rho>\<^sub>r)` 
   show "(\<V>, \<C>) \<Turnstile>\<^sub>\<kappa> \<V> (\<lfloor>e\<^sub>r\<rfloor>) \<Rrightarrow> \<langle>x,e,\<rho>\<rangle> # \<kappa>" by (simp add: static_eval_state_to_stack_let_case_right)
 qed
 
 
 lemma static_eval_state_to_env_let_fst: "
   (\<V>, \<C>) \<Turnstile>\<^sub>\<sigma> \<langle>LET x = FST x\<^sub>p in e; \<rho>; \<kappa>\<rangle> \<Longrightarrow> 
-  \<rho> x\<^sub>p = Some \<lbrace>prim.Pair x\<^sub>1 x\<^sub>2, \<rho>\<^sub>p\<rbrace> \<Longrightarrow> \<rho>\<^sub>p x\<^sub>1 = Some \<omega> \<Longrightarrow> 
+  \<rho> x\<^sub>p = Some (VClosure (Pair x\<^sub>1 x\<^sub>2) \<rho>\<^sub>p) \<Longrightarrow> \<rho>\<^sub>p x\<^sub>1 = Some \<omega> \<Longrightarrow> 
   (\<V>, \<C>) \<Turnstile>\<^sub>\<rho> \<rho>(x \<mapsto> \<omega>)
 "
 proof
-  assume "\<rho> x\<^sub>p = Some \<lbrace>prim.Pair x\<^sub>1 x\<^sub>2, \<rho>\<^sub>p\<rbrace>" and "\<rho>\<^sub>p x\<^sub>1 = Some \<omega>"
+  assume "\<rho> x\<^sub>p = Some (VClosure (Pair x\<^sub>1 x\<^sub>2) \<rho>\<^sub>p)" and "\<rho>\<^sub>p x\<^sub>1 = Some \<omega>"
   assume "(\<V>, \<C>) \<Turnstile>\<^sub>\<sigma> \<langle>LET x = FST x\<^sub>p in e; \<rho>; \<kappa>\<rangle>" then
   have "(\<V>, \<C>) \<Turnstile>\<^sub>e LET x = FST x\<^sub>p in e" "(\<V>, \<C>) \<Turnstile>\<^sub>\<rho> \<rho>" by (simp add: static_eval_state.simps)+
 
   thm static_eval_state.simps
 
-  from `(\<V>, \<C>) \<Turnstile>\<^sub>\<rho> \<rho>` `\<rho> x\<^sub>p = Some \<lbrace>prim.Pair x\<^sub>1 x\<^sub>2, \<rho>\<^sub>p\<rbrace>`
-  have "(\<V>, \<C>) \<Turnstile>\<^sub>\<omega> \<lbrace>prim.Pair x\<^sub>1 x\<^sub>2, \<rho>\<^sub>p\<rbrace>" by (blast intro: static_eval_env.cases) then
+  from `(\<V>, \<C>) \<Turnstile>\<^sub>\<rho> \<rho>` `\<rho> x\<^sub>p = Some (VClosure (Pair x\<^sub>1 x\<^sub>2) \<rho>\<^sub>p)`
+  have "(\<V>, \<C>) \<Turnstile>\<^sub>\<omega> (VClosure (Pair x\<^sub>1 x\<^sub>2) \<rho>\<^sub>p)" by (blast intro: static_eval_env.cases) then
   have "(\<V>, \<C>) \<Turnstile>\<^sub>\<rho> \<rho>\<^sub>p" by (blast intro: static_eval_value.cases)
 
   from `(\<V>, \<C>) \<Turnstile>\<^sub>\<rho> \<rho>\<^sub>p` `\<rho>\<^sub>p x\<^sub>1 = Some \<omega>`
   have "{|\<omega>|} \<subseteq> \<V> x\<^sub>1" "(\<V>, \<C>) \<Turnstile>\<^sub>\<omega> \<omega>" by (blast intro: static_eval_env.cases)+
 
-  from `(\<V>, \<C>) \<Turnstile>\<^sub>\<rho> \<rho>` `\<rho> x\<^sub>p = Some \<lbrace>prim.Pair x\<^sub>1 x\<^sub>2, \<rho>\<^sub>p\<rbrace>`
-  have " | \<lbrace>prim.Pair x\<^sub>1 x\<^sub>2, \<rho>\<^sub>p\<rbrace> | \<in> \<V> x\<^sub>p" by (blast intro: static_eval_env.cases) then
+  from `(\<V>, \<C>) \<Turnstile>\<^sub>\<rho> \<rho>` `\<rho> x\<^sub>p = Some (VClosure (Pair x\<^sub>1 x\<^sub>2) \<rho>\<^sub>p)`
+  have " | (VClosure (Pair x\<^sub>1 x\<^sub>2) \<rho>\<^sub>p) | \<in> \<V> x\<^sub>p" by (blast intro: static_eval_env.cases) then
   have "^prim.Pair x\<^sub>1 x\<^sub>2 \<in> \<V> x\<^sub>p" by simp
 
   from  `(\<V>, \<C>) \<Turnstile>\<^sub>e LET x = FST x\<^sub>p in e`
@@ -642,40 +642,40 @@ qed
 
 lemma static_eval_state_to_state_let_fst: "
   (\<V>, \<C>) \<Turnstile>\<^sub>\<sigma> \<langle>LET x = FST x\<^sub>p in e; \<rho>; \<kappa>\<rangle> \<Longrightarrow>
-  \<rho> x\<^sub>p = Some \<lbrace>prim.Pair x\<^sub>1 x\<^sub>2, \<rho>\<^sub>p\<rbrace> \<Longrightarrow> \<rho>\<^sub>p x\<^sub>1 = Some \<omega> \<Longrightarrow> 
+  \<rho> x\<^sub>p = Some (VClosure (Pair x\<^sub>1 x\<^sub>2) \<rho>\<^sub>p) \<Longrightarrow> \<rho>\<^sub>p x\<^sub>1 = Some \<omega> \<Longrightarrow> 
   (\<V>, \<C>) \<Turnstile>\<^sub>\<sigma> \<langle>e; \<rho>(x \<mapsto> \<omega>); \<kappa>\<rangle>
 "
 proof
   assume "(\<V>, \<C>) \<Turnstile>\<^sub>\<sigma> \<langle>LET x = FST x\<^sub>p in e; \<rho>; \<kappa>\<rangle>" then
   show "(\<V>, \<C>) \<Turnstile>\<^sub>e e" by (simp add: static_eval_state_to_exp_let)
 
-  assume "\<rho> x\<^sub>p = Some \<lbrace>prim.Pair x\<^sub>1 x\<^sub>2, \<rho>\<^sub>p\<rbrace>" and "\<rho>\<^sub>p x\<^sub>1 = Some \<omega>"
+  assume "\<rho> x\<^sub>p = Some (VClosure (Pair x\<^sub>1 x\<^sub>2) \<rho>\<^sub>p)" and "\<rho>\<^sub>p x\<^sub>1 = Some \<omega>"
   with `(\<V>, \<C>) \<Turnstile>\<^sub>\<sigma> \<langle>LET x = FST x\<^sub>p in e; \<rho>; \<kappa>\<rangle>`
   show "(\<V>, \<C>) \<Turnstile>\<^sub>\<rho> \<rho>(x \<mapsto> \<omega>)"  by (simp add: static_eval_state_to_env_let_fst)
 
-  from `\<rho> x\<^sub>p = Some \<lbrace>prim.Pair x\<^sub>1 x\<^sub>2, \<rho>\<^sub>p\<rbrace>` and `\<rho>\<^sub>p x\<^sub>1 = Some \<omega>`
+  from `\<rho> x\<^sub>p = Some (VClosure (Pair x\<^sub>1 x\<^sub>2) \<rho>\<^sub>p)` and `\<rho>\<^sub>p x\<^sub>1 = Some \<omega>`
   and `(\<V>, \<C>) \<Turnstile>\<^sub>\<sigma> \<langle>LET x = FST x\<^sub>p in e; \<rho>; \<kappa>\<rangle>`
   show "(\<V>, \<C>) \<Turnstile>\<^sub>\<kappa> \<V> (\<lfloor>e\<rfloor>) \<Rrightarrow> \<kappa>" by (simp add: static_eval_state_to_stack_let)
 qed
 
 
 lemma static_eval_state_to_env_let_snd: "
-  (\<V>, \<C>) \<Turnstile>\<^sub>\<sigma> \<langle>LET x = SND x\<^sub>p in e; \<rho>; \<kappa>\<rangle> \<Longrightarrow> \<rho> x\<^sub>p = Some \<lbrace>prim.Pair x\<^sub>1 x\<^sub>2, \<rho>\<^sub>p\<rbrace> \<Longrightarrow> \<rho>\<^sub>p x\<^sub>2 = Some \<omega> \<Longrightarrow> (\<V>, \<C>) \<Turnstile>\<^sub>\<rho> \<rho>(x \<mapsto> \<omega>)
+  (\<V>, \<C>) \<Turnstile>\<^sub>\<sigma> \<langle>LET x = SND x\<^sub>p in e; \<rho>; \<kappa>\<rangle> \<Longrightarrow> \<rho> x\<^sub>p = Some (VClosure (Pair x\<^sub>1 x\<^sub>2) \<rho>\<^sub>p) \<Longrightarrow> \<rho>\<^sub>p x\<^sub>2 = Some \<omega> \<Longrightarrow> (\<V>, \<C>) \<Turnstile>\<^sub>\<rho> \<rho>(x \<mapsto> \<omega>)
 "
 proof
-  assume "\<rho> x\<^sub>p = Some \<lbrace>prim.Pair x\<^sub>1 x\<^sub>2, \<rho>\<^sub>p\<rbrace>" and "\<rho>\<^sub>p x\<^sub>2 = Some \<omega>"
+  assume "\<rho> x\<^sub>p = Some (VClosure (Pair x\<^sub>1 x\<^sub>2) \<rho>\<^sub>p)" and "\<rho>\<^sub>p x\<^sub>2 = Some \<omega>"
   assume "(\<V>, \<C>) \<Turnstile>\<^sub>\<sigma> \<langle>LET x = SND x\<^sub>p in e; \<rho>; \<kappa>\<rangle>" then
   have "(\<V>, \<C>) \<Turnstile>\<^sub>e LET x = SND x\<^sub>p in e" "(\<V>, \<C>) \<Turnstile>\<^sub>\<rho> \<rho>" by (simp add: static_eval_state.simps)+
 
-  from `(\<V>, \<C>) \<Turnstile>\<^sub>\<rho> \<rho>` `\<rho> x\<^sub>p = Some \<lbrace>prim.Pair x\<^sub>1 x\<^sub>2, \<rho>\<^sub>p\<rbrace>`
-  have "(\<V>, \<C>) \<Turnstile>\<^sub>\<omega> \<lbrace>prim.Pair x\<^sub>1 x\<^sub>2, \<rho>\<^sub>p\<rbrace>" by (blast intro: static_eval_env.cases) then
+  from `(\<V>, \<C>) \<Turnstile>\<^sub>\<rho> \<rho>` `\<rho> x\<^sub>p = Some (VClosure (Pair x\<^sub>1 x\<^sub>2) \<rho>\<^sub>p)`
+  have "(\<V>, \<C>) \<Turnstile>\<^sub>\<omega> (VClosure (Pair x\<^sub>1 x\<^sub>2) \<rho>\<^sub>p)" by (blast intro: static_eval_env.cases) then
   have "(\<V>, \<C>) \<Turnstile>\<^sub>\<rho> \<rho>\<^sub>p" by (blast intro: static_eval_value.cases)
 
   from `(\<V>, \<C>) \<Turnstile>\<^sub>\<rho> \<rho>\<^sub>p` `\<rho>\<^sub>p x\<^sub>2 = Some \<omega>`
   have "{|\<omega>|} \<subseteq> \<V> x\<^sub>2" "(\<V>, \<C>) \<Turnstile>\<^sub>\<omega> \<omega>" by (blast intro: static_eval_env.cases)+
 
-  from `(\<V>, \<C>) \<Turnstile>\<^sub>\<rho> \<rho>` `\<rho> x\<^sub>p = Some \<lbrace>prim.Pair x\<^sub>1 x\<^sub>2, \<rho>\<^sub>p\<rbrace>`
-  have " | \<lbrace>prim.Pair x\<^sub>1 x\<^sub>2, \<rho>\<^sub>p\<rbrace> | \<in> \<V> x\<^sub>p" by (blast intro: static_eval_env.cases) then
+  from `(\<V>, \<C>) \<Turnstile>\<^sub>\<rho> \<rho>` `\<rho> x\<^sub>p = Some (VClosure (Pair x\<^sub>1 x\<^sub>2) \<rho>\<^sub>p)`
+  have " | (VClosure (Pair x\<^sub>1 x\<^sub>2) \<rho>\<^sub>p) | \<in> \<V> x\<^sub>p" by (blast intro: static_eval_env.cases) then
   have "^prim.Pair x\<^sub>1 x\<^sub>2 \<in> \<V> x\<^sub>p" by simp
 
   from  `(\<V>, \<C>) \<Turnstile>\<^sub>e LET x = SND x\<^sub>p in e`
@@ -705,18 +705,18 @@ qed
 
 lemma static_eval_state_to_state_let_snd: "
   (\<V>, \<C>) \<Turnstile>\<^sub>\<sigma> \<langle>LET x = SND x\<^sub>p in e; \<rho>; \<kappa>\<rangle> \<Longrightarrow>
-  \<rho> x\<^sub>p = Some \<lbrace>prim.Pair x\<^sub>1 x\<^sub>2, \<rho>\<^sub>p\<rbrace> \<Longrightarrow> \<rho>\<^sub>p x\<^sub>2 = Some \<omega> \<Longrightarrow> 
+  \<rho> x\<^sub>p = Some (VClosure (Pair x\<^sub>1 x\<^sub>2) \<rho>\<^sub>p) \<Longrightarrow> \<rho>\<^sub>p x\<^sub>2 = Some \<omega> \<Longrightarrow> 
   (\<V>, \<C>) \<Turnstile>\<^sub>\<sigma> \<langle>e; \<rho>(x \<mapsto> \<omega>); \<kappa>\<rangle>
 "
 proof
   assume "(\<V>, \<C>) \<Turnstile>\<^sub>\<sigma> \<langle>LET x = SND x\<^sub>p in e; \<rho>; \<kappa>\<rangle>" then
   show "(\<V>, \<C>) \<Turnstile>\<^sub>e e" by (simp add: static_eval_state_to_exp_let)
 
-  assume "\<rho> x\<^sub>p = Some \<lbrace>prim.Pair x\<^sub>1 x\<^sub>2, \<rho>\<^sub>p\<rbrace>" and "\<rho>\<^sub>p x\<^sub>2 = Some \<omega>"
+  assume "\<rho> x\<^sub>p = Some (VClosure (Pair x\<^sub>1 x\<^sub>2) \<rho>\<^sub>p)" and "\<rho>\<^sub>p x\<^sub>2 = Some \<omega>"
   with `(\<V>, \<C>) \<Turnstile>\<^sub>\<sigma> \<langle>LET x = SND x\<^sub>p in e; \<rho>; \<kappa>\<rangle>`
   show "(\<V>, \<C>) \<Turnstile>\<^sub>\<rho> \<rho>(x \<mapsto> \<omega>)" by (simp add: static_eval_state_to_env_let_snd)
 
-  from `\<rho> x\<^sub>p = Some \<lbrace>prim.Pair x\<^sub>1 x\<^sub>2, \<rho>\<^sub>p\<rbrace>` and `\<rho>\<^sub>p x\<^sub>2 = Some \<omega>`
+  from `\<rho> x\<^sub>p = Some (VClosure (Pair x\<^sub>1 x\<^sub>2) \<rho>\<^sub>p)` and `\<rho>\<^sub>p x\<^sub>2 = Some \<omega>`
   and `(\<V>, \<C>) \<Turnstile>\<^sub>\<sigma> \<langle>LET x = SND x\<^sub>p in e; \<rho>; \<kappa>\<rangle>`
   show "(\<V>, \<C>) \<Turnstile>\<^sub>\<kappa> \<V> (\<lfloor>e\<rfloor>) \<Rrightarrow> \<kappa>" by (simp add: static_eval_state_to_stack_let)
 qed
@@ -724,25 +724,25 @@ qed
 
 lemma static_eval_state_to_env_let_app: "
   (\<V>, \<C>) \<Turnstile>\<^sub>\<sigma> \<langle>LET x = APP f x\<^sub>a in e; \<rho>; \<kappa>\<rangle> \<Longrightarrow> 
-  \<rho> f = Some \<lbrace>Abs f\<^sub>l x\<^sub>l e\<^sub>l, \<rho>\<^sub>l\<rbrace> \<Longrightarrow> \<rho> x\<^sub>a = Some \<omega>\<^sub>a \<Longrightarrow> 
-  (\<V>, \<C>) \<Turnstile>\<^sub>\<rho> \<rho>\<^sub>l(f\<^sub>l \<mapsto> \<lbrace>Abs f\<^sub>l x\<^sub>l e\<^sub>l, \<rho>\<^sub>l\<rbrace>, x\<^sub>l \<mapsto> \<omega>\<^sub>a)
+  \<rho> f = Some (VClosure (Abs f\<^sub>l x\<^sub>l e\<^sub>l) \<rho>\<^sub>l) \<Longrightarrow> \<rho> x\<^sub>a = Some \<omega>\<^sub>a \<Longrightarrow> 
+  (\<V>, \<C>) \<Turnstile>\<^sub>\<rho> \<rho>\<^sub>l(f\<^sub>l \<mapsto> (VClosure (Abs f\<^sub>l x\<^sub>l e\<^sub>l) \<rho>\<^sub>l), x\<^sub>l \<mapsto> \<omega>\<^sub>a)
 "
 proof
-  assume "\<rho> f = Some \<lbrace>Abs f\<^sub>l x\<^sub>l e\<^sub>l, \<rho>\<^sub>l\<rbrace>" "\<rho> x\<^sub>a = Some \<omega>\<^sub>a"
+  assume "\<rho> f = Some (VClosure (Abs f\<^sub>l x\<^sub>l e\<^sub>l) \<rho>\<^sub>l)" "\<rho> x\<^sub>a = Some \<omega>\<^sub>a"
   assume "(\<V>, \<C>) \<Turnstile>\<^sub>\<sigma> \<langle>LET x = APP f x\<^sub>a in e; \<rho>; \<kappa>\<rangle>" then
   have "(\<V>, \<C>) \<Turnstile>\<^sub>e LET x = APP f x\<^sub>a in e" "(\<V>, \<C>) \<Turnstile>\<^sub>\<rho> \<rho>" by (simp add: static_eval_state.simps)+
 
   from `(\<V>, \<C>) \<Turnstile>\<^sub>\<rho> \<rho>` and `\<rho> x\<^sub>a = Some \<omega>\<^sub>a`
   have "{|\<omega>\<^sub>a|} \<subseteq> \<V> x\<^sub>a" "(\<V>, \<C>) \<Turnstile>\<^sub>\<omega> \<omega>\<^sub>a" by (blast intro: static_eval_env.cases)+
 
-  from `(\<V>, \<C>) \<Turnstile>\<^sub>\<rho> \<rho>` and `\<rho> f = Some \<lbrace>Abs f\<^sub>l x\<^sub>l e\<^sub>l, \<rho>\<^sub>l\<rbrace>`
-  have "{|\<lbrace>Abs f\<^sub>l x\<^sub>l e\<^sub>l, \<rho>\<^sub>l\<rbrace>|} \<subseteq> \<V> f" "(\<V>, \<C>) \<Turnstile>\<^sub>\<omega> \<lbrace>Abs f\<^sub>l x\<^sub>l e\<^sub>l, \<rho>\<^sub>l\<rbrace>" by (blast intro: static_eval_env.cases)+
+  from `(\<V>, \<C>) \<Turnstile>\<^sub>\<rho> \<rho>` and `\<rho> f = Some (VClosure (Abs f\<^sub>l x\<^sub>l e\<^sub>l) \<rho>\<^sub>l)`
+  have "{|(VClosure (Abs f\<^sub>l x\<^sub>l e\<^sub>l) \<rho>\<^sub>l)|} \<subseteq> \<V> f" "(\<V>, \<C>) \<Turnstile>\<^sub>\<omega> (VClosure (Abs f\<^sub>l x\<^sub>l e\<^sub>l) \<rho>\<^sub>l)" by (blast intro: static_eval_env.cases)+
 
-  from `{|\<lbrace>Abs f\<^sub>l x\<^sub>l e\<^sub>l, \<rho>\<^sub>l\<rbrace>|} \<subseteq> \<V> f`
+  from `{|(VClosure (Abs f\<^sub>l x\<^sub>l e\<^sub>l) \<rho>\<^sub>l)|} \<subseteq> \<V> f`
   have "^Abs f\<^sub>l x\<^sub>l e\<^sub>l \<in> \<V> f" by simp
 
-  from `(\<V>, \<C>) \<Turnstile>\<^sub>\<omega> \<lbrace>Abs f\<^sub>l x\<^sub>l e\<^sub>l, \<rho>\<^sub>l\<rbrace>`
-  have "{|\<lbrace>Abs f\<^sub>l x\<^sub>l e\<^sub>l, \<rho>\<^sub>l\<rbrace>|} \<subseteq> \<V> f\<^sub>l" "(\<V>, \<C>) \<Turnstile>\<^sub>\<rho> \<rho>\<^sub>l" by (rule static_eval_value.cases; auto)+
+  from `(\<V>, \<C>) \<Turnstile>\<^sub>\<omega> (VClosure (Abs f\<^sub>l x\<^sub>l e\<^sub>l) \<rho>\<^sub>l)`
+  have "{|(VClosure (Abs f\<^sub>l x\<^sub>l e\<^sub>l) \<rho>\<^sub>l)|} \<subseteq> \<V> f\<^sub>l" "(\<V>, \<C>) \<Turnstile>\<^sub>\<rho> \<rho>\<^sub>l" by (rule static_eval_value.cases; auto)+
 
 
   with `(\<V>, \<C>) \<Turnstile>\<^sub>e LET x = APP f x\<^sub>a in e`
@@ -760,28 +760,28 @@ proof
 
   {
     fix x' \<omega>'
-    assume "(\<rho>\<^sub>l(f\<^sub>l \<mapsto> \<lbrace>Abs f\<^sub>l x\<^sub>l e\<^sub>l, \<rho>\<^sub>l\<rbrace>, x\<^sub>l \<mapsto> \<omega>\<^sub>a)) x' = Some \<omega>'" "x' \<noteq> x\<^sub>l" "x' \<noteq> f\<^sub>l" then
+    assume "(\<rho>\<^sub>l(f\<^sub>l \<mapsto> (VClosure (Abs f\<^sub>l x\<^sub>l e\<^sub>l) \<rho>\<^sub>l), x\<^sub>l \<mapsto> \<omega>\<^sub>a)) x' = Some \<omega>'" "x' \<noteq> x\<^sub>l" "x' \<noteq> f\<^sub>l" then
     have "\<rho>\<^sub>l x' = Some \<omega>'" by simp
     with `(\<V>, \<C>) \<Turnstile>\<^sub>\<rho> \<rho>\<^sub>l` 
     have "{|\<omega>'|} \<subseteq> \<V> x' \<and> (\<V>, \<C>) \<Turnstile>\<^sub>\<omega> \<omega>'" by (simp add: static_eval_env.simps)
   }
-  with \<open>{|\<lbrace>Abs f\<^sub>l x\<^sub>l e\<^sub>l, \<rho>\<^sub>l\<rbrace>|} \<subseteq> \<V> f\<^sub>l\<close> \<open>(\<V>, \<C>) \<Turnstile>\<^sub>\<omega> \<lbrace>Abs f\<^sub>l x\<^sub>l e\<^sub>l, \<rho>\<^sub>l\<rbrace>\<close> \<open>(\<V>, \<C>) \<Turnstile>\<^sub>\<omega> \<omega>\<^sub>a\<close> \<open>{|\<omega>\<^sub>a|} \<subseteq> \<V> x\<^sub>l\<close>
-  show "\<forall>x \<omega>. (\<rho>\<^sub>l(f\<^sub>l \<mapsto> \<lbrace>Abs f\<^sub>l x\<^sub>l e\<^sub>l, \<rho>\<^sub>l\<rbrace>, x\<^sub>l \<mapsto> \<omega>\<^sub>a)) x = Some \<omega> \<longrightarrow> {|\<omega>|} \<subseteq> \<V> x \<and> (\<V>, \<C>) \<Turnstile>\<^sub>\<omega> \<omega>" by auto
+  with \<open>{|(VClosure (Abs f\<^sub>l x\<^sub>l e\<^sub>l) \<rho>\<^sub>l)|} \<subseteq> \<V> f\<^sub>l\<close> \<open>(\<V>, \<C>) \<Turnstile>\<^sub>\<omega> (VClosure (Abs f\<^sub>l x\<^sub>l e\<^sub>l) \<rho>\<^sub>l)\<close> \<open>(\<V>, \<C>) \<Turnstile>\<^sub>\<omega> \<omega>\<^sub>a\<close> \<open>{|\<omega>\<^sub>a|} \<subseteq> \<V> x\<^sub>l\<close>
+  show "\<forall>x \<omega>. (\<rho>\<^sub>l(f\<^sub>l \<mapsto> (VClosure (Abs f\<^sub>l x\<^sub>l e\<^sub>l) \<rho>\<^sub>l), x\<^sub>l \<mapsto> \<omega>\<^sub>a)) x = Some \<omega> \<longrightarrow> {|\<omega>|} \<subseteq> \<V> x \<and> (\<V>, \<C>) \<Turnstile>\<^sub>\<omega> \<omega>" by auto
 
 qed
 
 lemma static_eval_state_to_stack_let_app: "
   (\<V>, \<C>) \<Turnstile>\<^sub>\<sigma> \<langle>LET x = APP f x\<^sub>a in e; \<rho>; \<kappa>\<rangle> \<Longrightarrow> 
-  \<rho> f = Some \<lbrace>Abs f' x\<^sub>p e\<^sub>b, \<rho>'\<rbrace> \<Longrightarrow> \<rho> x\<^sub>a = Some \<omega>\<^sub>a \<Longrightarrow> 
+  \<rho> f = Some (VClosure (Abs f' x\<^sub>p e\<^sub>b) \<rho>') \<Longrightarrow> \<rho> x\<^sub>a = Some \<omega>\<^sub>a \<Longrightarrow> 
   (\<V>, \<C>) \<Turnstile>\<^sub>\<kappa> \<V> (\<lfloor>e\<^sub>b\<rfloor>) \<Rrightarrow> \<langle>x,e,\<rho>\<rangle> # \<kappa>
 "
 proof
-  assume "\<rho> f = Some \<lbrace>Abs f' x\<^sub>p e\<^sub>b, \<rho>'\<rbrace>" and "\<rho> x\<^sub>a = Some \<omega>\<^sub>a"
+  assume "\<rho> f = Some (VClosure (Abs f' x\<^sub>p e\<^sub>b) \<rho>')" and "\<rho> x\<^sub>a = Some \<omega>\<^sub>a"
   assume "(\<V>, \<C>) \<Turnstile>\<^sub>\<sigma> \<langle>LET x = APP f x\<^sub>a in e; \<rho>; \<kappa>\<rangle>" then
   have "(\<V>, \<C>) \<Turnstile>\<^sub>e LET x = APP f x\<^sub>a in e"  "(\<V>, \<C>) \<Turnstile>\<^sub>\<rho> \<rho>" by (blast intro: static_eval_state.cases)+
 
-  from `(\<V>, \<C>) \<Turnstile>\<^sub>\<rho> \<rho>` and `\<rho> f = Some \<lbrace>Abs f' x\<^sub>p e\<^sub>b, \<rho>'\<rbrace>`
-  have " {|\<lbrace>Abs f' x\<^sub>p e\<^sub>b, \<rho>'\<rbrace>|} \<subseteq> \<V> f" by (blast intro: static_eval_env.cases) then
+  from `(\<V>, \<C>) \<Turnstile>\<^sub>\<rho> \<rho>` and `\<rho> f = Some (VClosure (Abs f' x\<^sub>p e\<^sub>b) \<rho>')`
+  have " {|(VClosure (Abs f' x\<^sub>p e\<^sub>b) \<rho>')|} \<subseteq> \<V> f" by (blast intro: static_eval_env.cases) then
   have " ^Abs f' x\<^sub>p e\<^sub>b \<in> \<V> f" by simp
 
   from `(\<V>, \<C>) \<Turnstile>\<^sub>e LET x = APP f x\<^sub>a in e`
@@ -806,18 +806,18 @@ qed
 
 lemma static_eval_state_to_state_let_app: "
   (\<V>, \<C>) \<Turnstile>\<^sub>\<sigma> \<langle>LET x = APP f x\<^sub>a in e; \<rho>; \<kappa>\<rangle> \<Longrightarrow>
-  \<rho> f = Some \<lbrace>Abs f' x\<^sub>p e\<^sub>b, \<rho>'\<rbrace> \<Longrightarrow> \<rho> x\<^sub>a = Some \<omega>\<^sub>a \<Longrightarrow> 
-  (\<V>, \<C>) \<Turnstile>\<^sub>\<sigma> \<langle>e\<^sub>b; \<rho>'(f' \<mapsto> \<lbrace>Abs f' x\<^sub>p e\<^sub>b, \<rho>'\<rbrace>, x\<^sub>p \<mapsto> \<omega>\<^sub>a); \<langle>x,e,\<rho>\<rangle> # \<kappa>\<rangle>
+  \<rho> f = Some (VClosure (Abs f' x\<^sub>p e\<^sub>b) \<rho>') \<Longrightarrow> \<rho> x\<^sub>a = Some \<omega>\<^sub>a \<Longrightarrow> 
+  (\<V>, \<C>) \<Turnstile>\<^sub>\<sigma> \<langle>e\<^sub>b; \<rho>'(f' \<mapsto> (VClosure (Abs f' x\<^sub>p e\<^sub>b) \<rho>'), x\<^sub>p \<mapsto> \<omega>\<^sub>a); \<langle>x,e,\<rho>\<rangle> # \<kappa>\<rangle>
 "
 proof
-  assume "(\<V>, \<C>) \<Turnstile>\<^sub>\<sigma> \<langle>LET x = APP f x\<^sub>a in e; \<rho>; \<kappa>\<rangle>" and "\<rho> f = Some \<lbrace>Abs f' x\<^sub>p e\<^sub>b, \<rho>'\<rbrace>" then
+  assume "(\<V>, \<C>) \<Turnstile>\<^sub>\<sigma> \<langle>LET x = APP f x\<^sub>a in e; \<rho>; \<kappa>\<rangle>" and "\<rho> f = Some (VClosure (Abs f' x\<^sub>p e\<^sub>b) \<rho>')" then
   show "(\<V>, \<C>) \<Turnstile>\<^sub>e e\<^sub>b" by (blast intro: static_eval_state_to_exp_let_app)
 
   assume "\<rho> x\<^sub>a = Some \<omega>\<^sub>a"
-  with `(\<V>, \<C>) \<Turnstile>\<^sub>\<sigma> \<langle>LET x = APP f x\<^sub>a in e; \<rho>; \<kappa>\<rangle>` and `\<rho> f = Some \<lbrace>Abs f' x\<^sub>p e\<^sub>b, \<rho>'\<rbrace>`
-  show "(\<V>, \<C>) \<Turnstile>\<^sub>\<rho> \<rho>'(f' \<mapsto> \<lbrace>Abs f' x\<^sub>p e\<^sub>b, \<rho>'\<rbrace>, x\<^sub>p \<mapsto> \<omega>\<^sub>a)" by (blast intro: static_eval_state_to_env_let_app)
+  with `(\<V>, \<C>) \<Turnstile>\<^sub>\<sigma> \<langle>LET x = APP f x\<^sub>a in e; \<rho>; \<kappa>\<rangle>` and `\<rho> f = Some (VClosure (Abs f' x\<^sub>p e\<^sub>b) \<rho>')`
+  show "(\<V>, \<C>) \<Turnstile>\<^sub>\<rho> \<rho>'(f' \<mapsto> (VClosure (Abs f' x\<^sub>p e\<^sub>b) \<rho>'), x\<^sub>p \<mapsto> \<omega>\<^sub>a)" by (blast intro: static_eval_state_to_env_let_app)
 
-  from `\<rho> x\<^sub>a = Some \<omega>\<^sub>a` and  `(\<V>, \<C>) \<Turnstile>\<^sub>\<sigma> \<langle>LET x = APP f x\<^sub>a in e; \<rho>; \<kappa>\<rangle>` and `\<rho> f = Some \<lbrace>Abs f' x\<^sub>p e\<^sub>b, \<rho>'\<rbrace>`
+  from `\<rho> x\<^sub>a = Some \<omega>\<^sub>a` and  `(\<V>, \<C>) \<Turnstile>\<^sub>\<sigma> \<langle>LET x = APP f x\<^sub>a in e; \<rho>; \<kappa>\<rangle>` and `\<rho> f = Some (VClosure (Abs f' x\<^sub>p e\<^sub>b) \<rho>')`
   show "(\<V>, \<C>) \<Turnstile>\<^sub>\<kappa> \<V> (\<lfloor>e\<^sub>b\<rfloor>) \<Rrightarrow> \<langle>x,e,\<rho>\<rangle> # \<kappa>" by (blast intro: static_eval_state_to_stack_let_app)
 qed
 
@@ -839,49 +839,48 @@ proof -
     show "(\<V>, \<C>) \<Turnstile>\<^sub>\<sigma> \<sigma>'" by (simp add: static_eval_state_to_state_result)
   next
     case (Let_Unit x e \<rho> \<kappa>)
-    assume "\<sigma> = \<langle>LET x = \<lparr>\<rparr> in e;\<rho>;\<kappa>\<rangle>" and "\<sigma>' = \<langle>e;\<rho> ++ [x \<mapsto> \<lbrace>\<rbrace>];\<kappa>\<rangle>"
+    assume "\<sigma> = \<langle>LET x = \<lparr>\<rparr> in e;\<rho>;\<kappa>\<rangle>" and "\<sigma>' = \<langle>e;\<rho> ++ [x \<mapsto> VUnit];\<kappa>\<rangle>"
     with `(\<V>, \<C>) \<Turnstile>\<^sub>\<sigma> \<sigma>`
     show "(\<V>, \<C>) \<Turnstile>\<^sub>\<sigma> \<sigma>'" by (simp add: static_eval_state_to_state_let_unit)
   next
     case (Let_Prim x p e \<rho> \<kappa>)
-    assume "\<sigma> = \<langle>LET x = Prim p in e;\<rho>;\<kappa>\<rangle>" and "\<sigma>' = \<langle>e;\<rho> ++ [x \<mapsto> \<lbrace>p, \<rho>\<rbrace>];\<kappa>\<rangle>"
+    assume "\<sigma> = \<langle>LET x = Prim p in e;\<rho>;\<kappa>\<rangle>" and "\<sigma>' = \<langle>e;\<rho> ++ [x \<mapsto> (VClosure p \<rho>)];\<kappa>\<rangle>"
     with `(\<V>, \<C>) \<Turnstile>\<^sub>\<sigma> \<sigma>`
     show "(\<V>, \<C>) \<Turnstile>\<^sub>\<sigma> \<sigma>'" by (simp add: static_eval_state_to_state_let_prim)
   next
     case (Let_Fst \<rho> x\<^sub>p x\<^sub>1 x\<^sub>2 \<rho>\<^sub>p \<omega> x e \<kappa>)
     assume "\<sigma> = \<langle>LET x = FST x\<^sub>p in e;\<rho>;\<kappa>\<rangle>"
     and "\<sigma>' = \<langle>e;\<rho> ++ [x \<mapsto> \<omega>];\<kappa>\<rangle>"
-    and "\<rho> x\<^sub>p = Some \<lbrace>prim.Pair x\<^sub>1 x\<^sub>2, \<rho>\<^sub>p\<rbrace>" and "\<rho>\<^sub>p x\<^sub>1 = Some \<omega>"
+    and "\<rho> x\<^sub>p = Some (VClosure (Pair x\<^sub>1 x\<^sub>2) \<rho>\<^sub>p)" and "\<rho>\<^sub>p x\<^sub>1 = Some \<omega>"
     with `(\<V>, \<C>) \<Turnstile>\<^sub>\<sigma> \<sigma>`
     show "(\<V>, \<C>) \<Turnstile>\<^sub>\<sigma> \<sigma>'" by (simp add: static_eval_state_to_state_let_fst)
   next
     case (Let_Snd \<rho> x\<^sub>p x\<^sub>1 x\<^sub>2 \<rho>\<^sub>p \<omega> x e \<kappa>)
     assume "\<sigma> = \<langle>LET x = SND x\<^sub>p in e;\<rho>;\<kappa>\<rangle>"
     and "\<sigma>' = \<langle>e;\<rho> ++ [x \<mapsto> \<omega>];\<kappa>\<rangle>"
-    and "\<rho> x\<^sub>p = Some \<lbrace>prim.Pair x\<^sub>1 x\<^sub>2, \<rho>\<^sub>p\<rbrace>" and "\<rho>\<^sub>p x\<^sub>2 = Some \<omega>"
+    and "\<rho> x\<^sub>p = Some (VClosure (Pair x\<^sub>1 x\<^sub>2) \<rho>\<^sub>p)" and "\<rho>\<^sub>p x\<^sub>2 = Some \<omega>"
     with `(\<V>, \<C>) \<Turnstile>\<^sub>\<sigma> \<sigma>`
     show "(\<V>, \<C>) \<Turnstile>\<^sub>\<sigma> \<sigma>'" by (simp add: static_eval_state_to_state_let_snd)
   next
     case (Let_Case_Left \<rho> x\<^sub>s x\<^sub>l' \<rho>\<^sub>l \<omega>\<^sub>l x x\<^sub>l e\<^sub>l x\<^sub>r e\<^sub>r e \<kappa>)
-
     assume "\<sigma> = \<langle>LET x = CASE x\<^sub>s LEFT x\<^sub>l |> e\<^sub>l RIGHT x\<^sub>r |> e\<^sub>r in e;\<rho>;\<kappa>\<rangle>"
     and "\<sigma>' = \<langle>e\<^sub>l;\<rho> ++ [x\<^sub>l \<mapsto> \<omega>\<^sub>l];\<langle>x,e,\<rho>\<rangle> # \<kappa>\<rangle>"
-    and "\<rho> x\<^sub>s = Some \<lbrace>prim.Left x\<^sub>l', \<rho>\<^sub>l\<rbrace>" and "\<rho>\<^sub>l x\<^sub>l' = Some \<omega>\<^sub>l"
+    and "\<rho> x\<^sub>s = Some (VClosure (Left x\<^sub>l') \<rho>\<^sub>l)" and "\<rho>\<^sub>l x\<^sub>l' = Some \<omega>\<^sub>l"
     with `(\<V>, \<C>) \<Turnstile>\<^sub>\<sigma> \<sigma>`
     show "(\<V>, \<C>) \<Turnstile>\<^sub>\<sigma> \<sigma>'" by (simp add: static_eval_state_to_state_let_case_left)
   next
     case (Let_Case_Right \<rho> x\<^sub>s x\<^sub>r' \<rho>\<^sub>r \<omega>\<^sub>r x x\<^sub>l e\<^sub>l x\<^sub>r e\<^sub>r e \<kappa>)
     assume "\<sigma> = \<langle>LET x = CASE x\<^sub>s LEFT x\<^sub>l |> e\<^sub>l RIGHT x\<^sub>r |> e\<^sub>r in e;\<rho>;\<kappa>\<rangle>"
     and "\<sigma>' = \<langle>e\<^sub>r;\<rho> ++ [x\<^sub>r \<mapsto> \<omega>\<^sub>r];\<langle>x,e,\<rho>\<rangle> # \<kappa>\<rangle>"
-    and "\<rho> x\<^sub>s = Some \<lbrace>prim.Right x\<^sub>r', \<rho>\<^sub>r\<rbrace>"
+    and "\<rho> x\<^sub>s = Some (VClosure (Right x\<^sub>r') \<rho>\<^sub>r)"
     and "\<rho>\<^sub>r x\<^sub>r' = Some \<omega>\<^sub>r"
     with `(\<V>, \<C>) \<Turnstile>\<^sub>\<sigma> \<sigma>`
     show "(\<V>, \<C>) \<Turnstile>\<^sub>\<sigma> \<sigma>'" by (simp add: static_eval_state_to_state_let_case_right)
   next
     case (Let_App \<rho> f f\<^sub>l x\<^sub>l e\<^sub>l \<rho>\<^sub>l x\<^sub>a \<omega>\<^sub>a x e \<kappa>)
     assume "\<sigma> = \<langle>LET x = APP f x\<^sub>a in e;\<rho>;\<kappa>\<rangle>"
-    and "\<sigma>' = \<langle>e\<^sub>l;\<rho>\<^sub>l ++ [f\<^sub>l \<mapsto> \<lbrace>Abs f\<^sub>l x\<^sub>l e\<^sub>l, \<rho>\<^sub>l\<rbrace>, x\<^sub>l \<mapsto> \<omega>\<^sub>a];\<langle>x,e,\<rho>\<rangle> # \<kappa>\<rangle>"
-    and "\<rho> f = Some \<lbrace>Abs f\<^sub>l x\<^sub>l e\<^sub>l, \<rho>\<^sub>l\<rbrace>"
+    and "\<sigma>' = \<langle>e\<^sub>l;\<rho>\<^sub>l ++ [f\<^sub>l \<mapsto> (VClosure (Abs f\<^sub>l x\<^sub>l e\<^sub>l) \<rho>\<^sub>l), x\<^sub>l \<mapsto> \<omega>\<^sub>a];\<langle>x,e,\<rho>\<rangle> # \<kappa>\<rangle>"
+    and "\<rho> f = Some (VClosure (Abs f\<^sub>l x\<^sub>l e\<^sub>l) \<rho>\<^sub>l)"
     and "\<rho> x\<^sub>a = Some \<omega>\<^sub>a"
     with `(\<V>, \<C>) \<Turnstile>\<^sub>\<sigma> \<sigma>`
     show "(\<V>, \<C>) \<Turnstile>\<^sub>\<sigma> \<sigma>'" by (simp add: static_eval_state_to_state_let_app)
@@ -953,30 +952,30 @@ qed
 lemma static_eval_pool_let_sync_send_values_relate: "
   (\<V>, \<C>) \<Turnstile>\<^sub>\<E> \<E> \<Longrightarrow>
   \<E> \<pi>\<^sub>s = Some (\<langle>LET x\<^sub>s = SYNC x\<^sub>s\<^sub>e in e\<^sub>s; \<rho>\<^sub>s; \<kappa>\<^sub>s\<rangle>) \<Longrightarrow>
-  \<rho>\<^sub>s x\<^sub>s\<^sub>e = Some \<lbrace>Send_Evt x\<^sub>s\<^sub>c x\<^sub>m, \<rho>\<^sub>s\<^sub>e\<rbrace> \<Longrightarrow>
-  \<rho>\<^sub>s\<^sub>e x\<^sub>s\<^sub>c = Some \<lbrace>Ch \<pi>\<^sub>c x\<^sub>c\<rbrace> \<Longrightarrow>
+  \<rho>\<^sub>s x\<^sub>s\<^sub>e = Some (VClosure (Send_Evt x\<^sub>s\<^sub>c x\<^sub>m) \<rho>\<^sub>s\<^sub>e) \<Longrightarrow>
+  \<rho>\<^sub>s\<^sub>e x\<^sub>s\<^sub>c = Some (VChan (Ch \<pi>\<^sub>c x\<^sub>c)) \<Longrightarrow>
   {^\<lparr>\<rparr>} \<subseteq> \<V> x\<^sub>s \<and> \<V> x\<^sub>m \<subseteq> \<C> x\<^sub>c
 "
 proof -
   assume "(\<V>, \<C>) \<Turnstile>\<^sub>\<E> \<E>"
   and "\<E> \<pi>\<^sub>s = Some (\<langle>LET x\<^sub>s = SYNC x\<^sub>s\<^sub>e in e\<^sub>s; \<rho>\<^sub>s; \<kappa>\<^sub>s\<rangle>)"
-  and "\<rho>\<^sub>s x\<^sub>s\<^sub>e = Some \<lbrace>Send_Evt x\<^sub>s\<^sub>c x\<^sub>m, \<rho>\<^sub>s\<^sub>e\<rbrace>"
-  and "\<rho>\<^sub>s\<^sub>e x\<^sub>s\<^sub>c = Some \<lbrace>Ch \<pi>\<^sub>c x\<^sub>c\<rbrace>"
+  and "\<rho>\<^sub>s x\<^sub>s\<^sub>e = Some (VClosure (Send_Evt x\<^sub>s\<^sub>c x\<^sub>m) \<rho>\<^sub>s\<^sub>e)"
+  and "\<rho>\<^sub>s\<^sub>e x\<^sub>s\<^sub>c = Some (VChan (Ch \<pi>\<^sub>c x\<^sub>c))"
 
   from `(\<V>, \<C>) \<Turnstile>\<^sub>\<E> \<E>` and `\<E> \<pi>\<^sub>s = Some (\<langle>LET x\<^sub>s = SYNC x\<^sub>s\<^sub>e in e\<^sub>s; \<rho>\<^sub>s; \<kappa>\<^sub>s\<rangle>)`
   have "(\<V>, \<C>) \<Turnstile>\<^sub>\<sigma> \<langle>LET x\<^sub>s = SYNC x\<^sub>s\<^sub>e in e\<^sub>s; \<rho>\<^sub>s; \<kappa>\<^sub>s\<rangle>" by (simp add: static_eval_pool.simps) then
   have "(\<V>, \<C>) \<Turnstile>\<^sub>e LET x\<^sub>s = SYNC x\<^sub>s\<^sub>e in e\<^sub>s" "(\<V>, \<C>) \<Turnstile>\<^sub>\<rho> \<rho>\<^sub>s" by (simp add: static_eval_state.simps)+
 
-  from `(\<V>, \<C>) \<Turnstile>\<^sub>\<rho> \<rho>\<^sub>s` and `\<rho>\<^sub>s x\<^sub>s\<^sub>e = Some \<lbrace>Send_Evt x\<^sub>s\<^sub>c x\<^sub>m, \<rho>\<^sub>s\<^sub>e\<rbrace>`
-  have "{|\<lbrace>Send_Evt x\<^sub>s\<^sub>c x\<^sub>m, \<rho>\<^sub>s\<^sub>e\<rbrace>|} \<subseteq> \<V> x\<^sub>s\<^sub>e" and "(\<V>, \<C>) \<Turnstile>\<^sub>\<omega> \<lbrace>Send_Evt x\<^sub>s\<^sub>c x\<^sub>m, \<rho>\<^sub>s\<^sub>e\<rbrace>" by (blast intro: static_eval_env.cases)+
+  from `(\<V>, \<C>) \<Turnstile>\<^sub>\<rho> \<rho>\<^sub>s` and `\<rho>\<^sub>s x\<^sub>s\<^sub>e = Some (VClosure (Send_Evt x\<^sub>s\<^sub>c x\<^sub>m) \<rho>\<^sub>s\<^sub>e)`
+  have "{|(VClosure (Send_Evt x\<^sub>s\<^sub>c x\<^sub>m) \<rho>\<^sub>s\<^sub>e)|} \<subseteq> \<V> x\<^sub>s\<^sub>e" and "(\<V>, \<C>) \<Turnstile>\<^sub>\<omega> (VClosure (Send_Evt x\<^sub>s\<^sub>c x\<^sub>m) \<rho>\<^sub>s\<^sub>e)" by (blast intro: static_eval_env.cases)+
 
-  from `{|\<lbrace>Send_Evt x\<^sub>s\<^sub>c x\<^sub>m, \<rho>\<^sub>s\<^sub>e\<rbrace>|} \<subseteq> \<V> x\<^sub>s\<^sub>e`
+  from `{|(VClosure (Send_Evt x\<^sub>s\<^sub>c x\<^sub>m) \<rho>\<^sub>s\<^sub>e)|} \<subseteq> \<V> x\<^sub>s\<^sub>e`
   have "^Send_Evt x\<^sub>s\<^sub>c x\<^sub>m \<in> \<V> x\<^sub>s\<^sub>e" by simp
 
-  from `(\<V>, \<C>) \<Turnstile>\<^sub>\<omega> \<lbrace>Send_Evt x\<^sub>s\<^sub>c x\<^sub>m, \<rho>\<^sub>s\<^sub>e\<rbrace>`
+  from `(\<V>, \<C>) \<Turnstile>\<^sub>\<omega> (VClosure (Send_Evt x\<^sub>s\<^sub>c x\<^sub>m) \<rho>\<^sub>s\<^sub>e)`
   have "(\<V>, \<C>) \<Turnstile>\<^sub>\<rho> \<rho>\<^sub>s\<^sub>e" by (blast intro: static_eval_value.cases)
-  with `\<rho>\<^sub>s\<^sub>e x\<^sub>s\<^sub>c = Some \<lbrace>Ch \<pi>\<^sub>c x\<^sub>c\<rbrace>`
-  have "{|\<lbrace>Ch \<pi>\<^sub>c x\<^sub>c\<rbrace>|} \<subseteq> \<V> x\<^sub>s\<^sub>c" by (blast intro: static_eval_env.cases) then
+  with `\<rho>\<^sub>s\<^sub>e x\<^sub>s\<^sub>c = Some (VChan (Ch \<pi>\<^sub>c x\<^sub>c))`
+  have "{|(VChan (Ch \<pi>\<^sub>c x\<^sub>c))|} \<subseteq> \<V> x\<^sub>s\<^sub>c" by (blast intro: static_eval_env.cases) then
   have "{^Chan x\<^sub>c} \<subseteq> \<V> x\<^sub>s\<^sub>c" by simp then
   have "^Chan x\<^sub>c \<in> \<V> x\<^sub>s\<^sub>c" by auto
   
@@ -994,21 +993,21 @@ qed
 lemma static_eval_pool_let_sync_send_message_relate: "
   (\<V>, \<C>) \<Turnstile>\<^sub>\<E> \<E> \<Longrightarrow>
   \<E> \<pi>\<^sub>s = Some (\<langle>LET x\<^sub>s = SYNC x\<^sub>s\<^sub>e in e\<^sub>s; \<rho>\<^sub>s; \<kappa>\<^sub>s\<rangle>) \<Longrightarrow>
-  \<rho>\<^sub>s x\<^sub>s\<^sub>e = Some \<lbrace>Send_Evt x\<^sub>s\<^sub>c x\<^sub>m, \<rho>\<^sub>s\<^sub>e\<rbrace> \<Longrightarrow>
+  \<rho>\<^sub>s x\<^sub>s\<^sub>e = Some (VClosure (Send_Evt x\<^sub>s\<^sub>c x\<^sub>m) \<rho>\<^sub>s\<^sub>e) \<Longrightarrow>
   \<rho>\<^sub>s\<^sub>e x\<^sub>m = Some \<omega>\<^sub>m \<Longrightarrow>
   {|\<omega>\<^sub>m|} \<subseteq> \<V> x\<^sub>m \<and> (\<V>, \<C>) \<Turnstile>\<^sub>\<omega> \<omega>\<^sub>m
 "
 proof -
   assume "(\<V>, \<C>) \<Turnstile>\<^sub>\<E> \<E>"
   and "\<E> \<pi>\<^sub>s = Some (\<langle>LET x\<^sub>s = SYNC x\<^sub>s\<^sub>e in e\<^sub>s; \<rho>\<^sub>s; \<kappa>\<^sub>s\<rangle>)"
-  and "\<rho>\<^sub>s x\<^sub>s\<^sub>e = Some \<lbrace>Send_Evt x\<^sub>s\<^sub>c x\<^sub>m, \<rho>\<^sub>s\<^sub>e\<rbrace>"
+  and "\<rho>\<^sub>s x\<^sub>s\<^sub>e = Some (VClosure (Send_Evt x\<^sub>s\<^sub>c x\<^sub>m) \<rho>\<^sub>s\<^sub>e)"
   and "\<rho>\<^sub>s\<^sub>e x\<^sub>m = Some \<omega>\<^sub>m"
 
   from `(\<V>, \<C>) \<Turnstile>\<^sub>\<E> \<E>` and `\<E> \<pi>\<^sub>s = Some (\<langle>LET x\<^sub>s = SYNC x\<^sub>s\<^sub>e in e\<^sub>s; \<rho>\<^sub>s; \<kappa>\<^sub>s\<rangle>)`
   have "(\<V>, \<C>) \<Turnstile>\<^sub>\<sigma> \<langle>LET x\<^sub>s = SYNC x\<^sub>s\<^sub>e in e\<^sub>s; \<rho>\<^sub>s; \<kappa>\<^sub>s\<rangle>" by (simp add: static_eval_pool.simps) then
   have "(\<V>, \<C>) \<Turnstile>\<^sub>\<rho> \<rho>\<^sub>s" by (simp add: static_eval_state.simps)
-  with `\<rho>\<^sub>s x\<^sub>s\<^sub>e = Some \<lbrace>Send_Evt x\<^sub>s\<^sub>c x\<^sub>m, \<rho>\<^sub>s\<^sub>e\<rbrace>`
-  have "(\<V>, \<C>) \<Turnstile>\<^sub>\<omega> \<lbrace>Send_Evt x\<^sub>s\<^sub>c x\<^sub>m, \<rho>\<^sub>s\<^sub>e\<rbrace>" by (blast intro: static_eval_env.cases) then
+  with `\<rho>\<^sub>s x\<^sub>s\<^sub>e = Some (VClosure (Send_Evt x\<^sub>s\<^sub>c x\<^sub>m) \<rho>\<^sub>s\<^sub>e)`
+  have "(\<V>, \<C>) \<Turnstile>\<^sub>\<omega> (VClosure (Send_Evt x\<^sub>s\<^sub>c x\<^sub>m) \<rho>\<^sub>s\<^sub>e)" by (blast intro: static_eval_env.cases) then
   have "(\<V>, \<C>) \<Turnstile>\<^sub>\<rho> \<rho>\<^sub>s\<^sub>e" by (blast intro: static_eval_value.cases)
   with `\<rho>\<^sub>s\<^sub>e x\<^sub>m = Some \<omega>\<^sub>m`
   show "{|\<omega>\<^sub>m|} \<subseteq> \<V> x\<^sub>m \<and> (\<V>, \<C>) \<Turnstile>\<^sub>\<omega> \<omega>\<^sub>m" by (blast intro: static_eval_env.cases)
@@ -1017,15 +1016,15 @@ qed
 lemma static_eval_pool_to_env_let_sync_send: "
   (\<V>, \<C>) \<Turnstile>\<^sub>\<E> \<E> \<Longrightarrow>
   \<E> \<pi>\<^sub>s = Some (\<langle>LET x\<^sub>s = SYNC x\<^sub>s\<^sub>e in e\<^sub>s; \<rho>\<^sub>s; \<kappa>\<^sub>s\<rangle>) \<Longrightarrow>
-  \<rho>\<^sub>s x\<^sub>s\<^sub>e = Some \<lbrace>Send_Evt x\<^sub>s\<^sub>c x\<^sub>m, \<rho>\<^sub>s\<^sub>e\<rbrace> \<Longrightarrow>
-  \<rho>\<^sub>s\<^sub>e x\<^sub>s\<^sub>c = Some \<lbrace>c\<rbrace> \<Longrightarrow>
-  (\<V>, \<C>) \<Turnstile>\<^sub>\<rho> \<rho>\<^sub>s(x\<^sub>s \<mapsto> \<lbrace>\<rbrace>)
+  \<rho>\<^sub>s x\<^sub>s\<^sub>e = Some (VClosure (Send_Evt x\<^sub>s\<^sub>c x\<^sub>m) \<rho>\<^sub>s\<^sub>e) \<Longrightarrow>
+  \<rho>\<^sub>s\<^sub>e x\<^sub>s\<^sub>c = Some (VChan c) \<Longrightarrow>
+  (\<V>, \<C>) \<Turnstile>\<^sub>\<rho> \<rho>\<^sub>s(x\<^sub>s \<mapsto> VUnit)
 "
 proof
-  assume "\<rho>\<^sub>s\<^sub>e x\<^sub>s\<^sub>c = Some \<lbrace>c\<rbrace>"
+  assume "\<rho>\<^sub>s\<^sub>e x\<^sub>s\<^sub>c = Some (VChan c)"
   and  "(\<V>, \<C>) \<Turnstile>\<^sub>\<E> \<E>"
   and "\<E> \<pi>\<^sub>s = Some (\<langle>LET x\<^sub>s = SYNC x\<^sub>s\<^sub>e in e\<^sub>s; \<rho>\<^sub>s; \<kappa>\<^sub>s\<rangle>)"
-  and "\<rho>\<^sub>s x\<^sub>s\<^sub>e = Some \<lbrace>Send_Evt x\<^sub>s\<^sub>c x\<^sub>m, \<rho>\<^sub>s\<^sub>e\<rbrace>"
+  and "\<rho>\<^sub>s x\<^sub>s\<^sub>e = Some (VClosure (Send_Evt x\<^sub>s\<^sub>c x\<^sub>m) \<rho>\<^sub>s\<^sub>e)"
 
   from `(\<V>, \<C>) \<Turnstile>\<^sub>\<E> \<E>` and `\<E> \<pi>\<^sub>s = Some (\<langle>LET x\<^sub>s = SYNC x\<^sub>s\<^sub>e in e\<^sub>s; \<rho>\<^sub>s; \<kappa>\<^sub>s\<rangle>)`
   have "(\<V>, \<C>) \<Turnstile>\<^sub>\<sigma> \<langle>LET x\<^sub>s = SYNC x\<^sub>s\<^sub>e in e\<^sub>s; \<rho>\<^sub>s; \<kappa>\<^sub>s\<rangle>" by (simp add: static_eval_pool.simps) then
@@ -1035,53 +1034,53 @@ proof
   proof (cases c)
     case (Ch \<pi> x\<^sub>c)
     assume "c = Ch \<pi> x\<^sub>c" 
-    with `\<rho>\<^sub>s\<^sub>e x\<^sub>s\<^sub>c = Some \<lbrace>c\<rbrace>`
+    with `\<rho>\<^sub>s\<^sub>e x\<^sub>s\<^sub>c = Some (VChan c)`
     and  `(\<V>, \<C>) \<Turnstile>\<^sub>\<E> \<E>`
     and `\<E> \<pi>\<^sub>s = Some (\<langle>LET x\<^sub>s = SYNC x\<^sub>s\<^sub>e in e\<^sub>s; \<rho>\<^sub>s; \<kappa>\<^sub>s\<rangle>)`
-    and `\<rho>\<^sub>s x\<^sub>s\<^sub>e = Some \<lbrace>Send_Evt x\<^sub>s\<^sub>c x\<^sub>m, \<rho>\<^sub>s\<^sub>e\<rbrace>`
+    and `\<rho>\<^sub>s x\<^sub>s\<^sub>e = Some (VClosure (Send_Evt x\<^sub>s\<^sub>c x\<^sub>m) \<rho>\<^sub>s\<^sub>e)`
     show "{^\<lparr>\<rparr>} \<subseteq> \<V> x\<^sub>s" using static_eval_pool_let_sync_send_values_relate by simp
   qed
   
-  have "(\<V>, \<C>) \<Turnstile>\<^sub>\<omega> \<lbrace>\<rbrace>" by (simp add: Unit)
+  have "(\<V>, \<C>) \<Turnstile>\<^sub>\<omega> VUnit" by (simp add: Unit)
   {
     fix x' \<omega>'
-    assume "(\<rho>\<^sub>s(x\<^sub>s \<mapsto> \<lbrace>\<rbrace>)) x' = Some \<omega>'" "x' \<noteq> x\<^sub>s" then
+    assume "(\<rho>\<^sub>s(x\<^sub>s \<mapsto> VUnit)) x' = Some \<omega>'" "x' \<noteq> x\<^sub>s" then
     have "\<rho>\<^sub>s x' = Some \<omega>'" by simp
     with `(\<V>, \<C>) \<Turnstile>\<^sub>\<rho> \<rho>\<^sub>s` 
     have "{|\<omega>'|} \<subseteq> \<V> x' \<and> (\<V>, \<C>) \<Turnstile>\<^sub>\<omega> \<omega>'" by (simp add: static_eval_env.simps)
   }
-  with \<open>{^\<lparr>\<rparr>} \<subseteq> \<V> x\<^sub>s\<close> \<open>(\<V>, \<C>) \<Turnstile>\<^sub>\<omega> \<lbrace>\<rbrace>\<close> 
-  show "\<forall>x \<omega>. (\<rho>\<^sub>s(x\<^sub>s \<mapsto> \<lbrace>\<rbrace>)) x = Some \<omega> \<longrightarrow> {|\<omega>|} \<subseteq> \<V> x \<and> (\<V>, \<C>) \<Turnstile>\<^sub>\<omega> \<omega>" by simp
+  with \<open>{^\<lparr>\<rparr>} \<subseteq> \<V> x\<^sub>s\<close> \<open>(\<V>, \<C>) \<Turnstile>\<^sub>\<omega> VUnit\<close> 
+  show "\<forall>x \<omega>. (\<rho>\<^sub>s(x\<^sub>s \<mapsto> VUnit)) x = Some \<omega> \<longrightarrow> {|\<omega>|} \<subseteq> \<V> x \<and> (\<V>, \<C>) \<Turnstile>\<^sub>\<omega> \<omega>" by simp
 qed
 
 
 lemma static_eval_pool_let_sync_recv_values_relate: "
   (\<V>, \<C>) \<Turnstile>\<^sub>\<E> \<E> \<Longrightarrow>
   \<E> \<pi>\<^sub>r = Some (\<langle>LET x\<^sub>r = SYNC x\<^sub>r\<^sub>e in e\<^sub>r; \<rho>\<^sub>r; \<kappa>\<^sub>r\<rangle>) \<Longrightarrow>
-  \<rho>\<^sub>r x\<^sub>r\<^sub>e = Some \<lbrace>Recv_Evt x\<^sub>r\<^sub>c, \<rho>\<^sub>r\<^sub>e\<rbrace> \<Longrightarrow>
-  \<rho>\<^sub>r\<^sub>e x\<^sub>r\<^sub>c = Some \<lbrace>Ch \<pi>\<^sub>c x\<^sub>c\<rbrace> \<Longrightarrow>
+  \<rho>\<^sub>r x\<^sub>r\<^sub>e = Some (VClosure (Recv_Evt x\<^sub>r\<^sub>c) \<rho>\<^sub>r\<^sub>e) \<Longrightarrow>
+  \<rho>\<^sub>r\<^sub>e x\<^sub>r\<^sub>c = Some (VChan (Ch \<pi>\<^sub>c x\<^sub>c)) \<Longrightarrow>
   \<C> x\<^sub>c \<subseteq> \<V> x\<^sub>r
 "
 proof -
   assume "(\<V>, \<C>) \<Turnstile>\<^sub>\<E> \<E>"
   and "\<E> \<pi>\<^sub>r = Some (\<langle>LET x\<^sub>r = SYNC x\<^sub>r\<^sub>e in e\<^sub>r; \<rho>\<^sub>r; \<kappa>\<^sub>r\<rangle>)"
-  and "\<rho>\<^sub>r x\<^sub>r\<^sub>e = Some \<lbrace>Recv_Evt x\<^sub>r\<^sub>c, \<rho>\<^sub>r\<^sub>e\<rbrace>"
-  and "\<rho>\<^sub>r\<^sub>e x\<^sub>r\<^sub>c = Some \<lbrace>Ch \<pi>\<^sub>c x\<^sub>c\<rbrace>"
+  and "\<rho>\<^sub>r x\<^sub>r\<^sub>e = Some (VClosure (Recv_Evt x\<^sub>r\<^sub>c) \<rho>\<^sub>r\<^sub>e)"
+  and "\<rho>\<^sub>r\<^sub>e x\<^sub>r\<^sub>c = Some (VChan (Ch \<pi>\<^sub>c x\<^sub>c))"
 
   from `(\<V>, \<C>) \<Turnstile>\<^sub>\<E> \<E>` and `\<E> \<pi>\<^sub>r = Some (\<langle>LET x\<^sub>r = SYNC x\<^sub>r\<^sub>e in e\<^sub>r; \<rho>\<^sub>r; \<kappa>\<^sub>r\<rangle>)`
   have "(\<V>, \<C>) \<Turnstile>\<^sub>\<sigma> \<langle>LET x\<^sub>r = SYNC x\<^sub>r\<^sub>e in e\<^sub>r; \<rho>\<^sub>r; \<kappa>\<^sub>r\<rangle>" by (simp add: static_eval_pool.simps) then
   have "(\<V>, \<C>) \<Turnstile>\<^sub>e LET x\<^sub>r = SYNC x\<^sub>r\<^sub>e in e\<^sub>r" "(\<V>, \<C>) \<Turnstile>\<^sub>\<rho> \<rho>\<^sub>r" by (simp add: static_eval_state.simps)+
 
-  from `(\<V>, \<C>) \<Turnstile>\<^sub>\<rho> \<rho>\<^sub>r` and `\<rho>\<^sub>r x\<^sub>r\<^sub>e = Some \<lbrace>Recv_Evt x\<^sub>r\<^sub>c, \<rho>\<^sub>r\<^sub>e\<rbrace>`
-  have "{|\<lbrace>Recv_Evt x\<^sub>r\<^sub>c, \<rho>\<^sub>r\<^sub>e\<rbrace>|} \<subseteq> \<V> x\<^sub>r\<^sub>e" and "(\<V>, \<C>) \<Turnstile>\<^sub>\<omega> \<lbrace>Recv_Evt x\<^sub>r\<^sub>c, \<rho>\<^sub>r\<^sub>e\<rbrace>" by (blast intro: static_eval_env.cases)+
+  from `(\<V>, \<C>) \<Turnstile>\<^sub>\<rho> \<rho>\<^sub>r` and `\<rho>\<^sub>r x\<^sub>r\<^sub>e = Some (VClosure (Recv_Evt x\<^sub>r\<^sub>c) \<rho>\<^sub>r\<^sub>e)`
+  have "{|(VClosure (Recv_Evt x\<^sub>r\<^sub>c) \<rho>\<^sub>r\<^sub>e)|} \<subseteq> \<V> x\<^sub>r\<^sub>e" and "(\<V>, \<C>) \<Turnstile>\<^sub>\<omega> (VClosure (Recv_Evt x\<^sub>r\<^sub>c) \<rho>\<^sub>r\<^sub>e)" by (blast intro: static_eval_env.cases)+
 
-  from `{|\<lbrace>Recv_Evt x\<^sub>r\<^sub>c, \<rho>\<^sub>r\<^sub>e\<rbrace>|} \<subseteq> \<V> x\<^sub>r\<^sub>e`
+  from `{|(VClosure (Recv_Evt x\<^sub>r\<^sub>c) \<rho>\<^sub>r\<^sub>e)|} \<subseteq> \<V> x\<^sub>r\<^sub>e`
   have "^Recv_Evt x\<^sub>r\<^sub>c \<in> \<V> x\<^sub>r\<^sub>e" by simp
 
-  from `(\<V>, \<C>) \<Turnstile>\<^sub>\<omega> \<lbrace>Recv_Evt x\<^sub>r\<^sub>c, \<rho>\<^sub>r\<^sub>e\<rbrace>`
+  from `(\<V>, \<C>) \<Turnstile>\<^sub>\<omega> (VClosure (Recv_Evt x\<^sub>r\<^sub>c) \<rho>\<^sub>r\<^sub>e)`
   have "(\<V>, \<C>) \<Turnstile>\<^sub>\<rho> \<rho>\<^sub>r\<^sub>e" by (blast intro: static_eval_value.cases)
-  with `\<rho>\<^sub>r\<^sub>e x\<^sub>r\<^sub>c = Some \<lbrace>Ch \<pi>\<^sub>c x\<^sub>c\<rbrace>`
-  have "{|\<lbrace>Ch \<pi>\<^sub>c x\<^sub>c\<rbrace>|} \<subseteq> \<V> x\<^sub>r\<^sub>c" by (blast intro: static_eval_env.cases) then
+  with `\<rho>\<^sub>r\<^sub>e x\<^sub>r\<^sub>c = Some (VChan (Ch \<pi>\<^sub>c x\<^sub>c))`
+  have "{|(VChan (Ch \<pi>\<^sub>c x\<^sub>c))|} \<subseteq> \<V> x\<^sub>r\<^sub>c" by (blast intro: static_eval_env.cases) then
   have "{^Chan x\<^sub>c} \<subseteq> \<V> x\<^sub>r\<^sub>c" by simp then
   have "^Chan x\<^sub>c \<in> \<V> x\<^sub>r\<^sub>c" by auto
   
@@ -1110,25 +1109,25 @@ qed
 lemma static_eval_pool_to_env_let_sync_recv: "
   (\<V>, \<C>) \<Turnstile>\<^sub>\<E> \<E> \<Longrightarrow>
   \<E> \<pi>\<^sub>s = Some (\<langle>LET x\<^sub>s = SYNC x\<^sub>s\<^sub>e in e\<^sub>s; \<rho>\<^sub>s; \<kappa>\<^sub>s\<rangle>) \<Longrightarrow>
-  \<rho>\<^sub>s x\<^sub>s\<^sub>e = Some \<lbrace>Send_Evt x\<^sub>s\<^sub>c x\<^sub>m, \<rho>\<^sub>s\<^sub>e\<rbrace> \<Longrightarrow>
-  \<rho>\<^sub>s\<^sub>e x\<^sub>s\<^sub>c = Some \<lbrace>c\<rbrace> \<Longrightarrow>
+  \<rho>\<^sub>s x\<^sub>s\<^sub>e = Some (VClosure (Send_Evt x\<^sub>s\<^sub>c x\<^sub>m) \<rho>\<^sub>s\<^sub>e) \<Longrightarrow>
+  \<rho>\<^sub>s\<^sub>e x\<^sub>s\<^sub>c = Some (VChan c) \<Longrightarrow>
   \<rho>\<^sub>s\<^sub>e x\<^sub>m = Some \<omega>\<^sub>m \<Longrightarrow>
   \<E> \<pi>\<^sub>r = Some (\<langle>LET x\<^sub>r = SYNC x\<^sub>r\<^sub>e in e\<^sub>r; \<rho>\<^sub>r; \<kappa>\<^sub>r\<rangle>) \<Longrightarrow> 
-  \<rho>\<^sub>r x\<^sub>r\<^sub>e = Some \<lbrace>Recv_Evt x\<^sub>r\<^sub>c, \<rho>\<^sub>r\<^sub>e\<rbrace> \<Longrightarrow> 
-  \<rho>\<^sub>r\<^sub>e x\<^sub>r\<^sub>c = Some \<lbrace>c\<rbrace> \<Longrightarrow> 
+  \<rho>\<^sub>r x\<^sub>r\<^sub>e = Some (VClosure (Recv_Evt x\<^sub>r\<^sub>c) \<rho>\<^sub>r\<^sub>e) \<Longrightarrow> 
+  \<rho>\<^sub>r\<^sub>e x\<^sub>r\<^sub>c = Some (VChan c) \<Longrightarrow> 
   (\<V>, \<C>) \<Turnstile>\<^sub>\<rho> \<rho>\<^sub>r(x\<^sub>r \<mapsto> \<omega>\<^sub>m)
 "
 proof
   assume "(\<V>, \<C>) \<Turnstile>\<^sub>\<E> \<E>"
   and "\<E> \<pi>\<^sub>s = Some (\<langle>LET x\<^sub>s = SYNC x\<^sub>s\<^sub>e in e\<^sub>s; \<rho>\<^sub>s; \<kappa>\<^sub>s\<rangle>)"
-  and "\<rho>\<^sub>s x\<^sub>s\<^sub>e = Some \<lbrace>Send_Evt x\<^sub>s\<^sub>c x\<^sub>m, \<rho>\<^sub>s\<^sub>e\<rbrace>"
+  and "\<rho>\<^sub>s x\<^sub>s\<^sub>e = Some (VClosure (Send_Evt x\<^sub>s\<^sub>c x\<^sub>m) \<rho>\<^sub>s\<^sub>e)"
   and "\<rho>\<^sub>s\<^sub>e x\<^sub>m = Some \<omega>\<^sub>m" then
   have "{|\<omega>\<^sub>m|} \<subseteq> \<V> x\<^sub>m" "(\<V>, \<C>) \<Turnstile>\<^sub>\<omega> \<omega>\<^sub>m" using static_eval_pool_let_sync_send_message_relate by auto
 
-  assume "\<rho>\<^sub>s\<^sub>e x\<^sub>s\<^sub>c = Some \<lbrace>c\<rbrace>"
+  assume "\<rho>\<^sub>s\<^sub>e x\<^sub>s\<^sub>c = Some (VChan c)"
   and "\<E> \<pi>\<^sub>r = Some (\<langle>LET x\<^sub>r = SYNC x\<^sub>r\<^sub>e in e\<^sub>r; \<rho>\<^sub>r; \<kappa>\<^sub>r\<rangle>)"
-  and "\<rho>\<^sub>r x\<^sub>r\<^sub>e = Some \<lbrace>Recv_Evt x\<^sub>r\<^sub>c, \<rho>\<^sub>r\<^sub>e\<rbrace>"
-  and "\<rho>\<^sub>r\<^sub>e x\<^sub>r\<^sub>c = Some \<lbrace>c\<rbrace>"
+  and "\<rho>\<^sub>r x\<^sub>r\<^sub>e = Some (VClosure (Recv_Evt x\<^sub>r\<^sub>c) \<rho>\<^sub>r\<^sub>e)"
+  and "\<rho>\<^sub>r\<^sub>e x\<^sub>r\<^sub>c = Some (VChan c)"
 
   from `(\<V>, \<C>) \<Turnstile>\<^sub>\<E> \<E>` and `\<E> \<pi>\<^sub>r = Some (\<langle>LET x\<^sub>r = SYNC x\<^sub>r\<^sub>e in e\<^sub>r; \<rho>\<^sub>r; \<kappa>\<^sub>r\<rangle>)`
   have "(\<V>, \<C>) \<Turnstile>\<^sub>\<sigma> \<langle>LET x\<^sub>r = SYNC x\<^sub>r\<^sub>e in e\<^sub>r; \<rho>\<^sub>r; \<kappa>\<^sub>r\<rangle>" by (simp add: static_eval_pool.simps) then
@@ -1141,18 +1140,18 @@ proof
     assume "c = Ch \<pi>\<^sub>c x\<^sub>c" 
 
     with `c = Ch \<pi>\<^sub>c x\<^sub>c`
-    and `\<rho>\<^sub>s\<^sub>e x\<^sub>s\<^sub>c = Some \<lbrace>c\<rbrace>`
+    and `\<rho>\<^sub>s\<^sub>e x\<^sub>s\<^sub>c = Some (VChan c)`
     and `(\<V>, \<C>) \<Turnstile>\<^sub>\<E> \<E>`
-    and `\<rho>\<^sub>s x\<^sub>s\<^sub>e = Some \<lbrace>Send_Evt x\<^sub>s\<^sub>c x\<^sub>m, \<rho>\<^sub>s\<^sub>e\<rbrace>`
+    and `\<rho>\<^sub>s x\<^sub>s\<^sub>e = Some (VClosure (Send_Evt x\<^sub>s\<^sub>c x\<^sub>m) \<rho>\<^sub>s\<^sub>e)`
     and `\<E> \<pi>\<^sub>s = Some (\<langle>LET x\<^sub>s = SYNC x\<^sub>s\<^sub>e in e\<^sub>s; \<rho>\<^sub>s; \<kappa>\<^sub>s\<rangle>)`
     and `\<rho>\<^sub>s\<^sub>e x\<^sub>m = Some \<omega>\<^sub>m`
-    have "\<V> x\<^sub>m \<subseteq> \<C> x\<^sub>c" using \<open>\<rho>\<^sub>s\<^sub>e x\<^sub>s\<^sub>c = Some \<lbrace>c\<rbrace>\<close> static_eval_pool_let_sync_send_values_relate by blast
+    have "\<V> x\<^sub>m \<subseteq> \<C> x\<^sub>c" using \<open>\<rho>\<^sub>s\<^sub>e x\<^sub>s\<^sub>c = Some (VChan c)\<close> static_eval_pool_let_sync_send_values_relate by blast
 
     with `c = Ch \<pi>\<^sub>c x\<^sub>c`
-    and `\<rho>\<^sub>r\<^sub>e x\<^sub>r\<^sub>c = Some \<lbrace>c\<rbrace>`
+    and `\<rho>\<^sub>r\<^sub>e x\<^sub>r\<^sub>c = Some (VChan c)`
     and `(\<V>, \<C>) \<Turnstile>\<^sub>\<E> \<E>`
     and `\<E> \<pi>\<^sub>r = Some (\<langle>LET x\<^sub>r = SYNC x\<^sub>r\<^sub>e in e\<^sub>r; \<rho>\<^sub>r; \<kappa>\<^sub>r\<rangle>)`
-    and `\<rho>\<^sub>r x\<^sub>r\<^sub>e = Some \<lbrace>Recv_Evt x\<^sub>r\<^sub>c, \<rho>\<^sub>r\<^sub>e\<rbrace>`
+    and `\<rho>\<^sub>r x\<^sub>r\<^sub>e = Some (VClosure (Recv_Evt x\<^sub>r\<^sub>c) \<rho>\<^sub>r\<^sub>e)`
     have "\<C> x\<^sub>c \<subseteq> \<V> x\<^sub>r" using  static_eval_pool_let_sync_recv_values_relate by auto
 
     from `\<V> x\<^sub>m \<subseteq> \<C> x\<^sub>c` and `\<C> x\<^sub>c \<subseteq> \<V> x\<^sub>r`
@@ -1180,47 +1179,47 @@ qed
 lemma static_eval_preserved_under_sync: "
   (\<V>, \<C>) \<Turnstile>\<^sub>\<E> \<E> \<Longrightarrow>
   \<E> \<pi>\<^sub>s = Some (\<langle>LET x\<^sub>s = SYNC x\<^sub>s\<^sub>e in e\<^sub>s; \<rho>\<^sub>s; \<kappa>\<^sub>s\<rangle>) \<Longrightarrow>
-  \<rho>\<^sub>s x\<^sub>s\<^sub>e = Some \<lbrace>Send_Evt x\<^sub>s\<^sub>c x\<^sub>m, \<rho>\<^sub>s\<^sub>e\<rbrace> \<Longrightarrow>
-  \<rho>\<^sub>s\<^sub>e x\<^sub>s\<^sub>c = Some \<lbrace>c\<rbrace> \<Longrightarrow>
+  \<rho>\<^sub>s x\<^sub>s\<^sub>e = Some (VClosure (Send_Evt x\<^sub>s\<^sub>c x\<^sub>m) \<rho>\<^sub>s\<^sub>e) \<Longrightarrow>
+  \<rho>\<^sub>s\<^sub>e x\<^sub>s\<^sub>c = Some (VChan c) \<Longrightarrow>
   \<rho>\<^sub>s\<^sub>e x\<^sub>m = Some \<omega>\<^sub>m \<Longrightarrow>
   \<E> \<pi>\<^sub>r = Some (\<langle>LET x\<^sub>r = SYNC x\<^sub>r\<^sub>e in e\<^sub>r; \<rho>\<^sub>r; \<kappa>\<^sub>r\<rangle>) \<Longrightarrow>
-  \<rho>\<^sub>r x\<^sub>r\<^sub>e = Some \<lbrace>Recv_Evt x\<^sub>r\<^sub>c, \<rho>\<^sub>r\<^sub>e\<rbrace> \<Longrightarrow>
-  \<rho>\<^sub>r\<^sub>e x\<^sub>r\<^sub>c = Some \<lbrace>c\<rbrace> \<Longrightarrow> 
-  (\<V>, \<C>) \<Turnstile>\<^sub>\<E> \<E>(\<pi>\<^sub>s ;;(LNext x\<^sub>s) \<mapsto> \<langle>e\<^sub>s; \<rho>\<^sub>s(x\<^sub>s \<mapsto> \<lbrace>\<rbrace>); \<kappa>\<^sub>s\<rangle>, \<pi>\<^sub>r ;;(LNext x\<^sub>r) \<mapsto> \<langle>e\<^sub>r; \<rho>\<^sub>r(x\<^sub>r \<mapsto> \<omega>\<^sub>m); \<kappa>\<^sub>r\<rangle>)
+  \<rho>\<^sub>r x\<^sub>r\<^sub>e = Some (VClosure (Recv_Evt x\<^sub>r\<^sub>c) \<rho>\<^sub>r\<^sub>e) \<Longrightarrow>
+  \<rho>\<^sub>r\<^sub>e x\<^sub>r\<^sub>c = Some (VChan c) \<Longrightarrow> 
+  (\<V>, \<C>) \<Turnstile>\<^sub>\<E> \<E>(\<pi>\<^sub>s ;;(LNext x\<^sub>s) \<mapsto> \<langle>e\<^sub>s; \<rho>\<^sub>s(x\<^sub>s \<mapsto> VUnit); \<kappa>\<^sub>s\<rangle>, \<pi>\<^sub>r ;;(LNext x\<^sub>r) \<mapsto> \<langle>e\<^sub>r; \<rho>\<^sub>r(x\<^sub>r \<mapsto> \<omega>\<^sub>m); \<kappa>\<^sub>r\<rangle>)
 "
 proof
   assume "(\<V>, \<C>) \<Turnstile>\<^sub>\<E> \<E>"
   and "\<E> \<pi>\<^sub>s = Some (\<langle>LET x\<^sub>s = SYNC x\<^sub>s\<^sub>e in e\<^sub>s;\<rho>\<^sub>s;\<kappa>\<^sub>s\<rangle>)"
-  and "\<rho>\<^sub>s x\<^sub>s\<^sub>e = Some \<lbrace>Send_Evt x\<^sub>s\<^sub>c x\<^sub>m, \<rho>\<^sub>s\<^sub>e\<rbrace>"
-  and "\<rho>\<^sub>s\<^sub>e x\<^sub>s\<^sub>c = Some \<lbrace>c\<rbrace>"
+  and "\<rho>\<^sub>s x\<^sub>s\<^sub>e = Some (VClosure (Send_Evt x\<^sub>s\<^sub>c x\<^sub>m) \<rho>\<^sub>s\<^sub>e)"
+  and "\<rho>\<^sub>s\<^sub>e x\<^sub>s\<^sub>c = Some (VChan c)"
   and "\<rho>\<^sub>s\<^sub>e x\<^sub>m = Some \<omega>\<^sub>m"
   and "\<E> \<pi>\<^sub>r = Some (\<langle>LET x\<^sub>r = SYNC x\<^sub>r\<^sub>e in e\<^sub>r;\<rho>\<^sub>r;\<kappa>\<^sub>r\<rangle>)"
-  and "\<rho>\<^sub>r x\<^sub>r\<^sub>e = Some \<lbrace>Recv_Evt x\<^sub>r\<^sub>c, \<rho>\<^sub>r\<^sub>e\<rbrace>"
-  and "\<rho>\<^sub>r\<^sub>e x\<^sub>r\<^sub>c = Some \<lbrace>c\<rbrace>"
+  and "\<rho>\<^sub>r x\<^sub>r\<^sub>e = Some (VClosure (Recv_Evt x\<^sub>r\<^sub>c) \<rho>\<^sub>r\<^sub>e)"
+  and "\<rho>\<^sub>r\<^sub>e x\<^sub>r\<^sub>c = Some (VChan c)"
 
 
   from \<open>(\<V>, \<C>) \<Turnstile>\<^sub>\<E> \<E>\<close> and \<open>\<E> \<pi>\<^sub>s = Some (\<langle>LET x\<^sub>s = SYNC x\<^sub>s\<^sub>e in e\<^sub>s;\<rho>\<^sub>s;\<kappa>\<^sub>s\<rangle>)\<close> 
   have "(\<V>, \<C>) \<Turnstile>\<^sub>e e\<^sub>s" by (blast intro: static_eval_pool_to_exp_let)
 
   from \<open>(\<V>, \<C>) \<Turnstile>\<^sub>\<E> \<E>\<close> \<open>\<E> \<pi>\<^sub>s = Some (\<langle>LET x\<^sub>s = SYNC x\<^sub>s\<^sub>e in e\<^sub>s;\<rho>\<^sub>s;\<kappa>\<^sub>s\<rangle>)\<close> 
-  and \<open>\<rho>\<^sub>s x\<^sub>s\<^sub>e = Some \<lbrace>Send_Evt x\<^sub>s\<^sub>c x\<^sub>m, \<rho>\<^sub>s\<^sub>e\<rbrace>\<close> \<open>\<rho>\<^sub>s\<^sub>e x\<^sub>s\<^sub>c = Some \<lbrace>c\<rbrace>\<close> 
-  have "(\<V>, \<C>) \<Turnstile>\<^sub>\<rho> \<rho>\<^sub>s(x\<^sub>s \<mapsto> \<lbrace>\<rbrace>)" by (blast intro: static_eval_pool_to_env_let_sync_send)
+  and \<open>\<rho>\<^sub>s x\<^sub>s\<^sub>e = Some (VClosure (Send_Evt x\<^sub>s\<^sub>c x\<^sub>m) \<rho>\<^sub>s\<^sub>e)\<close> \<open>\<rho>\<^sub>s\<^sub>e x\<^sub>s\<^sub>c = Some (VChan c)\<close> 
+  have "(\<V>, \<C>) \<Turnstile>\<^sub>\<rho> \<rho>\<^sub>s(x\<^sub>s \<mapsto> VUnit)" by (blast intro: static_eval_pool_to_env_let_sync_send)
 
   from \<open>(\<V>, \<C>) \<Turnstile>\<^sub>\<E> \<E>\<close> and \<open>\<E> \<pi>\<^sub>s = Some (\<langle>LET x\<^sub>s = SYNC x\<^sub>s\<^sub>e in e\<^sub>s;\<rho>\<^sub>s;\<kappa>\<^sub>s\<rangle>)\<close>
   have  "(\<V>, \<C>) \<Turnstile>\<^sub>\<kappa> \<V> (\<lfloor>e\<^sub>s\<rfloor>) \<Rrightarrow> \<kappa>\<^sub>s" by (blast intro: static_eval_pool_to_stack_let)
 
-  from `(\<V>, \<C>) \<Turnstile>\<^sub>e e\<^sub>s` and `(\<V>, \<C>) \<Turnstile>\<^sub>\<rho> \<rho>\<^sub>s(x\<^sub>s \<mapsto> \<lbrace>\<rbrace>)` and `(\<V>, \<C>) \<Turnstile>\<^sub>\<kappa> \<V> (\<lfloor>e\<^sub>s\<rfloor>) \<Rrightarrow> \<kappa>\<^sub>s`
-  have "(\<V>, \<C>) \<Turnstile>\<^sub>\<sigma> \<langle>e\<^sub>s;\<rho>\<^sub>s(x\<^sub>s \<mapsto> \<lbrace>\<rbrace>);\<kappa>\<^sub>s\<rangle>" by (blast intro: static_eval_state.intros)
+  from `(\<V>, \<C>) \<Turnstile>\<^sub>e e\<^sub>s` and `(\<V>, \<C>) \<Turnstile>\<^sub>\<rho> \<rho>\<^sub>s(x\<^sub>s \<mapsto> VUnit)` and `(\<V>, \<C>) \<Turnstile>\<^sub>\<kappa> \<V> (\<lfloor>e\<^sub>s\<rfloor>) \<Rrightarrow> \<kappa>\<^sub>s`
+  have "(\<V>, \<C>) \<Turnstile>\<^sub>\<sigma> \<langle>e\<^sub>s;\<rho>\<^sub>s(x\<^sub>s \<mapsto> VUnit);\<kappa>\<^sub>s\<rangle>" by (blast intro: static_eval_state.intros)
 
   from \<open>(\<V>, \<C>) \<Turnstile>\<^sub>\<E> \<E>\<close> and \<open>\<E> \<pi>\<^sub>r = Some (\<langle>LET x\<^sub>r = SYNC x\<^sub>r\<^sub>e in e\<^sub>r;\<rho>\<^sub>r;\<kappa>\<^sub>r\<rangle>)\<close> 
   have "(\<V>, \<C>) \<Turnstile>\<^sub>e e\<^sub>r" by (blast intro: static_eval_pool_to_exp_let)
 
   from \<open>(\<V>, \<C>) \<Turnstile>\<^sub>\<E> \<E>\<close> 
   and \<open>\<E> \<pi>\<^sub>s = Some (\<langle>LET x\<^sub>s = SYNC x\<^sub>s\<^sub>e in e\<^sub>s;\<rho>\<^sub>s;\<kappa>\<^sub>s\<rangle>)\<close> 
-  and \<open>\<rho>\<^sub>s x\<^sub>s\<^sub>e = Some \<lbrace>Send_Evt x\<^sub>s\<^sub>c x\<^sub>m, \<rho>\<^sub>s\<^sub>e\<rbrace>\<close> 
-  and \<open>\<rho>\<^sub>s\<^sub>e x\<^sub>m = Some \<omega>\<^sub>m\<close> \<open>\<rho>\<^sub>s\<^sub>e x\<^sub>s\<^sub>c = Some \<lbrace>c\<rbrace>\<close>
+  and \<open>\<rho>\<^sub>s x\<^sub>s\<^sub>e = Some (VClosure (Send_Evt x\<^sub>s\<^sub>c x\<^sub>m) \<rho>\<^sub>s\<^sub>e)\<close> 
+  and \<open>\<rho>\<^sub>s\<^sub>e x\<^sub>m = Some \<omega>\<^sub>m\<close> \<open>\<rho>\<^sub>s\<^sub>e x\<^sub>s\<^sub>c = Some (VChan c)\<close>
   and \<open>\<E> \<pi>\<^sub>r = Some (\<langle>LET x\<^sub>r = SYNC x\<^sub>r\<^sub>e in e\<^sub>r;\<rho>\<^sub>r;\<kappa>\<^sub>r\<rangle>)\<close> 
-  and \<open>\<rho>\<^sub>r x\<^sub>r\<^sub>e = Some \<lbrace>Recv_Evt x\<^sub>r\<^sub>c, \<rho>\<^sub>r\<^sub>e\<rbrace>\<close> \<open>\<rho>\<^sub>r\<^sub>e x\<^sub>r\<^sub>c = Some \<lbrace>c\<rbrace>\<close> 
+  and \<open>\<rho>\<^sub>r x\<^sub>r\<^sub>e = Some (VClosure (Recv_Evt x\<^sub>r\<^sub>c) \<rho>\<^sub>r\<^sub>e)\<close> \<open>\<rho>\<^sub>r\<^sub>e x\<^sub>r\<^sub>c = Some (VChan c)\<close> 
   have "(\<V>, \<C>) \<Turnstile>\<^sub>\<rho> \<rho>\<^sub>r(x\<^sub>r \<mapsto> \<omega>\<^sub>m)" by (blast intro: static_eval_pool_to_env_let_sync_recv)
 
   from \<open>(\<V>, \<C>) \<Turnstile>\<^sub>\<E> \<E>\<close> and \<open>\<E> \<pi>\<^sub>r = Some (\<langle>LET x\<^sub>r = SYNC x\<^sub>r\<^sub>e in e\<^sub>r;\<rho>\<^sub>r;\<kappa>\<^sub>r\<rangle>)\<close>
@@ -1232,12 +1231,12 @@ proof
   {
     fix \<pi> \<sigma>
     assume  "\<pi> \<noteq> \<pi>\<^sub>s ;;(LNext x\<^sub>s)" and "\<pi> \<noteq> \<pi>\<^sub>r ;; (LNext x\<^sub>r)"
-    and "(\<E>(\<pi>\<^sub>s ;;(LNext x\<^sub>s) \<mapsto> \<langle>e\<^sub>s;\<rho>\<^sub>s(x\<^sub>s \<mapsto> \<lbrace>\<rbrace>);\<kappa>\<^sub>s\<rangle>, \<pi>\<^sub>r ;; (LNext x\<^sub>r) \<mapsto> \<langle>e\<^sub>r;\<rho>\<^sub>r(x\<^sub>r \<mapsto> \<omega>\<^sub>m);\<kappa>\<^sub>r\<rangle>)) \<pi> = Some \<sigma>" then
+    and "(\<E>(\<pi>\<^sub>s ;;(LNext x\<^sub>s) \<mapsto> \<langle>e\<^sub>s;\<rho>\<^sub>s(x\<^sub>s \<mapsto> VUnit);\<kappa>\<^sub>s\<rangle>, \<pi>\<^sub>r ;; (LNext x\<^sub>r) \<mapsto> \<langle>e\<^sub>r;\<rho>\<^sub>r(x\<^sub>r \<mapsto> \<omega>\<^sub>m);\<kappa>\<^sub>r\<rangle>)) \<pi> = Some \<sigma>" then
     have "\<E> \<pi> = Some \<sigma>" by simp
     with \<open>(\<V>, \<C>) \<Turnstile>\<^sub>\<E> \<E>\<close>
     have "(\<V>, \<C>) \<Turnstile>\<^sub>\<sigma> \<sigma>" by (blast intro: static_eval_pool.cases)
-  } with `(\<V>, \<C>) \<Turnstile>\<^sub>\<sigma> \<langle>e\<^sub>r;\<rho>\<^sub>r (x\<^sub>r \<mapsto> \<omega>\<^sub>m);\<kappa>\<^sub>r\<rangle>` `(\<V>, \<C>) \<Turnstile>\<^sub>\<sigma> \<langle>e\<^sub>s;\<rho>\<^sub>s (x\<^sub>s \<mapsto> \<lbrace>\<rbrace>);\<kappa>\<^sub>s\<rangle>`
-  show "\<forall>\<pi> \<sigma>. (\<E>(\<pi>\<^sub>s ;; (LNext x\<^sub>s) \<mapsto> \<langle>e\<^sub>s;\<rho>\<^sub>s(x\<^sub>s \<mapsto> \<lbrace>\<rbrace>);\<kappa>\<^sub>s\<rangle>, \<pi>\<^sub>r ;;(LNext x\<^sub>r) \<mapsto> \<langle>e\<^sub>r;\<rho>\<^sub>r(x\<^sub>r \<mapsto> \<omega>\<^sub>m);\<kappa>\<^sub>r\<rangle>)) \<pi> = Some \<sigma> \<longrightarrow> (\<V>, \<C>) \<Turnstile>\<^sub>\<sigma> \<sigma>" by simp
+  } with `(\<V>, \<C>) \<Turnstile>\<^sub>\<sigma> \<langle>e\<^sub>r;\<rho>\<^sub>r (x\<^sub>r \<mapsto> \<omega>\<^sub>m);\<kappa>\<^sub>r\<rangle>` `(\<V>, \<C>) \<Turnstile>\<^sub>\<sigma> \<langle>e\<^sub>s;\<rho>\<^sub>s (x\<^sub>s \<mapsto> VUnit);\<kappa>\<^sub>s\<rangle>`
+  show "\<forall>\<pi> \<sigma>. (\<E>(\<pi>\<^sub>s ;; (LNext x\<^sub>s) \<mapsto> \<langle>e\<^sub>s;\<rho>\<^sub>s(x\<^sub>s \<mapsto> VUnit);\<kappa>\<^sub>s\<rangle>, \<pi>\<^sub>r ;;(LNext x\<^sub>r) \<mapsto> \<langle>e\<^sub>r;\<rho>\<^sub>r(x\<^sub>r \<mapsto> \<omega>\<^sub>m);\<kappa>\<^sub>r\<rangle>)) \<pi> = Some \<sigma> \<longrightarrow> (\<V>, \<C>) \<Turnstile>\<^sub>\<sigma> \<sigma>" by simp
 
 qed
 
@@ -1245,83 +1244,83 @@ qed
 lemma static_eval_pool_to_env_let_chan: "
   (\<V>, \<C>) \<Turnstile>\<^sub>\<E> \<E> \<Longrightarrow>
   \<E> \<pi> = Some (\<langle>LET x = CHAN \<lparr>\<rparr> in e; \<rho>; \<kappa>\<rangle>) \<Longrightarrow> 
-  (\<V>, \<C>) \<Turnstile>\<^sub>\<rho> \<rho>(x \<mapsto> \<lbrace>Ch \<pi> x\<rbrace>)
+  (\<V>, \<C>) \<Turnstile>\<^sub>\<rho> \<rho>(x \<mapsto> (VChan (Ch \<pi> x)))
 "
 proof
   assume "(\<V>, \<C>) \<Turnstile>\<^sub>\<E> \<E>" and "\<E> \<pi> = Some (\<langle>LET x = CHAN \<lparr>\<rparr> in e; \<rho>; \<kappa>\<rangle>)" then
   have "(\<V>, \<C>) \<Turnstile>\<^sub>\<sigma> \<langle>LET x = CHAN \<lparr>\<rparr> in e; \<rho>; \<kappa>\<rangle>" by (blast intro: static_eval_pool.cases) then
   have "(\<V>, \<C>) \<Turnstile>\<^sub>e LET x = CHAN \<lparr>\<rparr> in e" by (blast intro: static_eval_state.cases) then
   have "{^Chan x} \<subseteq> \<V> x"  by (blast intro: static_eval.cases)
-  have "(\<V>, \<C>) \<Turnstile>\<^sub>\<omega> \<lbrace>Ch \<pi> x\<rbrace>" by (simp add: Chan)
+  have "(\<V>, \<C>) \<Turnstile>\<^sub>\<omega> (VChan (Ch \<pi> x))" by (simp add: Chan)
 
   from `(\<V>, \<C>) \<Turnstile>\<^sub>\<sigma> \<langle>LET x = CHAN \<lparr>\<rparr> in e; \<rho>; \<kappa>\<rangle>` 
   have "(\<V>, \<C>) \<Turnstile>\<^sub>\<rho> \<rho>" by (simp add: static_eval_state.simps)+
   {
     fix x' \<omega>'
-    assume "(\<rho>(x \<mapsto> \<lbrace>Ch \<pi> x\<rbrace>)) x' = Some \<omega>'" and "x \<noteq> x'"then
+    assume "(\<rho>(x \<mapsto> (VChan (Ch \<pi> x)))) x' = Some \<omega>'" and "x \<noteq> x'"then
     have "\<rho> x' = Some \<omega>'" by simp with `(\<V>, \<C>) \<Turnstile>\<^sub>\<rho> \<rho>`
     have "{|\<omega>'|} \<subseteq> \<V> x' \<and> (\<V>, \<C>) \<Turnstile>\<^sub>\<omega> \<omega>'" by (simp add: static_eval_env.simps)
-  } with `{^Chan x} \<subseteq> \<V> x` and `(\<V>, \<C>) \<Turnstile>\<^sub>\<omega> \<lbrace>Ch \<pi> x\<rbrace>`
-  show "\<forall>x' \<omega>'. (\<rho>(x \<mapsto> \<lbrace>Ch \<pi> x\<rbrace>)) x' = Some \<omega>' \<longrightarrow> {|\<omega>'|} \<subseteq> \<V> x' \<and> (\<V>, \<C>) \<Turnstile>\<^sub>\<omega> \<omega>'" by simp
+  } with `{^Chan x} \<subseteq> \<V> x` and `(\<V>, \<C>) \<Turnstile>\<^sub>\<omega> (VChan (Ch \<pi> x))`
+  show "\<forall>x' \<omega>'. (\<rho>(x \<mapsto> (VChan (Ch \<pi> x)))) x' = Some \<omega>' \<longrightarrow> {|\<omega>'|} \<subseteq> \<V> x' \<and> (\<V>, \<C>) \<Turnstile>\<^sub>\<omega> \<omega>'" by simp
 qed
 
 
 lemma static_eval_preserved_under_chan: "
   (\<V>, \<C>) \<Turnstile>\<^sub>\<E> \<E> \<Longrightarrow>
   \<E> \<pi> = Some (\<langle>LET x = CHAN \<lparr>\<rparr> in e; \<rho>; \<kappa>\<rangle>) \<Longrightarrow> 
-  (\<V>, \<C>) \<Turnstile>\<^sub>\<E> \<E>(\<pi> ;;(LNext x) \<mapsto> \<langle>e; \<rho>(x \<mapsto> \<lbrace>Ch \<pi> x\<rbrace>); \<kappa>\<rangle>)
+  (\<V>, \<C>) \<Turnstile>\<^sub>\<E> \<E>(\<pi> ;;(LNext x) \<mapsto> \<langle>e; \<rho>(x \<mapsto> (VChan (Ch \<pi> x))); \<kappa>\<rangle>)
 "
 proof
   assume "(\<V>, \<C>) \<Turnstile>\<^sub>\<E> \<E>" and "\<E> \<pi> = Some (\<langle>LET x = CHAN \<lparr>\<rparr> in e; \<rho>; \<kappa>\<rangle>)" then
   have "(\<V>, \<C>) \<Turnstile>\<^sub>e e" by (blast intro: static_eval_pool_to_exp_let)
 
   from `(\<V>, \<C>) \<Turnstile>\<^sub>\<E> \<E>` and `\<E> \<pi> = Some (\<langle>LET x = CHAN \<lparr>\<rparr> in e; \<rho>; \<kappa>\<rangle>)`
-  have "(\<V>, \<C>) \<Turnstile>\<^sub>\<rho> \<rho>(x \<mapsto> \<lbrace>Ch \<pi> x\<rbrace>)" by (blast intro: static_eval_pool_to_env_let_chan )
+  have "(\<V>, \<C>) \<Turnstile>\<^sub>\<rho> \<rho>(x \<mapsto> (VChan (Ch \<pi> x)))" by (blast intro: static_eval_pool_to_env_let_chan )
 
   from `(\<V>, \<C>) \<Turnstile>\<^sub>\<E> \<E>` and `\<E> \<pi> = Some (\<langle>LET x = CHAN \<lparr>\<rparr> in e; \<rho>; \<kappa>\<rangle>)`
   have "(\<V>, \<C>) \<Turnstile>\<^sub>\<kappa> \<V> (\<lfloor>e\<rfloor>) \<Rrightarrow> \<kappa>" by (blast intro: static_eval_pool_to_stack_let)
 
-  from `(\<V>, \<C>) \<Turnstile>\<^sub>e e` and `(\<V>, \<C>) \<Turnstile>\<^sub>\<rho> \<rho>(x \<mapsto> \<lbrace>Ch \<pi> x\<rbrace>)` and `(\<V>, \<C>) \<Turnstile>\<^sub>\<kappa> \<V> (\<lfloor>e\<rfloor>) \<Rrightarrow> \<kappa>`
-  have "(\<V>, \<C>) \<Turnstile>\<^sub>\<sigma> \<langle>e;\<rho>(x \<mapsto> \<lbrace>Ch \<pi> x\<rbrace>);\<kappa>\<rangle>" by (blast intro: static_eval_state.intros)
+  from `(\<V>, \<C>) \<Turnstile>\<^sub>e e` and `(\<V>, \<C>) \<Turnstile>\<^sub>\<rho> \<rho>(x \<mapsto> (VChan (Ch \<pi> x)))` and `(\<V>, \<C>) \<Turnstile>\<^sub>\<kappa> \<V> (\<lfloor>e\<rfloor>) \<Rrightarrow> \<kappa>`
+  have "(\<V>, \<C>) \<Turnstile>\<^sub>\<sigma> \<langle>e;\<rho>(x \<mapsto> (VChan (Ch \<pi> x)));\<kappa>\<rangle>" by (blast intro: static_eval_state.intros)
   {
     fix \<pi>' \<sigma>'
-    assume "(\<E>(\<pi> ;;(LNext x) \<mapsto> \<langle>e;\<rho>(x \<mapsto> \<lbrace>Ch \<pi> x\<rbrace>);\<kappa>\<rangle>)) \<pi>' = Some \<sigma>'" 
+    assume "(\<E>(\<pi> ;;(LNext x) \<mapsto> \<langle>e;\<rho>(x \<mapsto> (VChan (Ch \<pi> x)));\<kappa>\<rangle>)) \<pi>' = Some \<sigma>'" 
     and "\<pi>' \<noteq> \<pi> ;;(LNext x)" then
     have "\<E> \<pi>' = Some \<sigma>'" by simp with `(\<V>, \<C>) \<Turnstile>\<^sub>\<E> \<E>`
     have "(\<V>, \<C>) \<Turnstile>\<^sub>\<sigma> \<sigma>'" by (simp add: static_eval_pool.simps)
-  } with `(\<V>, \<C>) \<Turnstile>\<^sub>\<sigma> \<langle>e;\<rho>(x \<mapsto> \<lbrace>Ch \<pi> x\<rbrace>);\<kappa>\<rangle>`
-  show "\<forall>\<pi>' \<sigma>'. (\<E>(\<pi> ;;(LNext x) \<mapsto> \<langle>e;\<rho>(x \<mapsto> \<lbrace>Ch \<pi> x\<rbrace>);\<kappa>\<rangle>)) \<pi>' = Some \<sigma>' \<longrightarrow> (\<V>, \<C>) \<Turnstile>\<^sub>\<sigma> \<sigma>'" by simp
+  } with `(\<V>, \<C>) \<Turnstile>\<^sub>\<sigma> \<langle>e;\<rho>(x \<mapsto> (VChan (Ch \<pi> x)));\<kappa>\<rangle>`
+  show "\<forall>\<pi>' \<sigma>'. (\<E>(\<pi> ;;(LNext x) \<mapsto> \<langle>e;\<rho>(x \<mapsto> (VChan (Ch \<pi> x)));\<kappa>\<rangle>)) \<pi>' = Some \<sigma>' \<longrightarrow> (\<V>, \<C>) \<Turnstile>\<^sub>\<sigma> \<sigma>'" by simp
 qed
 
 
 lemma static_eval_pool_to_env_let_spawn: "
   (\<V>, \<C>) \<Turnstile>\<^sub>\<E> \<E> \<Longrightarrow>
   \<E> \<pi> = Some (\<langle>LET x = SPAWN e\<^sub>c in e; \<rho>; \<kappa>\<rangle>) \<Longrightarrow> 
-  (\<V>, \<C>) \<Turnstile>\<^sub>\<rho> \<rho>(x \<mapsto> \<lbrace>\<rbrace>)"
+  (\<V>, \<C>) \<Turnstile>\<^sub>\<rho> \<rho>(x \<mapsto> VUnit)"
 proof
 
   assume "(\<V>, \<C>) \<Turnstile>\<^sub>\<E> \<E>" and "\<E> \<pi> = Some (\<langle>LET x = SPAWN e\<^sub>c in e; \<rho>; \<kappa>\<rangle>)" then
   have "(\<V>, \<C>) \<Turnstile>\<^sub>\<sigma> \<langle>LET x = SPAWN e\<^sub>c in e; \<rho>; \<kappa>\<rangle>" by (simp add: static_eval_pool.simps) then
   have "(\<V>, \<C>) \<Turnstile>\<^sub>e LET x = SPAWN e\<^sub>c in e" by (blast intro: static_eval_state.cases) then
   have "{^\<lparr>\<rparr>} \<subseteq> \<V> x"  by (blast intro: static_eval.cases) then
-  have "(\<V>, \<C>) \<Turnstile>\<^sub>\<omega> \<lbrace>\<rbrace>" by (simp add: Unit)
+  have "(\<V>, \<C>) \<Turnstile>\<^sub>\<omega> VUnit" by (simp add: Unit)
 
   from `(\<V>, \<C>) \<Turnstile>\<^sub>\<sigma> \<langle>LET x = SPAWN e\<^sub>c in e; \<rho>; \<kappa>\<rangle>` 
   have "(\<V>, \<C>) \<Turnstile>\<^sub>\<rho> \<rho>" by (simp add: static_eval_state.simps)
 
   {
     fix x' \<omega>'
-    assume "(\<rho>(x \<mapsto> \<lbrace>\<rbrace>)) x' = Some \<omega>'" and "x \<noteq> x'" then
+    assume "(\<rho>(x \<mapsto> VUnit)) x' = Some \<omega>'" and "x \<noteq> x'" then
     have "\<rho> x' = Some \<omega>'" by simp with `(\<V>, \<C>) \<Turnstile>\<^sub>\<rho> \<rho>`
     have "{|\<omega>'|} \<subseteq> \<V> x' \<and> (\<V>, \<C>) \<Turnstile>\<^sub>\<omega> \<omega>'" by (blast intro: static_eval_env.cases)
-  } with `{^\<lparr>\<rparr>} \<subseteq> \<V> x` and `(\<V>, \<C>) \<Turnstile>\<^sub>\<omega> \<lbrace>\<rbrace>`
-  show "\<forall>x' \<omega>'. (\<rho>(x \<mapsto> \<lbrace>\<rbrace>)) x' = Some \<omega>' \<longrightarrow> {|\<omega>'|} \<subseteq> \<V> x' \<and> (\<V>, \<C>) \<Turnstile>\<^sub>\<omega> \<omega>'" by simp
+  } with `{^\<lparr>\<rparr>} \<subseteq> \<V> x` and `(\<V>, \<C>) \<Turnstile>\<^sub>\<omega> VUnit`
+  show "\<forall>x' \<omega>'. (\<rho>(x \<mapsto> VUnit)) x' = Some \<omega>' \<longrightarrow> {|\<omega>'|} \<subseteq> \<V> x' \<and> (\<V>, \<C>) \<Turnstile>\<^sub>\<omega> \<omega>'" by simp
 qed
 
 lemma static_eval_preserved_under_spawn: "
   (\<V>, \<C>) \<Turnstile>\<^sub>\<E> \<E> \<Longrightarrow>
   \<E> \<pi> = Some (\<langle>LET x = SPAWN e\<^sub>c in e; \<rho>; \<kappa>\<rangle>) \<Longrightarrow> 
-  (\<V>, \<C>) \<Turnstile>\<^sub>\<E> \<E>(\<pi> ;;(LNext x) \<mapsto> \<langle>e; \<rho>(x \<mapsto> \<lbrace>\<rbrace>); \<kappa>\<rangle>, \<pi>;;(LSpawn x) \<mapsto> \<langle>e\<^sub>c; \<rho>; []\<rangle>)
+  (\<V>, \<C>) \<Turnstile>\<^sub>\<E> \<E>(\<pi> ;;(LNext x) \<mapsto> \<langle>e; \<rho>(x \<mapsto> VUnit); \<kappa>\<rangle>, \<pi>;;(LSpawn x) \<mapsto> \<langle>e\<^sub>c; \<rho>; []\<rangle>)
 "
 proof
 
@@ -1331,13 +1330,13 @@ proof
   have "(\<V>, \<C>) \<Turnstile>\<^sub>e e" by (blast intro: static_eval_pool_to_exp_let)
 
   from `(\<V>, \<C>) \<Turnstile>\<^sub>\<E> \<E>` and `\<E> \<pi> = Some (\<langle>LET x = SPAWN e\<^sub>c in e; \<rho>; \<kappa>\<rangle>)`
-  have "(\<V>, \<C>) \<Turnstile>\<^sub>\<rho> \<rho>(x \<mapsto> \<lbrace>\<rbrace>)" by (blast intro: static_eval_pool_to_env_let_spawn)
+  have "(\<V>, \<C>) \<Turnstile>\<^sub>\<rho> \<rho>(x \<mapsto> VUnit)" by (blast intro: static_eval_pool_to_env_let_spawn)
 
   from `(\<V>, \<C>) \<Turnstile>\<^sub>\<E> \<E>` and `\<E> \<pi> = Some (\<langle>LET x = SPAWN e\<^sub>c in e; \<rho>; \<kappa>\<rangle>)`
   have "(\<V>, \<C>) \<Turnstile>\<^sub>\<kappa> \<V> (\<lfloor>e\<rfloor>) \<Rrightarrow> \<kappa>" by (blast intro: static_eval_pool_to_stack_let)
 
-  from \<open>(\<V>, \<C>) \<Turnstile>\<^sub>\<kappa> \<V> (\<lfloor>e\<rfloor>) \<Rrightarrow> \<kappa>\<close> \<open>(\<V>, \<C>) \<Turnstile>\<^sub>\<rho> \<rho>(x \<mapsto> \<lbrace>\<rbrace>)\<close> \<open>(\<V>, \<C>) \<Turnstile>\<^sub>e e\<close>
-  have "(\<V>, \<C>) \<Turnstile>\<^sub>\<sigma> \<langle>e;\<rho>(x \<mapsto> \<lbrace>\<rbrace>);\<kappa>\<rangle>" by (simp add: static_eval_state.intros)
+  from \<open>(\<V>, \<C>) \<Turnstile>\<^sub>\<kappa> \<V> (\<lfloor>e\<rfloor>) \<Rrightarrow> \<kappa>\<close> \<open>(\<V>, \<C>) \<Turnstile>\<^sub>\<rho> \<rho>(x \<mapsto> VUnit)\<close> \<open>(\<V>, \<C>) \<Turnstile>\<^sub>e e\<close>
+  have "(\<V>, \<C>) \<Turnstile>\<^sub>\<sigma> \<langle>e;\<rho>(x \<mapsto> VUnit);\<kappa>\<rangle>" by (simp add: static_eval_state.intros)
 
   from `(\<V>, \<C>) \<Turnstile>\<^sub>\<E> \<E>` and `\<E> \<pi> = Some (\<langle>LET x = SPAWN e\<^sub>c in e; \<rho>; \<kappa>\<rangle>)`
   have "(\<V>, \<C>) \<Turnstile>\<^sub>\<sigma> \<langle>LET x = SPAWN e\<^sub>c in e; \<rho>; \<kappa>\<rangle>" by (simp add: static_eval_pool.simps) then
@@ -1352,12 +1351,12 @@ proof
 
   {
     fix \<pi>' \<sigma>'
-    assume "(\<E>(\<pi> ;;(LNext x) \<mapsto> \<langle>e;\<rho>(x \<mapsto> \<lbrace>\<rbrace>);\<kappa>\<rangle>, \<pi> ;; (LSpawn x) \<mapsto> \<langle>e\<^sub>c;\<rho>;[]\<rangle>)) \<pi>' = Some \<sigma>'"
+    assume "(\<E>(\<pi> ;;(LNext x) \<mapsto> \<langle>e;\<rho>(x \<mapsto> VUnit);\<kappa>\<rangle>, \<pi> ;; (LSpawn x) \<mapsto> \<langle>e\<^sub>c;\<rho>;[]\<rangle>)) \<pi>' = Some \<sigma>'"
     and "\<pi>' \<noteq> \<pi> ;; (LNext x)" and " \<pi>' \<noteq> \<pi> ;; (LSpawn x)" then
     have "\<E> \<pi>' = Some \<sigma>'" by simp with `(\<V>, \<C>) \<Turnstile>\<^sub>\<E> \<E>`
     have "(\<V>, \<C>) \<Turnstile>\<^sub>\<sigma> \<sigma>'" by (blast intro: static_eval_pool.cases)
-  } with `(\<V>, \<C>) \<Turnstile>\<^sub>\<sigma> \<langle>e;\<rho>(x \<mapsto> \<lbrace>\<rbrace>);\<kappa>\<rangle>` and `(\<V>, \<C>) \<Turnstile>\<^sub>\<sigma> \<langle>e\<^sub>c;\<rho>;[]\<rangle>`
-  show "\<forall>\<pi>' \<sigma>'. (\<E>(\<pi> ;; (LNext x) \<mapsto> \<langle>e;\<rho>(x \<mapsto> \<lbrace>\<rbrace>);\<kappa>\<rangle>, \<pi> ;; (LSpawn x) \<mapsto> \<langle>e\<^sub>c;\<rho>;[]\<rangle>)) \<pi>' = Some \<sigma>' \<longrightarrow> (\<V>, \<C>) \<Turnstile>\<^sub>\<sigma> \<sigma>'" by simp
+  } with `(\<V>, \<C>) \<Turnstile>\<^sub>\<sigma> \<langle>e;\<rho>(x \<mapsto> VUnit);\<kappa>\<rangle>` and `(\<V>, \<C>) \<Turnstile>\<^sub>\<sigma> \<langle>e\<^sub>c;\<rho>;[]\<rangle>`
+  show "\<forall>\<pi>' \<sigma>'. (\<E>(\<pi> ;; (LNext x) \<mapsto> \<langle>e;\<rho>(x \<mapsto> VUnit);\<kappa>\<rangle>, \<pi> ;; (LSpawn x) \<mapsto> \<langle>e\<^sub>c;\<rho>;[]\<rangle>)) \<pi>' = Some \<sigma>' \<longrightarrow> (\<V>, \<C>) \<Turnstile>\<^sub>\<sigma> \<sigma>'" by simp
 qed
 
 
@@ -1401,36 +1400,36 @@ proof -
     show "(\<V>, \<C>) \<Turnstile>\<^sub>\<E> \<E>'" by simp
   next
     case (Let_Chan \<pi> x e \<rho> \<kappa>)
-    assume "\<E>' = \<E> ++ [\<pi> ;; (LNext x) \<mapsto> \<langle>e;\<rho> ++ [x \<mapsto> \<lbrace>Ch \<pi> x\<rbrace>];\<kappa>\<rangle>]"
+    assume "\<E>' = \<E> ++ [\<pi> ;; (LNext x) \<mapsto> \<langle>e;\<rho> ++ [x \<mapsto> (VChan (Ch \<pi> x))];\<kappa>\<rangle>]"
     assume "leaf \<E> \<pi>" and "\<E> \<pi> = Some (\<langle>LET x = CHAN \<lparr>\<rparr> in e;\<rho>;\<kappa>\<rangle>)"
     with \<open>(\<V>, \<C>) \<Turnstile>\<^sub>\<E> \<E>\<close>
-    have "(\<V>, \<C>) \<Turnstile>\<^sub>\<E> \<E>(\<pi> ;; (LNext x) \<mapsto> \<langle>e;\<rho> ++ [x \<mapsto> \<lbrace>Ch \<pi> x\<rbrace>];\<kappa>\<rangle>)" by (simp add: static_eval_preserved_under_chan)
-    with \<open>\<E>' = \<E> ++ [\<pi> ;; (LNext x) \<mapsto> \<langle>e;\<rho> ++ [x \<mapsto> \<lbrace>Ch \<pi> x\<rbrace>];\<kappa>\<rangle>]\<close>
+    have "(\<V>, \<C>) \<Turnstile>\<^sub>\<E> \<E>(\<pi> ;; (LNext x) \<mapsto> \<langle>e;\<rho> ++ [x \<mapsto> (VChan (Ch \<pi> x))];\<kappa>\<rangle>)" by (simp add: static_eval_preserved_under_chan)
+    with \<open>\<E>' = \<E> ++ [\<pi> ;; (LNext x) \<mapsto> \<langle>e;\<rho> ++ [x \<mapsto> (VChan (Ch \<pi> x))];\<kappa>\<rangle>]\<close>
     show "(\<V>, \<C>) \<Turnstile>\<^sub>\<E> \<E>'" by simp
   next
     case (Let_Spawn \<pi> x e\<^sub>c e \<rho> \<kappa>)
-    assume "\<E>' = \<E> ++ [\<pi> ;; (LNext x) \<mapsto> \<langle>e;\<rho> ++ [x \<mapsto> \<lbrace>\<rbrace>];\<kappa>\<rangle>, \<pi> ;; (LSpawn x) \<mapsto> \<langle>e\<^sub>c;\<rho>;[]\<rangle>]"
+    assume "\<E>' = \<E> ++ [\<pi> ;; (LNext x) \<mapsto> \<langle>e;\<rho> ++ [x \<mapsto> VUnit];\<kappa>\<rangle>, \<pi> ;; (LSpawn x) \<mapsto> \<langle>e\<^sub>c;\<rho>;[]\<rangle>]"
     assume "leaf \<E> \<pi>" and "\<E> \<pi> = Some (\<langle>LET x = SPAWN e\<^sub>c in e;\<rho>;\<kappa>\<rangle>)"
     with \<open>(\<V>, \<C>) \<Turnstile>\<^sub>\<E> \<E>\<close>
-    have "(\<V>, \<C>) \<Turnstile>\<^sub>\<E> \<E>(\<pi> ;; (LNext x) \<mapsto> \<langle>e;\<rho> ++ [x \<mapsto> \<lbrace>\<rbrace>];\<kappa>\<rangle>, \<pi> ;; (LSpawn x) \<mapsto> \<langle>e\<^sub>c;\<rho>;[]\<rangle>)" by (simp add: static_eval_preserved_under_spawn)
-    with \<open>\<E>' = \<E> ++ [\<pi> ;; (LNext x) \<mapsto> \<langle>e;\<rho> ++ [x \<mapsto> \<lbrace>\<rbrace>];\<kappa>\<rangle>, \<pi> ;; (LSpawn x) \<mapsto> \<langle>e\<^sub>c;\<rho>;[]\<rangle>]\<close>
+    have "(\<V>, \<C>) \<Turnstile>\<^sub>\<E> \<E>(\<pi> ;; (LNext x) \<mapsto> \<langle>e;\<rho> ++ [x \<mapsto> VUnit];\<kappa>\<rangle>, \<pi> ;; (LSpawn x) \<mapsto> \<langle>e\<^sub>c;\<rho>;[]\<rangle>)" by (simp add: static_eval_preserved_under_spawn)
+    with \<open>\<E>' = \<E> ++ [\<pi> ;; (LNext x) \<mapsto> \<langle>e;\<rho> ++ [x \<mapsto> VUnit];\<kappa>\<rangle>, \<pi> ;; (LSpawn x) \<mapsto> \<langle>e\<^sub>c;\<rho>;[]\<rangle>]\<close>
     show "(\<V>, \<C>) \<Turnstile>\<^sub>\<E> \<E>'" by simp
   next
     case (Let_Sync \<pi>\<^sub>s x\<^sub>s x\<^sub>s\<^sub>e e\<^sub>s \<rho>\<^sub>s \<kappa>\<^sub>s x\<^sub>s\<^sub>c x\<^sub>m \<rho>\<^sub>s\<^sub>e \<pi>\<^sub>r x\<^sub>r x\<^sub>r\<^sub>e e\<^sub>r \<rho>\<^sub>r \<kappa>\<^sub>r x\<^sub>r\<^sub>c \<rho>\<^sub>r\<^sub>e c \<omega>\<^sub>m)
-    assume "\<E>' = \<E> ++ [\<pi>\<^sub>s ;; (LNext x\<^sub>s) \<mapsto> \<langle>e\<^sub>s;\<rho>\<^sub>s ++ [x\<^sub>s \<mapsto> \<lbrace>\<rbrace>];\<kappa>\<^sub>s\<rangle>, \<pi>\<^sub>r ;; (LNext x\<^sub>r) \<mapsto> \<langle>e\<^sub>r;\<rho>\<^sub>r ++ [x\<^sub>r \<mapsto> \<omega>\<^sub>m];\<kappa>\<^sub>r\<rangle>]"
+    assume "\<E>' = \<E> ++ [\<pi>\<^sub>s ;; (LNext x\<^sub>s) \<mapsto> \<langle>e\<^sub>s;\<rho>\<^sub>s ++ [x\<^sub>s \<mapsto> VUnit];\<kappa>\<^sub>s\<rangle>, \<pi>\<^sub>r ;; (LNext x\<^sub>r) \<mapsto> \<langle>e\<^sub>r;\<rho>\<^sub>r ++ [x\<^sub>r \<mapsto> \<omega>\<^sub>m];\<kappa>\<^sub>r\<rangle>]"
 
     assume "leaf \<E> \<pi>\<^sub>s"
     and "\<E> \<pi>\<^sub>s = Some (\<langle>LET x\<^sub>s = SYNC x\<^sub>s\<^sub>e in e\<^sub>s;\<rho>\<^sub>s;\<kappa>\<^sub>s\<rangle>)"
-    and "\<rho>\<^sub>s x\<^sub>s\<^sub>e = Some \<lbrace>Send_Evt x\<^sub>s\<^sub>c x\<^sub>m, \<rho>\<^sub>s\<^sub>e\<rbrace>"
+    and "\<rho>\<^sub>s x\<^sub>s\<^sub>e = Some (VClosure (Send_Evt x\<^sub>s\<^sub>c x\<^sub>m) \<rho>\<^sub>s\<^sub>e)"
     and "leaf \<E> \<pi>\<^sub>r"
     and "\<E> \<pi>\<^sub>r = Some (\<langle>LET x\<^sub>r = SYNC x\<^sub>r\<^sub>e in e\<^sub>r;\<rho>\<^sub>r;\<kappa>\<^sub>r\<rangle>)"
-    and "\<rho>\<^sub>r x\<^sub>r\<^sub>e = Some \<lbrace>Recv_Evt x\<^sub>r\<^sub>c, \<rho>\<^sub>r\<^sub>e\<rbrace>"
-    and "\<rho>\<^sub>s\<^sub>e x\<^sub>s\<^sub>c = Some \<lbrace>c\<rbrace>"
-    and "\<rho>\<^sub>r\<^sub>e x\<^sub>r\<^sub>c = Some \<lbrace>c\<rbrace>"
+    and "\<rho>\<^sub>r x\<^sub>r\<^sub>e = Some (VClosure (Recv_Evt x\<^sub>r\<^sub>c) \<rho>\<^sub>r\<^sub>e)"
+    and "\<rho>\<^sub>s\<^sub>e x\<^sub>s\<^sub>c = Some (VChan c)"
+    and "\<rho>\<^sub>r\<^sub>e x\<^sub>r\<^sub>c = Some (VChan c)"
     and "\<rho>\<^sub>s\<^sub>e x\<^sub>m = Some \<omega>\<^sub>m"
     with \<open>(\<V>, \<C>) \<Turnstile>\<^sub>\<E> \<E>\<close>
-    have "(\<V>, \<C>) \<Turnstile>\<^sub>\<E> \<E>(\<pi>\<^sub>s ;; (LNext x\<^sub>s) \<mapsto> \<langle>e\<^sub>s;\<rho>\<^sub>s ++ [x\<^sub>s \<mapsto> \<lbrace>\<rbrace>];\<kappa>\<^sub>s\<rangle>, \<pi>\<^sub>r ;; (LNext x\<^sub>r) \<mapsto> \<langle>e\<^sub>r;\<rho>\<^sub>r ++ [x\<^sub>r \<mapsto> \<omega>\<^sub>m];\<kappa>\<^sub>r\<rangle>)" by (simp add: static_eval_preserved_under_sync)
-    with \<open>\<E>' = \<E> ++ [\<pi>\<^sub>s ;; (LNext x\<^sub>s) \<mapsto> \<langle>e\<^sub>s;\<rho>\<^sub>s ++ [x\<^sub>s \<mapsto> \<lbrace>\<rbrace>];\<kappa>\<^sub>s\<rangle>, \<pi>\<^sub>r ;; (LNext x\<^sub>r) \<mapsto> \<langle>e\<^sub>r;\<rho>\<^sub>r ++ [x\<^sub>r \<mapsto> \<omega>\<^sub>m];\<kappa>\<^sub>r\<rangle>]\<close>
+    have "(\<V>, \<C>) \<Turnstile>\<^sub>\<E> \<E>(\<pi>\<^sub>s ;; (LNext x\<^sub>s) \<mapsto> \<langle>e\<^sub>s;\<rho>\<^sub>s ++ [x\<^sub>s \<mapsto> VUnit];\<kappa>\<^sub>s\<rangle>, \<pi>\<^sub>r ;; (LNext x\<^sub>r) \<mapsto> \<langle>e\<^sub>r;\<rho>\<^sub>r ++ [x\<^sub>r \<mapsto> \<omega>\<^sub>m];\<kappa>\<^sub>r\<rangle>)" by (simp add: static_eval_preserved_under_sync)
+    with \<open>\<E>' = \<E> ++ [\<pi>\<^sub>s ;; (LNext x\<^sub>s) \<mapsto> \<langle>e\<^sub>s;\<rho>\<^sub>s ++ [x\<^sub>s \<mapsto> VUnit];\<kappa>\<^sub>s\<rangle>, \<pi>\<^sub>r ;; (LNext x\<^sub>r) \<mapsto> \<langle>e\<^sub>r;\<rho>\<^sub>r ++ [x\<^sub>r \<mapsto> \<omega>\<^sub>m];\<kappa>\<^sub>r\<rangle>]\<close>
     show "(\<V>, \<C>) \<Turnstile>\<^sub>\<E> \<E>'" by simp
   qed
 qed
