theory/Dynamic_Com_Topo_Analysis.thy
@@ -5,15 +5,15 @@ begin
 definition is_send_path :: "trace_pool \<Rightarrow> chan \<Rightarrow> control_path \<Rightarrow> bool" where
   "is_send_path \<E> c \<pi>\<^sub>y \<equiv> (\<exists> x\<^sub>y x\<^sub>e e\<^sub>n \<kappa> \<rho> x\<^sub>s\<^sub>c x\<^sub>m \<rho>\<^sub>e.
     \<E> \<pi>\<^sub>y = Some (\<langle>LET x\<^sub>y = SYNC x\<^sub>e in e\<^sub>n; \<rho>; \<kappa>\<rangle>) \<and>
-    \<rho> x\<^sub>e = Some \<lbrace>Send_Evt x\<^sub>s\<^sub>c x\<^sub>m, \<rho>\<^sub>e\<rbrace> \<and> 
-    \<rho>\<^sub>e x\<^sub>s\<^sub>c = Some \<lbrace>c\<rbrace>
+    \<rho> x\<^sub>e = Some (VClosure (Send_Evt x\<^sub>s\<^sub>c x\<^sub>m) \<rho>\<^sub>e) \<and> 
+    \<rho>\<^sub>e x\<^sub>s\<^sub>c = Some (VChan c)
   )"
 
 definition is_recv_path :: "trace_pool \<Rightarrow> chan \<Rightarrow> control_path \<Rightarrow> bool" where
   "is_recv_path \<E> c \<pi>\<^sub>y \<equiv> (\<exists> x\<^sub>y x\<^sub>e e\<^sub>n \<kappa> \<rho> x\<^sub>r\<^sub>c \<rho>\<^sub>e.
     \<E> \<pi>\<^sub>y = Some (\<langle>LET x\<^sub>y = SYNC x\<^sub>e in e\<^sub>n; \<rho>; \<kappa>\<rangle>) \<and> 
-    \<rho> x\<^sub>e = Some \<lbrace>Recv_Evt x\<^sub>r\<^sub>c, \<rho>\<^sub>e\<rbrace> \<and> 
-    \<rho>\<^sub>e x\<^sub>r\<^sub>c = Some \<lbrace>c\<rbrace>
+    \<rho> x\<^sub>e = Some (VClosure (Recv_Evt x\<^sub>r\<^sub>c) \<rho>\<^sub>e) \<and> 
+    \<rho>\<^sub>e x\<^sub>r\<^sub>c = Some (VChan c)
   )"
 
 
