theory/Dynamic_Semantics.thy
@@ -14,9 +14,9 @@ type_synonym control_path = "control_label list"
 datatype chan = Ch control_path var
 
 datatype val = 
-  V_Unit ("\<lbrace>\<rbrace>") |
-  V_Chan chan ("\<lbrace>_\<rbrace>") |
-  V_Closure prim "var \<rightharpoonup> val" ("\<lbrace>_, _\<rbrace>")
+  VUnit |
+  VChan chan |
+  VClosure prim "var \<rightharpoonup> val"
 
 type_synonym val_env = "var \<rightharpoonup> val"
   
@@ -31,28 +31,28 @@ inductive seq_step :: "state \<Rightarrow> state \<Rightarrow> bool" (infix "\<h
     \<langle>RESULT x; \<rho>; \<langle>x\<^sub>\<kappa>, e\<^sub>\<kappa>, \<rho>\<^sub>\<kappa>\<rangle> # \<kappa>\<rangle> \<hookrightarrow> \<langle>e\<^sub>\<kappa>; \<rho>\<^sub>\<kappa> ++ [x\<^sub>\<kappa> \<mapsto> \<omega>]; \<kappa>\<rangle>
   " |
   Let_Unit: "
-    \<langle>LET x = \<lparr>\<rparr> in e; \<rho>; \<kappa>\<rangle> \<hookrightarrow> \<langle>e; \<rho> ++ [x \<mapsto> \<lbrace>\<rbrace>]; \<kappa>\<rangle>
+    \<langle>LET x = \<lparr>\<rparr> in e; \<rho>; \<kappa>\<rangle> \<hookrightarrow> \<langle>e; \<rho> ++ [x \<mapsto> VUnit]; \<kappa>\<rangle>
   " |
   Let_Prim: "
-    \<langle>LET x = Prim p in e; \<rho>; \<kappa>\<rangle> \<hookrightarrow> \<langle>e; \<rho> ++ [x \<mapsto> \<lbrace>p, \<rho>\<rbrace>]; \<kappa>\<rangle>
+    \<langle>LET x = Prim p in e; \<rho>; \<kappa>\<rangle> \<hookrightarrow> \<langle>e; \<rho> ++ [x \<mapsto> (VClosure p \<rho>)]; \<kappa>\<rangle>
   " |
   Let_Fst: "
     \<lbrakk> 
-      \<rho> x\<^sub>p = Some \<lbrace>Pair x\<^sub>1 x\<^sub>2, \<rho>\<^sub>p\<rbrace>; 
+      \<rho> x\<^sub>p = Some (VClosure (Pair x\<^sub>1 x\<^sub>2) \<rho>\<^sub>p); 
       \<rho>\<^sub>p x\<^sub>1 = Some \<omega> 
     \<rbrakk> \<Longrightarrow>
     \<langle>LET x = FST x\<^sub>p in e; \<rho>; \<kappa>\<rangle> \<hookrightarrow> \<langle>e; \<rho> ++ [x \<mapsto> \<omega>]; \<kappa>\<rangle>
   " |
   Let_Snd: "
     \<lbrakk> 
-      \<rho> x\<^sub>p = Some \<lbrace>Pair x\<^sub>1 x\<^sub>2, \<rho>\<^sub>p\<rbrace>; 
+      \<rho> x\<^sub>p = Some (VClosure (Pair x\<^sub>1 x\<^sub>2) \<rho>\<^sub>p); 
       \<rho>\<^sub>p x\<^sub>2 = Some \<omega> 
     \<rbrakk> \<Longrightarrow>
     \<langle>LET x = SND x\<^sub>p in e; \<rho>; \<kappa>\<rangle> \<hookrightarrow> \<langle>e; \<rho> ++ [x \<mapsto> \<omega>]; \<kappa>\<rangle>
   " |
   Let_Case_Left: "
     \<lbrakk> 
-      \<rho> x\<^sub>s = Some \<lbrace>Left x\<^sub>l', \<rho>\<^sub>l\<rbrace>; 
+      \<rho> x\<^sub>s = Some (VClosure (Left x\<^sub>l') \<rho>\<^sub>l); 
       \<rho>\<^sub>l x\<^sub>l' = Some \<omega>\<^sub>l
     \<rbrakk> \<Longrightarrow>
     \<langle>LET x = CASE x\<^sub>s LEFT x\<^sub>l |> e\<^sub>l RIGHT x\<^sub>r |> e\<^sub>r in e; \<rho>; \<kappa>\<rangle> \<hookrightarrow> 
@@ -60,7 +60,7 @@ inductive seq_step :: "state \<Rightarrow> state \<Rightarrow> bool" (infix "\<h
   " |
   Let_Case_Right: "
     \<lbrakk>
-      \<rho> x\<^sub>s = Some \<lbrace>Right x\<^sub>r', \<rho>\<^sub>r\<rbrace>; 
+      \<rho> x\<^sub>s = Some (VClosure (Right x\<^sub>r') \<rho>\<^sub>r); 
       \<rho>\<^sub>r x\<^sub>r' = Some \<omega>\<^sub>r
     \<rbrakk> \<Longrightarrow>
     \<langle>LET x = CASE x\<^sub>s LEFT x\<^sub>l |> e\<^sub>l RIGHT x\<^sub>r |> e\<^sub>r in e; \<rho>; \<kappa>\<rangle> \<hookrightarrow> 
@@ -68,11 +68,11 @@ inductive seq_step :: "state \<Rightarrow> state \<Rightarrow> bool" (infix "\<h
   " |
   Let_App: "
     \<lbrakk>
-      \<rho> f = Some \<lbrace>Abs f\<^sub>l x\<^sub>l e\<^sub>l, \<rho>\<^sub>l\<rbrace> ; 
+      \<rho> f = Some (VClosure (Abs f\<^sub>l x\<^sub>l e\<^sub>l) \<rho>\<^sub>l); 
       \<rho> x\<^sub>a = Some \<omega>\<^sub>a 
     \<rbrakk> \<Longrightarrow>
     \<langle>LET x = APP f x\<^sub>a in e; \<rho>; \<kappa>\<rangle> \<hookrightarrow> 
-    \<langle>e\<^sub>l; \<rho>\<^sub>l ++ [f\<^sub>l \<mapsto> \<lbrace>Abs f\<^sub>l x\<^sub>l e\<^sub>l, \<rho>\<^sub>l\<rbrace>, x\<^sub>l \<mapsto> \<omega>\<^sub>a]; \<langle>x, e, \<rho>\<rangle> # \<kappa>\<rangle>
+    \<langle>e\<^sub>l; \<rho>\<^sub>l ++ [f\<^sub>l \<mapsto> (VClosure (Abs f\<^sub>l x\<^sub>l e\<^sub>l) \<rho>\<^sub>l), x\<^sub>l \<mapsto> \<omega>\<^sub>a]; \<langle>x, e, \<rho>\<rangle> # \<kappa>\<rangle>
   "
 
 
@@ -118,7 +118,7 @@ inductive concur_step :: "trace_pool \<Rightarrow> trace_pool \<Rightarrow> bool
       \<E> \<pi> = Some (\<langle>LET x = CHAN \<lparr>\<rparr> in e; \<rho>; \<kappa>\<rangle>)
     \<rbrakk> \<Longrightarrow>
     \<E> \<rightarrow> \<E> ++ [
-      \<pi>;;(LNext x) \<mapsto> (\<langle>e; \<rho> ++ [x \<mapsto> \<lbrace>Ch \<pi> x\<rbrace>]; \<kappa>\<rangle>)
+      \<pi>;;(LNext x) \<mapsto> (\<langle>e; \<rho> ++ [x \<mapsto> (VChan (Ch \<pi> x))]; \<kappa>\<rangle>)
     ]
   " |
   Let_Spawn: "
@@ -127,7 +127,7 @@ inductive concur_step :: "trace_pool \<Rightarrow> trace_pool \<Rightarrow> bool
       \<E> \<pi> = Some (\<langle>LET x = SPAWN e\<^sub>c in e; \<rho>; \<kappa>\<rangle>)
     \<rbrakk> \<Longrightarrow>
     \<E> \<rightarrow> \<E> ++ [
-      \<pi>;;(LNext x) \<mapsto> (\<langle>e; \<rho> ++ [x \<mapsto> \<lbrace>\<rbrace>]; \<kappa>\<rangle>), 
+      \<pi>;;(LNext x) \<mapsto> (\<langle>e; \<rho> ++ [x \<mapsto> VUnit]; \<kappa>\<rangle>), 
       \<pi>;;(LSpawn x) \<mapsto> (\<langle>e\<^sub>c; \<rho>; []\<rangle>) 
     ]
   " |
@@ -136,19 +136,19 @@ inductive concur_step :: "trace_pool \<Rightarrow> trace_pool \<Rightarrow> bool
    
       leaf \<E> \<pi>\<^sub>s ;
       \<E> \<pi>\<^sub>s = Some (\<langle>LET x\<^sub>s = SYNC x\<^sub>s\<^sub>e in e\<^sub>s; \<rho>\<^sub>s; \<kappa>\<^sub>s\<rangle>);
-      \<rho>\<^sub>s x\<^sub>s\<^sub>e = Some \<lbrace>Send_Evt x\<^sub>s\<^sub>c x\<^sub>m, \<rho>\<^sub>s\<^sub>e\<rbrace>;
+      \<rho>\<^sub>s x\<^sub>s\<^sub>e = Some (VClosure (Send_Evt x\<^sub>s\<^sub>c x\<^sub>m) \<rho>\<^sub>s\<^sub>e);
 
       leaf \<E> \<pi>\<^sub>r ;
       \<E> \<pi>\<^sub>r = Some (\<langle>LET x\<^sub>r = SYNC x\<^sub>r\<^sub>e in e\<^sub>r; \<rho>\<^sub>r; \<kappa>\<^sub>r\<rangle>);
-      \<rho>\<^sub>r x\<^sub>r\<^sub>e = Some \<lbrace>Recv_Evt x\<^sub>r\<^sub>c, \<rho>\<^sub>r\<^sub>e\<rbrace>;
+      \<rho>\<^sub>r x\<^sub>r\<^sub>e = Some (VClosure (Recv_Evt x\<^sub>r\<^sub>c) \<rho>\<^sub>r\<^sub>e);
 
-      \<rho>\<^sub>s\<^sub>e x\<^sub>s\<^sub>c = Some \<lbrace>c\<rbrace>; 
-      \<rho>\<^sub>r\<^sub>e x\<^sub>r\<^sub>c = Some \<lbrace>c\<rbrace>;      
+      \<rho>\<^sub>s\<^sub>e x\<^sub>s\<^sub>c = Some (VChan c); 
+      \<rho>\<^sub>r\<^sub>e x\<^sub>r\<^sub>c = Some (VChan c);      
       \<rho>\<^sub>s\<^sub>e x\<^sub>m = Some \<omega>\<^sub>m 
 
     \<rbrakk> \<Longrightarrow>
     \<E> \<rightarrow> \<E> ++ [
-      \<pi>\<^sub>s;;(LNext x\<^sub>s) \<mapsto> (\<langle>e\<^sub>s; \<rho>\<^sub>s ++ [x\<^sub>s \<mapsto> \<lbrace>\<rbrace>]; \<kappa>\<^sub>s\<rangle>), 
+      \<pi>\<^sub>s;;(LNext x\<^sub>s) \<mapsto> (\<langle>e\<^sub>s; \<rho>\<^sub>s ++ [x\<^sub>s \<mapsto> VUnit]; \<kappa>\<^sub>s\<rangle>), 
       \<pi>\<^sub>r;;(LNext x\<^sub>r) \<mapsto> (\<langle>e\<^sub>r; \<rho>\<^sub>r ++ [x\<^sub>r \<mapsto> \<omega>\<^sub>m]; \<kappa>\<^sub>r\<rangle>)
     ]
   "
