theory/Sound_Com_Topo_Analysis.thy
@@ -9,8 +9,8 @@ begin
 
 lemma static_send_chan_doesnt_exist_sound: "
   \<lbrakk>
-    \<rho>\<^sub>e x\<^sub>s\<^sub>c = Some \<lbrace>Ch \<pi> x\<^sub>c\<rbrace>;
-    \<rho>\<^sub>y x\<^sub>e = Some \<lbrace>Send_Evt x\<^sub>s\<^sub>c x\<^sub>m, \<rho>\<^sub>e\<rbrace>;
+    \<rho>\<^sub>e x\<^sub>s\<^sub>c = Some (VChan (Ch \<pi> x\<^sub>c));
+    \<rho>\<^sub>y x\<^sub>e = Some (VClosure (Send_Evt x\<^sub>s\<^sub>c x\<^sub>m) \<rho>\<^sub>e);
     \<E>' \<pi>\<^sub>y = Some (\<langle>LET x\<^sub>y = SYNC x\<^sub>e in e\<^sub>y;\<rho>\<^sub>y;\<kappa>\<^sub>y\<rangle>);
     [[] \<mapsto> \<langle>e;Map.empty;[]\<rangle>] \<rightarrow>* \<E>';
     (\<V>, \<C>) \<Turnstile>\<^sub>e e
@@ -23,16 +23,16 @@ lemma static_send_chan_doesnt_exist_sound: "
  apply (drule spec[of _ \<pi>\<^sub>y], drule spec[of _ "\<langle>LET x\<^sub>y = SYNC x\<^sub>e in e\<^sub>y;\<rho>\<^sub>y;\<kappa>\<^sub>y\<rangle>"], simp)
  apply (erule static_eval_state.cases; auto)
  apply (erule static_eval_env.cases; auto)
- apply (drule spec[of _ x\<^sub>e], drule spec[of _ "\<lbrace>Send_Evt x\<^sub>s\<^sub>c x\<^sub>m, \<rho>\<^sub>e\<rbrace>"]; simp)
+ apply (drule spec[of _ x\<^sub>e], drule spec[of _ "(VClosure (Send_Evt x\<^sub>s\<^sub>c x\<^sub>m) \<rho>\<^sub>e)"]; simp)
  apply (erule conjE)
  apply (erule static_eval_value.cases; auto)
  apply (erule static_eval_env.cases; auto)
- apply (drule spec[of _ x\<^sub>s\<^sub>c], drule spec[of _ "\<lbrace>Ch \<pi> x\<^sub>c\<rbrace>"]; simp)
+ apply (drule spec[of _ x\<^sub>s\<^sub>c], drule spec[of _ "(VChan (Ch \<pi> x\<^sub>c))"]; simp)
 done
 
 lemma static_send_evt_doesnt_exist_sound: "
   \<lbrakk>
-    \<rho>\<^sub>y x\<^sub>e = Some \<lbrace>Send_Evt x\<^sub>s\<^sub>c x\<^sub>m, \<rho>\<^sub>e\<rbrace>;
+    \<rho>\<^sub>y x\<^sub>e = Some (VClosure (Send_Evt x\<^sub>s\<^sub>c x\<^sub>m) \<rho>\<^sub>e);
     [[] \<mapsto> \<langle>e;Map.empty;[]\<rangle>] \<rightarrow>* \<E>';
     \<E>' \<pi>\<^sub>y = Some (\<langle>LET x\<^sub>y = SYNC x\<^sub>e in e\<^sub>y;\<rho>\<^sub>y;\<kappa>\<^sub>y\<rangle>);
     (\<V>, \<C>) \<Turnstile>\<^sub>e e
@@ -41,37 +41,13 @@ lemma static_send_evt_doesnt_exist_sound: "
 "
   apply (drule values_not_bound_sound_coro; assumption?; auto)
 done
-(*
-lemma static_message_isnt_sent_sound: "
-  \<lbrakk>
-    \<rho>\<^sub>y x\<^sub>e = Some \<lbrace>Send_Evt x\<^sub>s\<^sub>c x\<^sub>m, \<rho>\<^sub>e\<rbrace>;
-    \<rho>\<^sub>e x\<^sub>s\<^sub>c = Some \<lbrace>Ch \<pi> x\<^sub>c\<rbrace>;
-    \<E>' \<pi>\<^sub>y = Some (\<langle>LET x\<^sub>y = SYNC x\<^sub>e in e\<^sub>y;\<rho>\<^sub>y;\<kappa>\<^sub>y\<rangle>);
-    [[] \<mapsto> \<langle>e;Map.empty;[]\<rangle>] \<rightarrow>* \<E>';
-    (\<V>, \<C>) \<Turnstile>\<^sub>e e
-  \<rbrakk> \<Longrightarrow> 
-  \<V> x\<^sub>m \<subseteq> \<C> x\<^sub>c
-"
-  apply (frule static_eval_to_pool)
-  apply (drule static_eval_preserved_under_concur_step_star [of _ _ _ \<E>']; assumption?)
-  apply (erule static_eval_pool.cases; auto)
-  apply (drule spec[of _ \<pi>\<^sub>y], drule spec[of _ "\<langle>LET x\<^sub>y = SYNC x\<^sub>e in e\<^sub>y;\<rho>\<^sub>y;\<kappa>\<^sub>y\<rangle>"], simp)
-  apply (erule static_eval_state.cases; auto)
-  apply (erule static_eval.cases[of _ "LET x\<^sub>y = SYNC x\<^sub>e in e\<^sub>y"]; auto)
-  apply (thin_tac "\<forall>x\<^sub>r\<^sub>c. ^Recv_Evt x\<^sub>r\<^sub>c \<in> \<V> x\<^sub>e \<longrightarrow> (\<forall>x\<^sub>c. ^Chan x\<^sub>c \<in> \<V> x\<^sub>r\<^sub>c \<longrightarrow> \<C> x\<^sub>c \<subseteq> \<V> x\<^sub>y)")
-  apply (drule spec[of _ x\<^sub>s\<^sub>c], drule spec[of _ x\<^sub>m])
-  apply (frule static_send_evt_doesnt_exist_sound; assumption?)
-  apply (erule impE; simp)
-  apply (drule spec[of _ x\<^sub>c])
-  apply (drule static_send_chan_doesnt_exist_sound; assumption?; auto)
-done
-*)
+
 
 lemma isnt_send_path_sound': "
   \<lbrakk>
     \<E>' \<pi>\<^sub>y = Some (\<langle>LET x\<^sub>y = SYNC x\<^sub>e in e\<^sub>y;\<rho>\<^sub>y;\<kappa>\<^sub>y\<rangle>);
-    \<rho>\<^sub>e x\<^sub>s\<^sub>c = Some \<lbrace>Ch \<pi> x\<^sub>c\<rbrace>;
-    \<rho>\<^sub>y x\<^sub>e = Some \<lbrace>Send_Evt x\<^sub>s\<^sub>c x\<^sub>m, \<rho>\<^sub>e\<rbrace>;
+    \<rho>\<^sub>e x\<^sub>s\<^sub>c = Some (VChan (Ch \<pi> x\<^sub>c));
+    \<rho>\<^sub>y x\<^sub>e = Some (VClosure (Send_Evt x\<^sub>s\<^sub>c x\<^sub>m) \<rho>\<^sub>e);
     [[] \<mapsto> \<langle>e;Map.empty;[]\<rangle>] \<rightarrow>* \<E>';
     (\<V>, \<C>) \<Turnstile>\<^sub>e e
   \<rbrakk> \<Longrightarrow> 
@@ -263,8 +239,8 @@ using isnt_send_path_sound runtime_send_paths_are_inclusive by blast
 
 lemma static_recv_chan_doesnt_exist_sound: "
   \<lbrakk>
-    \<rho>\<^sub>e x\<^sub>r\<^sub>c = Some \<lbrace>Ch \<pi> x\<^sub>c\<rbrace>;
-    \<rho>\<^sub>y x\<^sub>e = Some \<lbrace>Recv_Evt x\<^sub>r\<^sub>c, \<rho>\<^sub>e\<rbrace>;
+    \<rho>\<^sub>e x\<^sub>r\<^sub>c = Some (VChan (Ch \<pi> x\<^sub>c));
+    \<rho>\<^sub>y x\<^sub>e = Some (VClosure (Recv_Evt x\<^sub>r\<^sub>c) \<rho>\<^sub>e);
     \<E>' \<pi>\<^sub>y = Some (\<langle>LET x\<^sub>y = SYNC x\<^sub>e in e\<^sub>y;\<rho>\<^sub>y;\<kappa>\<^sub>y\<rangle>);
     [[] \<mapsto> \<langle>e;Map.empty;[]\<rangle>] \<rightarrow>* \<E>';
     (\<V>, \<C>) \<Turnstile>\<^sub>e e
@@ -277,16 +253,16 @@ lemma static_recv_chan_doesnt_exist_sound: "
  apply (drule spec[of _ \<pi>\<^sub>y], drule spec[of _ "\<langle>LET x\<^sub>y = SYNC x\<^sub>e in e\<^sub>y;\<rho>\<^sub>y;\<kappa>\<^sub>y\<rangle>"], simp)
  apply (erule static_eval_state.cases; auto)
  apply (erule static_eval_env.cases; auto)
- apply (drule spec[of _ x\<^sub>e], drule spec[of _ "\<lbrace>Recv_Evt x\<^sub>r\<^sub>c, \<rho>\<^sub>e\<rbrace>"]; simp)
+ apply (drule spec[of _ x\<^sub>e], drule spec[of _ "(VClosure (Recv_Evt x\<^sub>r\<^sub>c) \<rho>\<^sub>e)"]; simp)
  apply (erule conjE)
  apply (erule static_eval_value.cases; auto)
  apply (erule static_eval_env.cases; auto)
- apply (drule spec[of _ x\<^sub>r\<^sub>c], drule spec[of _ "\<lbrace>Ch \<pi> x\<^sub>c\<rbrace>"]; simp)
+ apply (drule spec[of _ x\<^sub>r\<^sub>c], drule spec[of _ "(VChan (Ch \<pi> x\<^sub>c))"]; simp)
 done
 
 lemma static_recv_evt_doesnt_exist_sound: "
   \<lbrakk>
-    \<rho>\<^sub>y x\<^sub>e = Some \<lbrace>Recv_Evt x\<^sub>r\<^sub>c, \<rho>\<^sub>e\<rbrace>;
+    \<rho>\<^sub>y x\<^sub>e = Some (VClosure (Recv_Evt x\<^sub>r\<^sub>c) \<rho>\<^sub>e);
     \<E>' \<pi>\<^sub>y = Some (\<langle>LET x\<^sub>y = SYNC x\<^sub>e in e\<^sub>y;\<rho>\<^sub>y;\<kappa>\<^sub>y\<rangle>);
     [[] \<mapsto> \<langle>e;Map.empty;[]\<rangle>] \<rightarrow>* \<E>';
     (\<V>, \<C>) \<Turnstile>\<^sub>e e
@@ -299,8 +275,8 @@ done
 lemma isnt_recv_path_sound': "
   \<lbrakk>
     \<E>' \<pi>\<^sub>y = Some (\<langle>LET x\<^sub>y = SYNC x\<^sub>e in e\<^sub>y;\<rho>\<^sub>y;\<kappa>\<^sub>y\<rangle>); 
-    \<rho>\<^sub>y x\<^sub>e = Some \<lbrace>Recv_Evt x\<^sub>r\<^sub>c, \<rho>\<^sub>e\<rbrace>;
-    \<rho>\<^sub>e x\<^sub>r\<^sub>c = Some \<lbrace>Ch \<pi> x\<^sub>c\<rbrace>;
+    \<rho>\<^sub>y x\<^sub>e = Some (VClosure (Recv_Evt x\<^sub>r\<^sub>c) \<rho>\<^sub>e);
+    \<rho>\<^sub>e x\<^sub>r\<^sub>c = Some (VChan (Ch \<pi> x\<^sub>c));
     [[] \<mapsto> \<langle>e;Map.empty;[]\<rangle>] \<rightarrow>* \<E>';
     (\<V>, \<C>) \<Turnstile>\<^sub>e e
   \<rbrakk> \<Longrightarrow>
@@ -331,7 +307,7 @@ lemma runtime_recv_paths_are_inclusive: "
     [[] \<mapsto> \<langle>e;Map.empty;[]\<rangle>] \<rightarrow>* \<E>';
     is_recv_path \<E>' c \<pi>\<^sub>1';
     is_recv_path \<E>' c \<pi>\<^sub>2'
-  \<rbrakk> \<Longrightarrow> 
+  \<rbrakk> \<Longrightarrow>
   \<pi>\<^sub>1' \<asymp> \<pi>\<^sub>2'
 "
 apply (unfold is_recv_path_def; auto)
