theory/Sound_Traceability.thy
@@ -114,19 +114,19 @@ inductive subexp :: "exp \<Rightarrow> exp \<Rightarrow> bool" ("_ \<preceq>\<^s
 lemma static_traceable_exp_preserved_sync_recv_evt: "
 \<lbrakk>
   \<forall>\<pi> e \<rho> \<kappa>. \<E> \<pi> = Some (\<langle>e;\<rho>;\<kappa>\<rangle>) \<longrightarrow> \<V> \<turnstile> e\<^sub>0 \<down> \<pi> \<mapsto> e;
-  (\<V>, \<C>) \<Turnstile>\<^sub>\<E> \<E>(\<pi>\<^sub>s ;; (LNext x\<^sub>s) \<mapsto> \<langle>e\<^sub>s;\<rho>\<^sub>s(x\<^sub>s \<mapsto> \<lbrace>\<rbrace>);\<kappa>\<^sub>s\<rangle>, \<pi>\<^sub>r ;; (LNext x\<^sub>r) \<mapsto> \<langle>e';\<rho>\<^sub>r(x\<^sub>r \<mapsto> \<omega>\<^sub>m);\<kappa>'\<rangle>);
+  (\<V>, \<C>) \<Turnstile>\<^sub>\<E> \<E>(\<pi>\<^sub>s ;; (LNext x\<^sub>s) \<mapsto> \<langle>e\<^sub>s;\<rho>\<^sub>s(x\<^sub>s \<mapsto> VUnit);\<kappa>\<^sub>s\<rangle>, \<pi>\<^sub>r ;; (LNext x\<^sub>r) \<mapsto> \<langle>e';\<rho>\<^sub>r(x\<^sub>r \<mapsto> \<omega>\<^sub>m);\<kappa>'\<rangle>);
   \<E> \<pi>\<^sub>r = Some (\<langle>LET x\<^sub>r = SYNC x\<^sub>r\<^sub>e in e\<^sub>n;\<rho>\<^sub>r;\<kappa>'\<rangle>)
 \<rbrakk> \<Longrightarrow> 
 \<V> \<turnstile> e\<^sub>0 \<down> \<pi>\<^sub>r ;; (LNext x\<^sub>r) \<mapsto> e\<^sub>n
 "
 proof -
-  assume "(\<V>, \<C>) \<Turnstile>\<^sub>\<E> \<E>(\<pi>\<^sub>s ;; (LNext x\<^sub>s) \<mapsto> \<langle>e\<^sub>s;\<rho>\<^sub>s(x\<^sub>s \<mapsto> \<lbrace>\<rbrace>);\<kappa>\<^sub>s\<rangle>, \<pi>\<^sub>r ;; (LNext x\<^sub>r) \<mapsto> \<langle>e';\<rho>\<^sub>r(x\<^sub>r \<mapsto> \<omega>\<^sub>m);\<kappa>'\<rangle>)"
+  assume "(\<V>, \<C>) \<Turnstile>\<^sub>\<E> \<E>(\<pi>\<^sub>s ;; (LNext x\<^sub>s) \<mapsto> \<langle>e\<^sub>s;\<rho>\<^sub>s(x\<^sub>s \<mapsto> VUnit);\<kappa>\<^sub>s\<rangle>, \<pi>\<^sub>r ;; (LNext x\<^sub>r) \<mapsto> \<langle>e';\<rho>\<^sub>r(x\<^sub>r \<mapsto> \<omega>\<^sub>m);\<kappa>'\<rangle>)"
   assume " \<forall>\<pi> e \<rho> \<kappa>. \<E> \<pi> = Some (\<langle>e;\<rho>;\<kappa>\<rangle>) \<longrightarrow> \<V> \<turnstile> e\<^sub>0 \<down> \<pi> \<mapsto> e"
   and "\<E> \<pi>\<^sub>r = Some (\<langle>LET x\<^sub>r = SYNC x\<^sub>r\<^sub>e in e\<^sub>n;\<rho>\<^sub>r;\<kappa>'\<rangle>)" then
   have "\<V> \<turnstile> e\<^sub>0 \<down> \<pi>\<^sub>r \<mapsto> LET x\<^sub>r = SYNC x\<^sub>r\<^sub>e in e\<^sub>n" by simp
-  have "(\<E>(\<pi>\<^sub>s ;; (LNext x\<^sub>s) \<mapsto> \<langle>e\<^sub>s;\<rho>\<^sub>s(x\<^sub>s \<mapsto> \<lbrace>\<rbrace>);\<kappa>\<^sub>s\<rangle>, \<pi>\<^sub>r ;; (LNext x\<^sub>r) \<mapsto> \<langle>e';\<rho>\<^sub>r(x\<^sub>r \<mapsto> \<omega>\<^sub>m);\<kappa>'\<rangle>)) (\<pi>\<^sub>r ;; (LNext x\<^sub>r)) 
+  have "(\<E>(\<pi>\<^sub>s ;; (LNext x\<^sub>s) \<mapsto> \<langle>e\<^sub>s;\<rho>\<^sub>s(x\<^sub>s \<mapsto> VUnit);\<kappa>\<^sub>s\<rangle>, \<pi>\<^sub>r ;; (LNext x\<^sub>r) \<mapsto> \<langle>e';\<rho>\<^sub>r(x\<^sub>r \<mapsto> \<omega>\<^sub>m);\<kappa>'\<rangle>)) (\<pi>\<^sub>r ;; (LNext x\<^sub>r)) 
       = Some (\<langle>e';\<rho>\<^sub>r(x\<^sub>r \<mapsto> \<omega>\<^sub>m);\<kappa>'\<rangle>)" by simp
-  with \<open>(\<V>, \<C>) \<Turnstile>\<^sub>\<E> \<E>(\<pi>\<^sub>s ;; (LNext x\<^sub>s) \<mapsto> \<langle>e\<^sub>s;\<rho>\<^sub>s(x\<^sub>s \<mapsto> \<lbrace>\<rbrace>);\<kappa>\<^sub>s\<rangle>, \<pi>\<^sub>r ;; (LNext x\<^sub>r) \<mapsto> \<langle>e';\<rho>\<^sub>r(x\<^sub>r \<mapsto> \<omega>\<^sub>m);\<kappa>'\<rangle>)\<close>
+  with \<open>(\<V>, \<C>) \<Turnstile>\<^sub>\<E> \<E>(\<pi>\<^sub>s ;; (LNext x\<^sub>s) \<mapsto> \<langle>e\<^sub>s;\<rho>\<^sub>s(x\<^sub>s \<mapsto> VUnit);\<kappa>\<^sub>s\<rangle>, \<pi>\<^sub>r ;; (LNext x\<^sub>r) \<mapsto> \<langle>e';\<rho>\<^sub>r(x\<^sub>r \<mapsto> \<omega>\<^sub>m);\<kappa>'\<rangle>)\<close>
   have "\<parallel>\<rho>\<^sub>r(x\<^sub>r \<mapsto> \<omega>\<^sub>m)\<parallel> \<sqsubseteq> \<V>" by (blast intro: static_eval_pool_to_precise)
 
   have "(\<rho>\<^sub>r(x\<^sub>r \<mapsto> \<omega>\<^sub>m)) x\<^sub>r = Some \<omega>\<^sub>m" by simp
@@ -141,29 +141,29 @@ lemma static_traceable_exp_preserved_sync_send_evt: "
 \<lbrakk>
   \<forall>\<pi> e \<rho> \<kappa>. \<E> \<pi> = Some (\<langle>e;\<rho>;\<kappa>\<rangle>) \<longrightarrow> \<V> \<turnstile> e\<^sub>0 \<down> \<pi> \<mapsto> e;
   \<E> \<pi>\<^sub>s = Some (\<langle>LET x\<^sub>s = SYNC x\<^sub>s\<^sub>e in e';\<rho>\<^sub>s;\<kappa>'\<rangle>);
-  (\<V>, \<C>) \<Turnstile>\<^sub>\<E> \<E>(\<pi>\<^sub>s ;; (LNext x\<^sub>s) \<mapsto> \<langle>e';\<rho>\<^sub>s(x\<^sub>s \<mapsto> \<lbrace>\<rbrace>);\<kappa>'\<rangle>, \<pi>\<^sub>r ;; (LNext x\<^sub>r) \<mapsto> \<langle>e\<^sub>r;\<rho>\<^sub>r(x\<^sub>r \<mapsto> \<omega>\<^sub>m);\<kappa>\<^sub>r\<rangle>);
+  (\<V>, \<C>) \<Turnstile>\<^sub>\<E> \<E>(\<pi>\<^sub>s ;; (LNext x\<^sub>s) \<mapsto> \<langle>e';\<rho>\<^sub>s(x\<^sub>s \<mapsto> VUnit);\<kappa>'\<rangle>, \<pi>\<^sub>r ;; (LNext x\<^sub>r) \<mapsto> \<langle>e\<^sub>r;\<rho>\<^sub>r(x\<^sub>r \<mapsto> \<omega>\<^sub>m);\<kappa>\<^sub>r\<rangle>);
   \<pi>\<^sub>s \<noteq> \<pi>\<^sub>r
 \<rbrakk> \<Longrightarrow> 
 \<V> \<turnstile> e\<^sub>0 \<down> \<pi>\<^sub>s ;; (LNext x\<^sub>s) \<mapsto> e'
 "
 proof -
-  assume "(\<V>, \<C>) \<Turnstile>\<^sub>\<E> \<E>(\<pi>\<^sub>s ;; (LNext x\<^sub>s) \<mapsto> \<langle>e';\<rho>\<^sub>s(x\<^sub>s \<mapsto> \<lbrace>\<rbrace>);\<kappa>'\<rangle>, \<pi>\<^sub>r ;; (LNext x\<^sub>r) \<mapsto> \<langle>e\<^sub>r;\<rho>\<^sub>r(x\<^sub>r \<mapsto> \<omega>\<^sub>m);\<kappa>\<^sub>r\<rangle>)"
+  assume "(\<V>, \<C>) \<Turnstile>\<^sub>\<E> \<E>(\<pi>\<^sub>s ;; (LNext x\<^sub>s) \<mapsto> \<langle>e';\<rho>\<^sub>s(x\<^sub>s \<mapsto> VUnit);\<kappa>'\<rangle>, \<pi>\<^sub>r ;; (LNext x\<^sub>r) \<mapsto> \<langle>e\<^sub>r;\<rho>\<^sub>r(x\<^sub>r \<mapsto> \<omega>\<^sub>m);\<kappa>\<^sub>r\<rangle>)"
   and "\<pi>\<^sub>s \<noteq> \<pi>\<^sub>r"
   assume "\<forall>\<pi> e \<rho> \<kappa>. \<E> \<pi> = Some (\<langle>e;\<rho>;\<kappa>\<rangle>) \<longrightarrow> \<V> \<turnstile> e\<^sub>0 \<down> \<pi> \<mapsto> e"
   and "\<E> \<pi>\<^sub>s = Some (\<langle>LET x\<^sub>s = SYNC x\<^sub>s\<^sub>e in e';\<rho>\<^sub>s;\<kappa>'\<rangle>)" then
   have "\<V> \<turnstile> e\<^sub>0 \<down> \<pi>\<^sub>s \<mapsto> LET x\<^sub>s = SYNC x\<^sub>s\<^sub>e in e'" by simp
 
   with `\<pi>\<^sub>s \<noteq> \<pi>\<^sub>r`
-  have "(\<E>(\<pi>\<^sub>s ;; (LNext x\<^sub>s) \<mapsto> \<langle>e';\<rho>\<^sub>s(x\<^sub>s \<mapsto> \<lbrace>\<rbrace>);\<kappa>'\<rangle>, \<pi>\<^sub>r ;; (LNext x\<^sub>r) \<mapsto> \<langle>e\<^sub>r;\<rho>\<^sub>r(x\<^sub>r \<mapsto> \<omega>\<^sub>m);\<kappa>\<^sub>r\<rangle>)) (\<pi>\<^sub>s ;; (LNext x\<^sub>s)) 
-      = Some (\<langle>e';\<rho>\<^sub>s(x\<^sub>s \<mapsto> \<lbrace>\<rbrace>);\<kappa>'\<rangle>)" by simp
-  with `\<pi>\<^sub>s \<noteq> \<pi>\<^sub>r` \<open>(\<V>, \<C>) \<Turnstile>\<^sub>\<E> \<E>(\<pi>\<^sub>s ;; (LNext x\<^sub>s) \<mapsto> \<langle>e';\<rho>\<^sub>s(x\<^sub>s \<mapsto> \<lbrace>\<rbrace>);\<kappa>'\<rangle>, \<pi>\<^sub>r ;; (LNext x\<^sub>r) \<mapsto> \<langle>e\<^sub>r;\<rho>\<^sub>r(x\<^sub>r \<mapsto> \<omega>\<^sub>m);\<kappa>\<^sub>r\<rangle>)\<close>
-  have "\<parallel>\<rho>\<^sub>s(x\<^sub>s \<mapsto> \<lbrace>\<rbrace>)\<parallel> \<sqsubseteq> \<V>" using static_eval_pool_to_precise by blast
+  have "(\<E>(\<pi>\<^sub>s ;; (LNext x\<^sub>s) \<mapsto> \<langle>e';\<rho>\<^sub>s(x\<^sub>s \<mapsto> VUnit);\<kappa>'\<rangle>, \<pi>\<^sub>r ;; (LNext x\<^sub>r) \<mapsto> \<langle>e\<^sub>r;\<rho>\<^sub>r(x\<^sub>r \<mapsto> \<omega>\<^sub>m);\<kappa>\<^sub>r\<rangle>)) (\<pi>\<^sub>s ;; (LNext x\<^sub>s)) 
+      = Some (\<langle>e';\<rho>\<^sub>s(x\<^sub>s \<mapsto> VUnit);\<kappa>'\<rangle>)" by simp
+  with `\<pi>\<^sub>s \<noteq> \<pi>\<^sub>r` \<open>(\<V>, \<C>) \<Turnstile>\<^sub>\<E> \<E>(\<pi>\<^sub>s ;; (LNext x\<^sub>s) \<mapsto> \<langle>e';\<rho>\<^sub>s(x\<^sub>s \<mapsto> VUnit);\<kappa>'\<rangle>, \<pi>\<^sub>r ;; (LNext x\<^sub>r) \<mapsto> \<langle>e\<^sub>r;\<rho>\<^sub>r(x\<^sub>r \<mapsto> \<omega>\<^sub>m);\<kappa>\<^sub>r\<rangle>)\<close>
+  have "\<parallel>\<rho>\<^sub>s(x\<^sub>s \<mapsto> VUnit)\<parallel> \<sqsubseteq> \<V>" using static_eval_pool_to_precise by blast
 
-  have "(\<rho>\<^sub>s(x\<^sub>s \<mapsto> \<lbrace>\<rbrace>)) x\<^sub>s = Some \<lbrace>\<rbrace>" by simp
-  with `\<parallel>\<rho>\<^sub>s(x\<^sub>s \<mapsto> \<lbrace>\<rbrace>)\<parallel> \<sqsubseteq> \<V>`
-  have " |\<lbrace>\<rbrace>| \<in> \<V> x\<^sub>s" using abstracted_value_exists by fastforce
+  have "(\<rho>\<^sub>s(x\<^sub>s \<mapsto> VUnit)) x\<^sub>s = Some VUnit" by simp
+  with `\<parallel>\<rho>\<^sub>s(x\<^sub>s \<mapsto> VUnit)\<parallel> \<sqsubseteq> \<V>`
+  have " |VUnit| \<in> \<V> x\<^sub>s" using abstracted_value_exists by fastforce
 
-  from \<open>\<V> \<turnstile> e\<^sub>0 \<down> \<pi>\<^sub>s \<mapsto> LET x\<^sub>s = SYNC x\<^sub>s\<^sub>e in e'\<close> \<open>|\<lbrace>\<rbrace>| \<in> \<V> x\<^sub>s\<close>
+  from \<open>\<V> \<turnstile> e\<^sub>0 \<down> \<pi>\<^sub>s \<mapsto> LET x\<^sub>s = SYNC x\<^sub>s\<^sub>e in e'\<close> \<open>|VUnit| \<in> \<V> x\<^sub>s\<close>
   show "\<V> \<turnstile> e\<^sub>0 \<down> \<pi>\<^sub>s ;; (LNext x\<^sub>s) \<mapsto> e'" using static_traceable.Let_Sync by blast
 
 qed
@@ -342,7 +342,7 @@ lemma static_traceable_exp_preserved_under_seq_step_up: "
 done
 
 lemma static_traceable_exp_preserved_under_chan:"
-  (\<E>(\<pi> ;; (LNext x) \<mapsto> \<langle>e;\<rho>(x \<mapsto> \<lbrace>Ch \<pi> x\<rbrace>);\<kappa>\<rangle>)) \<pi>' = Some (\<langle>e';\<rho>';\<kappa>'\<rangle>) \<Longrightarrow>
+  (\<E>(\<pi> ;; (LNext x) \<mapsto> \<langle>e;\<rho>(x \<mapsto> (VChan (Ch \<pi> x)));\<kappa>\<rangle>)) \<pi>' = Some (\<langle>e';\<rho>';\<kappa>'\<rangle>) \<Longrightarrow>
   \<forall>\<pi> e \<rho> \<kappa>. \<E> \<pi> = Some (\<langle>e;\<rho>;\<kappa>\<rangle>) \<longrightarrow> \<V> \<turnstile> e\<^sub>0 \<down> \<pi> \<mapsto> e \<and> \<V> \<tturnstile> e\<^sub>0 \<down> \<pi> \<mapsto> \<kappa> \<Longrightarrow>
   \<E> \<pi> = Some (\<langle>LET x = CHAN \<lparr>\<rparr> in e;\<rho>;\<kappa>\<rangle>) \<Longrightarrow> 
   \<V> \<turnstile> e\<^sub>0 \<down> \<pi>' \<mapsto> e'
@@ -351,7 +351,7 @@ lemma static_traceable_exp_preserved_under_chan:"
 done
 
 lemma static_traceable_exp_preserved_under_spawn: "
-  (\<E>(\<pi> ;; (LNext x) \<mapsto> \<langle>e;\<rho>(x \<mapsto> \<lbrace>\<rbrace>);\<kappa>\<rangle>, \<pi> ;; (LSpawn x) \<mapsto> \<langle>e\<^sub>c;\<rho>;[]\<rangle>)) \<pi>' = Some (\<langle>e';\<rho>';\<kappa>'\<rangle>) \<Longrightarrow>
+  (\<E>(\<pi> ;; (LNext x) \<mapsto> \<langle>e;\<rho>(x \<mapsto> VUnit);\<kappa>\<rangle>, \<pi> ;; (LSpawn x) \<mapsto> \<langle>e\<^sub>c;\<rho>;[]\<rangle>)) \<pi>' = Some (\<langle>e';\<rho>';\<kappa>'\<rangle>) \<Longrightarrow>
   \<forall>\<pi> e \<rho> \<kappa>. \<E> \<pi> = Some (\<langle>e;\<rho>;\<kappa>\<rangle>) \<longrightarrow> \<V> \<turnstile> e\<^sub>0 \<down> \<pi> \<mapsto> e \<and> \<V> \<tturnstile> e\<^sub>0 \<down> \<pi> \<mapsto> \<kappa> \<Longrightarrow>
   \<E> \<pi> = Some (\<langle>LET x = SPAWN e\<^sub>c in e;\<rho>;\<kappa>\<rangle>) \<Longrightarrow> 
   \<V> \<turnstile> e\<^sub>0 \<down> \<pi>' \<mapsto> e'
@@ -360,8 +360,8 @@ lemma static_traceable_exp_preserved_under_spawn: "
 done
  
 lemma static_traceable_exp_preserved_under_sync: "
-  \<E> \<rightarrow> \<E>(\<pi>\<^sub>s ;; (LNext x\<^sub>s) \<mapsto> \<langle>e\<^sub>s;\<rho>\<^sub>s(x\<^sub>s \<mapsto> \<lbrace>\<rbrace>);\<kappa>\<^sub>s\<rangle>, \<pi>\<^sub>r ;; (LNext x\<^sub>r) \<mapsto> \<langle>e\<^sub>r;\<rho>\<^sub>r(x\<^sub>r \<mapsto> \<omega>\<^sub>m);\<kappa>\<^sub>r\<rangle>) \<Longrightarrow>
-  (\<E>(\<pi>\<^sub>s ;; (LNext x\<^sub>s) \<mapsto> \<langle>e\<^sub>s;\<rho>\<^sub>s(x\<^sub>s \<mapsto> \<lbrace>\<rbrace>);\<kappa>\<^sub>s\<rangle>, \<pi>\<^sub>r ;; (LNext x\<^sub>r) \<mapsto> \<langle>e\<^sub>r;\<rho>\<^sub>r(x\<^sub>r \<mapsto> \<omega>\<^sub>m);\<kappa>\<^sub>r\<rangle>)) \<pi>' = Some (\<langle>e';\<rho>';\<kappa>'\<rangle>) \<Longrightarrow>
+  \<E> \<rightarrow> \<E>(\<pi>\<^sub>s ;; (LNext x\<^sub>s) \<mapsto> \<langle>e\<^sub>s;\<rho>\<^sub>s(x\<^sub>s \<mapsto> VUnit);\<kappa>\<^sub>s\<rangle>, \<pi>\<^sub>r ;; (LNext x\<^sub>r) \<mapsto> \<langle>e\<^sub>r;\<rho>\<^sub>r(x\<^sub>r \<mapsto> \<omega>\<^sub>m);\<kappa>\<^sub>r\<rangle>) \<Longrightarrow>
+  (\<E>(\<pi>\<^sub>s ;; (LNext x\<^sub>s) \<mapsto> \<langle>e\<^sub>s;\<rho>\<^sub>s(x\<^sub>s \<mapsto> VUnit);\<kappa>\<^sub>s\<rangle>, \<pi>\<^sub>r ;; (LNext x\<^sub>r) \<mapsto> \<langle>e\<^sub>r;\<rho>\<^sub>r(x\<^sub>r \<mapsto> \<omega>\<^sub>m);\<kappa>\<^sub>r\<rangle>)) \<pi>' = Some (\<langle>e';\<rho>';\<kappa>'\<rangle>) \<Longrightarrow>
   \<forall>\<pi> e \<rho> \<kappa>. \<E> \<pi> = Some (\<langle>e;\<rho>;\<kappa>\<rangle>) \<longrightarrow> \<V> \<turnstile> e\<^sub>0 \<down> \<pi> \<mapsto> e \<and> \<V> \<tturnstile> e\<^sub>0 \<down> \<pi> \<mapsto> \<kappa> \<Longrightarrow>
   (\<V>, \<C>) \<Turnstile>\<^sub>\<E> \<E> \<Longrightarrow>
   \<E> \<pi>\<^sub>s = Some (\<langle>LET x\<^sub>s = SYNC x\<^sub>s\<^sub>e in e\<^sub>s;\<rho>\<^sub>s;\<kappa>\<^sub>s\<rangle>) \<Longrightarrow>
@@ -459,25 +459,25 @@ proof -
   next
     case (Let_Chan \<pi> x e \<rho> \<kappa>)
 
-    assume "\<E>' = \<E> ++ [\<pi> ;; (LNext x) \<mapsto> \<langle>e;\<rho> ++ [x \<mapsto> \<lbrace>Ch \<pi> x\<rbrace>];\<kappa>\<rangle>]"
+    assume "\<E>' = \<E> ++ [\<pi> ;; (LNext x) \<mapsto> \<langle>e;\<rho> ++ [x \<mapsto> (VChan (Ch \<pi> x))];\<kappa>\<rangle>]"
     and "\<E> \<pi> = Some (\<langle>LET x = CHAN \<lparr>\<rparr> in e;\<rho>;\<kappa>\<rangle>)"
 
     from \<open>\<E>' \<pi>' = Some (\<langle>e';\<rho>';\<kappa>'\<rangle>)\<close> 
-    and \<open>\<E>' = \<E> ++ [\<pi> ;; (LNext x) \<mapsto> \<langle>e;\<rho> ++ [x \<mapsto> \<lbrace>Ch \<pi> x\<rbrace>];\<kappa>\<rangle>]\<close>
+    and \<open>\<E>' = \<E> ++ [\<pi> ;; (LNext x) \<mapsto> \<langle>e;\<rho> ++ [x \<mapsto> (VChan (Ch \<pi> x))];\<kappa>\<rangle>]\<close>
 
-    have \<open>(\<E>(\<pi> ;; (LNext x) \<mapsto> \<langle>e;\<rho> ++ [x \<mapsto> \<lbrace>Ch \<pi> x\<rbrace>];\<kappa>\<rangle>)) \<pi>' = Some (\<langle>e';\<rho>';\<kappa>'\<rangle>)\<close> by auto
+    have \<open>(\<E>(\<pi> ;; (LNext x) \<mapsto> \<langle>e;\<rho> ++ [x \<mapsto> (VChan (Ch \<pi> x))];\<kappa>\<rangle>)) \<pi>' = Some (\<langle>e';\<rho>';\<kappa>'\<rangle>)\<close> by auto
     with  \<open>\<forall>\<pi> e \<rho> \<kappa>. \<E> \<pi> = Some (\<langle>e;\<rho>;\<kappa>\<rangle>) \<longrightarrow> \<V> \<turnstile> e\<^sub>0 \<down> \<pi> \<mapsto> e \<and> \<V> \<tturnstile> e\<^sub>0 \<down> \<pi> \<mapsto> \<kappa>\<close> 
     and \<open>\<E> \<pi> = Some (\<langle>LET x = CHAN \<lparr>\<rparr> in e;\<rho>;\<kappa>\<rangle>)\<close>
 
     show "\<V> \<turnstile> e\<^sub>0 \<down> \<pi>' \<mapsto> e'" by (auto simp: static_traceable_exp_preserved_under_chan)
   next
     case (Let_Spawn \<pi> x e\<^sub>c e \<rho> \<kappa>)
-    assume "\<E>' = \<E> ++ [\<pi> ;; (LNext x) \<mapsto> \<langle>e;\<rho> ++ [x \<mapsto> \<lbrace>\<rbrace>];\<kappa>\<rangle>, \<pi> ;; (LSpawn x) \<mapsto> \<langle>e\<^sub>c;\<rho>;[]\<rangle>]"
+    assume "\<E>' = \<E> ++ [\<pi> ;; (LNext x) \<mapsto> \<langle>e;\<rho> ++ [x \<mapsto> VUnit];\<kappa>\<rangle>, \<pi> ;; (LSpawn x) \<mapsto> \<langle>e\<^sub>c;\<rho>;[]\<rangle>]"
     and "\<E> \<pi> = Some (\<langle>LET x = SPAWN e\<^sub>c in e;\<rho>;\<kappa>\<rangle>)"
 
-    from \<open>\<E>' \<pi>' = Some (\<langle>e';\<rho>';\<kappa>'\<rangle>)\<close> and \<open>\<E>' = \<E> ++ [\<pi> ;; (LNext x) \<mapsto> \<langle>e;\<rho> ++ [x \<mapsto> \<lbrace>\<rbrace>];\<kappa>\<rangle>, \<pi> ;; (LSpawn x) \<mapsto> \<langle>e\<^sub>c;\<rho>;[]\<rangle>]\<close>
+    from \<open>\<E>' \<pi>' = Some (\<langle>e';\<rho>';\<kappa>'\<rangle>)\<close> and \<open>\<E>' = \<E> ++ [\<pi> ;; (LNext x) \<mapsto> \<langle>e;\<rho> ++ [x \<mapsto> VUnit];\<kappa>\<rangle>, \<pi> ;; (LSpawn x) \<mapsto> \<langle>e\<^sub>c;\<rho>;[]\<rangle>]\<close>
 
-    have \<open>(\<E>(\<pi> ;; (LNext x) \<mapsto> \<langle>e;\<rho> ++ [x \<mapsto> \<lbrace>\<rbrace>];\<kappa>\<rangle>, \<pi> ;; (LSpawn x) \<mapsto> \<langle>e\<^sub>c;\<rho>;[]\<rangle>)) \<pi>' = Some (\<langle>e';\<rho>';\<kappa>'\<rangle>)\<close> by auto
+    have \<open>(\<E>(\<pi> ;; (LNext x) \<mapsto> \<langle>e;\<rho> ++ [x \<mapsto> VUnit];\<kappa>\<rangle>, \<pi> ;; (LSpawn x) \<mapsto> \<langle>e\<^sub>c;\<rho>;[]\<rangle>)) \<pi>' = Some (\<langle>e';\<rho>';\<kappa>'\<rangle>)\<close> by auto
     with \<open>\<forall>\<pi> e \<rho> \<kappa>. \<E> \<pi> = Some (\<langle>e;\<rho>;\<kappa>\<rangle>) \<longrightarrow> \<V> \<turnstile> e\<^sub>0 \<down> \<pi> \<mapsto> e \<and> \<V> \<tturnstile> e\<^sub>0 \<down> \<pi> \<mapsto> \<kappa>\<close> 
     and \<open>\<E> \<pi> = Some (\<langle>LET x = SPAWN e\<^sub>c in e;\<rho>;\<kappa>\<rangle>)\<close>
 
@@ -485,15 +485,15 @@ proof -
   next
     case (Let_Sync \<pi>\<^sub>s x\<^sub>s x\<^sub>s\<^sub>e e\<^sub>s \<rho>\<^sub>s \<kappa>\<^sub>s x\<^sub>s\<^sub>c x\<^sub>m \<rho>\<^sub>s\<^sub>e \<pi>\<^sub>r x\<^sub>r x\<^sub>r\<^sub>e e\<^sub>r \<rho>\<^sub>r \<kappa>\<^sub>r x\<^sub>r\<^sub>c \<rho>\<^sub>r\<^sub>e c \<omega>\<^sub>m)
 
-    assume "\<E>' = \<E> ++ [\<pi>\<^sub>s ;; (LNext x\<^sub>s) \<mapsto> \<langle>e\<^sub>s;\<rho>\<^sub>s ++ [x\<^sub>s \<mapsto> \<lbrace>\<rbrace>];\<kappa>\<^sub>s\<rangle>, \<pi>\<^sub>r ;; (LNext x\<^sub>r) \<mapsto> \<langle>e\<^sub>r;\<rho>\<^sub>r ++ [x\<^sub>r \<mapsto> \<omega>\<^sub>m];\<kappa>\<^sub>r\<rangle>]"
+    assume "\<E>' = \<E> ++ [\<pi>\<^sub>s ;; (LNext x\<^sub>s) \<mapsto> \<langle>e\<^sub>s;\<rho>\<^sub>s ++ [x\<^sub>s \<mapsto> VUnit];\<kappa>\<^sub>s\<rangle>, \<pi>\<^sub>r ;; (LNext x\<^sub>r) \<mapsto> \<langle>e\<^sub>r;\<rho>\<^sub>r ++ [x\<^sub>r \<mapsto> \<omega>\<^sub>m];\<kappa>\<^sub>r\<rangle>]"
     and "\<E> \<pi>\<^sub>s = Some (\<langle>LET x\<^sub>s = SYNC x\<^sub>s\<^sub>e in e\<^sub>s;\<rho>\<^sub>s;\<kappa>\<^sub>s\<rangle>)"
     and "\<E> \<pi>\<^sub>r = Some (\<langle>LET x\<^sub>r = SYNC x\<^sub>r\<^sub>e in e\<^sub>r;\<rho>\<^sub>r;\<kappa>\<^sub>r\<rangle>)"
 
     from \<open>\<E> \<rightarrow> \<E>'\<close> `\<E>' \<pi>' = Some (\<langle>e';\<rho>';\<kappa>'\<rangle>)` and `\<E>' \<pi>' = Some (\<langle>e';\<rho>';\<kappa>'\<rangle>)`
-    and \<open>\<E>' = \<E> ++ [\<pi>\<^sub>s ;; (LNext x\<^sub>s) \<mapsto> \<langle>e\<^sub>s;\<rho>\<^sub>s ++ [x\<^sub>s \<mapsto> \<lbrace>\<rbrace>];\<kappa>\<^sub>s\<rangle>, \<pi>\<^sub>r ;; (LNext x\<^sub>r) \<mapsto> \<langle>e\<^sub>r;\<rho>\<^sub>r ++ [x\<^sub>r \<mapsto> \<omega>\<^sub>m];\<kappa>\<^sub>r\<rangle>]\<close>
+    and \<open>\<E>' = \<E> ++ [\<pi>\<^sub>s ;; (LNext x\<^sub>s) \<mapsto> \<langle>e\<^sub>s;\<rho>\<^sub>s ++ [x\<^sub>s \<mapsto> VUnit];\<kappa>\<^sub>s\<rangle>, \<pi>\<^sub>r ;; (LNext x\<^sub>r) \<mapsto> \<langle>e\<^sub>r;\<rho>\<^sub>r ++ [x\<^sub>r \<mapsto> \<omega>\<^sub>m];\<kappa>\<^sub>r\<rangle>]\<close>
 
-    have "\<E> \<rightarrow> \<E>(\<pi>\<^sub>s ;; (LNext x\<^sub>s) \<mapsto> \<langle>e\<^sub>s;\<rho>\<^sub>s ++ [x\<^sub>s \<mapsto> \<lbrace>\<rbrace>];\<kappa>\<^sub>s\<rangle>, \<pi>\<^sub>r ;; (LNext x\<^sub>r) \<mapsto> \<langle>e\<^sub>r;\<rho>\<^sub>r ++ [x\<^sub>r \<mapsto> \<omega>\<^sub>m];\<kappa>\<^sub>r\<rangle>)"
-    and "(\<E>(\<pi>\<^sub>s ;; (LNext x\<^sub>s) \<mapsto> \<langle>e\<^sub>s;\<rho>\<^sub>s ++ [x\<^sub>s \<mapsto> \<lbrace>\<rbrace>];\<kappa>\<^sub>s\<rangle>, \<pi>\<^sub>r ;; (LNext x\<^sub>r) \<mapsto> \<langle>e\<^sub>r;\<rho>\<^sub>r ++ [x\<^sub>r \<mapsto> \<omega>\<^sub>m];\<kappa>\<^sub>r\<rangle>)) \<pi>' = Some (\<langle>e';\<rho>';\<kappa>'\<rangle>)" by auto+
+    have "\<E> \<rightarrow> \<E>(\<pi>\<^sub>s ;; (LNext x\<^sub>s) \<mapsto> \<langle>e\<^sub>s;\<rho>\<^sub>s ++ [x\<^sub>s \<mapsto> VUnit];\<kappa>\<^sub>s\<rangle>, \<pi>\<^sub>r ;; (LNext x\<^sub>r) \<mapsto> \<langle>e\<^sub>r;\<rho>\<^sub>r ++ [x\<^sub>r \<mapsto> \<omega>\<^sub>m];\<kappa>\<^sub>r\<rangle>)"
+    and "(\<E>(\<pi>\<^sub>s ;; (LNext x\<^sub>s) \<mapsto> \<langle>e\<^sub>s;\<rho>\<^sub>s ++ [x\<^sub>s \<mapsto> VUnit];\<kappa>\<^sub>s\<rangle>, \<pi>\<^sub>r ;; (LNext x\<^sub>r) \<mapsto> \<langle>e\<^sub>r;\<rho>\<^sub>r ++ [x\<^sub>r \<mapsto> \<omega>\<^sub>m];\<kappa>\<^sub>r\<rangle>)) \<pi>' = Some (\<langle>e';\<rho>';\<kappa>'\<rangle>)" by auto+
     with  \<open>\<forall>\<pi> e \<rho> \<kappa>. \<E> \<pi> = Some (\<langle>e;\<rho>;\<kappa>\<rangle>) \<longrightarrow> \<V> \<turnstile> e\<^sub>0 \<down> \<pi> \<mapsto> e \<and> \<V> \<tturnstile> e\<^sub>0 \<down> \<pi> \<mapsto> \<kappa>\<close> 
     and \<open>(\<V>, \<C>) \<Turnstile>\<^sub>\<E> \<E>\<close> 
     and \<open>\<E> \<pi>\<^sub>s = Some (\<langle>LET x\<^sub>s = SYNC x\<^sub>s\<^sub>e in e\<^sub>s;\<rho>\<^sub>s;\<kappa>\<^sub>s\<rangle>)\<close>
